riumes

“EPD

ENVIRONMENTAL PRODUCT DECLARATION

Contents

Programme information and verification
About us
Product description
Technical compliance
Scope of EPD
Product stage
Life cycle assessment (LCA) methodology
Background data
Explanation of averages
Allocation
Cut-off criteria
Key assumptions
Life cycle assessment (LCA) results
Environmental profiles
Other environmental information
Product specification
References

Contact information

OO OO © OO D D OÙ R ©

NO = = =
SO NO ©  —
Programme information and verification

An Environmental Product Declaration (EPD) is a standardised way of quantifying the potential environmental impacts of
a product or system. EPDs are produced according to a consistent set of rules — Product Category Rules (PCR) — that
define the requirements within a given product category. These rules are a key part of ISO 14025 as they enable
transparency and comparability between EPDs. This EPD provides environmental indicators for Humes precast steel-
reinforced concrete products manufactured at the Humes production facility in Tamworth (NSW) in Australia. This EPD is
a “cradle-to-gate” declaration covering production of the precast concrete products and their supply chain.

This EPD is verified to be compliant with EN 15804. EPD of construction products may not be comparable if they do not
comply with EN15804. EPDs within the same product category but from different programs or utilising different PCRs may
not be comparable. Holcim (Australia), as the EPD owner, has the sole ownership, liability and responsibility for the EPD.

Holcim (Australia) Pty Ltd
Level 7, 799 Pacific Highway
Declaration Owner Chatswood NSW 2067, Australia

Web: www.holcim.com.au 1 O | ci m

Phone: +61 2 9412 6600

EPD Australasia Limited
Address: 315a Hardy Street | E P D
Nel 7010, New Zeal

EPD Program Operator elson 7010, New Zea and AUSTRALASIA
Web: www.epd-australasia.com

Email: info@epd-australasia.com
Phone: +61 2 8005 8206

ENVIRONMENTAL PRODUCT DECLARATION

start2see Pty Ltd

309 / 2a Montrose Place

Hawthorn East Vic 3123, Australia
Web: www.start2see.com.au

Email: Rob.Rouwette@start2see.com.au
Phone: +61 403 834 470

START2SEE

LIFE CYCLE ASSESSMENTS

EPD Produced by:

EPD registration number: S-P-01544 1.0

Reference year for data: 2018-07-01 — 2019-06-30

CEN standard EN 15804 served as the core PCR

PCR: PCR 2012:01 Construction Products and Construction Services, Version 2.3, 2018-11-15
PCR 2012:01-SUB-PCR-G Concrete and concrete elements, version 2.3, 2018-11-22

LE TATEN ETC TT The Technical Committee of the International EPD® System.
by: Chair: Massimo Marino. Contact via info@environdec.com

Independent verification of

a me
the declaration and data, EPD process certification (Internal)

& EPD verification (External)

according to ISO 14025:

Third party verifier: Jeff Vickers, thinkstep-anz
Web: www.thinkstep-anz.com
Email: jeffvickers@thinkstep-anz.com

Phone: +61 2 8007 5770 7
Accredited or approved by: EPD Australasia anz

Precast Concrete

=
=
=)
e]
=)
TD
O
Le
ce)
=

tenant À PM (us Fa Hits
“ ». L

n | dif
RENE LAN
LL ASMAUEX
LUS AL Van TIC | V4 sul"
ae) 1 LL LE RAS PATENER 1 75
cute 4m mr. | pa" | =] = e | | : A

{ DEN pe a

L
|

V n! Ti

Humes Tamworth

[es
.2
É
Humes Concrete Products (Humes) is a division of Holcim E
(Australia) Pty Ltd which is owned by the world's largest &
building materials company, LafargeHolcim. Humes pride Mission
ourselves on delivering customised solutions to maximise Humes aims to be the most respected and

installation, performance, and budgetary outcomes for successfully operated company in our industry,
our clients. Today, Humes employs more than 600 people creating value for all of our stakeholders.

and is the largest civil precast concrete manufacturer in Secbeder cree cie eeer cie.

Australia. companies, LafargeHolcim, our vision is to perfect
progress as we provide the foundations for society's
future. Achieving our mission involves a

commitment to the following:

This EPD covers precast products manufactured at our
plant in Tamworth, NSW (Tamworth is highlighted in
Figure 1). We have ten factories around Australia
producing reinforced concrete products. Humes innovative solutions for our customers
Tamworth is one of two factories located in NSW and is employees with a passion for performance

presently supplying large infrastructure projects such as En Gen EE lELCENE corporate EURE
a forward-looking organisation

a culture that promotes sustainable
development
long-term financial performance

the Inland Rail Project.

At a Glance

We have a long history of engineering precast and

prestressed concrete solutions and, after 100 years of
manufacture, our product range has never been more
diverse, more competitive, or more in-tune with our
clients’ needs than it is today.

We offer a range of solutions for bridges and platforms,
road and rail infrastructure, tunnels and shafts, retaining
walls, pipeline systems, water treatment, reuse and
detention, and traffic management. We can customise
our solutions to ensure they create maximum value for
your project, accommodating your site conditions, design
requirements and construction factors.

The quality and reliability of Humes’ products and
services are the foundation of our success. Our ability to
deliver to client specifications on major projects across
Australia has established Humes as a valuable and
reliable partner.

Figure 1: Location of Humes’ precast concrete
production facilities

Precast Concrete 3
Product description

Humes manufacture a full range of box culverts,
ballast kerbs and wing wall sizes and
configurations. This EPD covers box culverts and
headwalls manufactured at Humes Tamworth, of
which a significant amount are supplied to the
Inland Rail Project.

Culvert products’ intended use is bridging for
pedestrian, fauna and stock crossings under road
and rail applications. Humes precast concrete box
culverts are also suitable for difficult site
conditions as installation requires minimal
excavation and backfill.

Reinforced concrete products are made from
coarse and fine aggregates, cement, water, and
steel reinforcement. Other material used can
include supplementary cementitious materials
(SCM) such as fly ash and chemical admixtures,
which have varied effects on the concrete
depending on the admixture used.

Humes Tamworth has already supplied over 4000
precast products to the Inland Rail Parkes to
Narromine (P2N) section. The culverts are
manufactured as inverted U-shape culverts (see
Figure 2 and Figure 3) and are both railway load
class 300LA and road class SM1600.

The culverts supplied are also classified as both
small and large box culverts, ranging from 600 mm
to 3000 mm span:; 450 to 2400 mm height and are
all 2400 mm in length. Wingwall units are
manufactured to fit the 450 to 2400 mm height
range of the culverts.

Figure 2: Schematic of steel cage in a large box
culvert

The product as supplied is non-hazardous. The
products included in this EPD do not contain any
substances of very high concern as defined by
European REACH regulation in concentrations
>0.1% (m/m).

Dust from this product is classified as Hazardous
according to the Approved Criteria for Classifying
Hazardous Substances 3'{ Edition (NOHSC 2004).
Precast concrete products and pipes are classified
as non-dangerous goods according to the
Australian Code for the Transport of Dangerous
Goods by Road and Rail. When concrete products
are cut, sawn, abraded or crushed, dust is created
which contains crystalline silica, some of which
may be respirable (particles small enough to go
into the deep parts of the lung when breathed in),
and which is hazardous. Exposure through
inhalation should be avoided.

Precast concrete products form part of the UN CPC
375 — "Concrete” industry classification and the
ANZSIC 2034 — "Concrete Product Manufacturing”
product group classification.

EPD for Tamworth precast products for infrastructure applications

Technical Compliance

Humes culvert units are designed and Table 1: Product content
manufactured to comply with AS 1597.1:2010

Precast reinforced concrete box culverts Part
1: Small culverts (not exceeding 1200 mm
span and 1200 mm height) and AS
1597.2:2013 Precast reinforced concrete box
culverts Part 2: Large culverts (exceeding 1200
mm span or 1200 mm height and up to and
including 4200 mm span and 4200 mm
height). Culverts supplied to the Inland Rail
project are also additionally compliant to RMS
QA Specification R16 Precast Reinforced
Concrete Box Culverts. In addition, culvert
units have a reference service life (RSL) of 100
years, when manufactured and installed in
accordance with AS1597.1 & AS1597.2. The

design load of rail way load class culverts is * Cement in concrete contains traces of Chromium VI (hexavalent).

300LA and the design load of road load class ** Crystalline silica (quartz) may be a constituent of sand, crushed stone,
. | | gravel and fly ash used in any particular concrete mix.

culverts is SM1600 in accordance with both *#* Cementitious additives may contain traces of metals.

AS5100 & AS1597 series requirements. The

ballast kerb and wing wall designs for the Note: Grout may be used to fill gaps between units.

Inland Rail project were supplied by Australian This grout is not included in the scope of this EPD.

Rail Track Corporation (ARTC) and are
manufactured to the design requirements.

Figure 3: Examples of box culverts and headwalls

CR ee

Multi-cell installation using Link Slab® unit Crown unit Invert unit

Headwalls for pipes Headwalls for box culverts

œ ©

Precast Concrete 5

Product Description

Scope of Environmental Product Declaration

This EPD covers the cradle-to-gate life cycle stages A1-A3. Downstream stages have not
been included as shown in Table 2 and Figure 4.

Table 2: Scope of EPD

c

A O)

ro) = ©

an (o) e) ©

=) an £ >

> 2  G ©

D G a e) =

D + = € =

» € GS < A a

a ” 2 = co) Z oO ra ci)

Le) ei [en dv _ _ =) [0] >

dus c c C © £ © © = U 0

2 + © + © œ M MIE, © NN © | = Ne D ©, MAR
m © + © + = © 9 2 2 + © à æ ‘x
>= eo = eo = CRE s 2 © © € œ Oo 6 d E
= E = © = & © 5 GG © 2 € à à n S
8 © © $ à g 8 D 9 5 2 2 à © £ à à 2
CO OH à +k £S D 2m «OC C0 0 + = à we
A1 A2 A3 A4 A5 B1 B2 B3 B4 B5 B6 B7 C1 C2 C3 C4 D

Scenario Scenario Scenario

Ÿ Ÿ Ÿ MND  MND MND MND MND MND MND NR  NR MND MND MND MND MND

= module is included in this study
MND = module is not declared; NR = module is not relevant

Figure 4: Cradle-to-gate life cycle of precast concrete products

A1 - Raw materials A3 - Manufacturing
Aggregate, sand, A2 - Transport to factory Waste concrete, diesel,
cement, water, steel, Sea, road, rail electricity, natural gas

admixture

k |
À

we

>

EPD for Tamworth precast products for infrastructure applications
Product Stage

Raw Material Stage A1

All raw materials used in the production of Humes
Concrete Products comply with the following
standards as required by AS1597.1 & AS1597.2:

e AS/NZS 3972: General purpose and blended
cements (SA 2010)

e AS 3582.1 Supplementary cementitious
materials Part 1: Fly Ash (SA 2016)

e AS/NZS 4671 Steel reinforcing materials (SA
2001)

e AS 2758.1 Aggregates and rock for
engineering purposes Part 1: Concrete
Aggregates (SA 2014)

e AS 1478 Chemical admixtures for concrete,
mortar and grout (SA 2000)

Transportation Stage A2

Raw materials are typically transported to our site
via articulated trucks. The impact of transportation
is determined from the specific supply sources for
Tamworth.

Manufacturing Stage A3

The typical manufacturing process of Humes
Concrete Products is by casting specially
formulated concrete into a reusable steel mould.
Compaction is achieved by utilising Self
Compacting Concrete (SCC), a special type of
concrete which can be placed and consolidated
under its own weight without vibration. The freshly
poured concrete and mould is then cured in a
temperature and humidity-controlled environment
to accelerate concrete curing before the product is
removed from the mould. After removal from the
mould the product is transferred to the outdoor
yard storage area where it continues to cure until it
is approved by final quality checks and transported
to the installation site.

Precast Concrete

7
Life Cycle Assessment (LCA) Methodology

Background Data

Primary data have been collected for the 2019
financial year (FY19) (1 July 2018 — 30 June 2019).
They have been sourced directly from Humes'
Tamworth factory that manufactures the precast
products. Background data have predominantly
been sourced from AusLCI and the AusLCI shadow
database. Data for reinforcing steel (bars) has been
sourced from our supplier's (nfraBuild — formerly
ARC/OnesSteel) EPD (registration number S-P-
00855) (OneSteel 2016). Data for admixtures have
been sourced from five EPDs published in
December 2015 by EFCA (European Federation of
Concrete Admixtures Associations Ltd.) (EFCA
2015a-e). As a result, the vast majority of the
environmental profiles of our products are based
on life cycle data that have been updated in the
last five years. Background data used are less than
10 years old.

Methodological choices have been applied in line
with EN 15804 (CEN 2013); deviations have been
recorded.

Explanation of Averages

Humes produces a large number of precast
products, each with unique characteristics (e.g.
class, length, height, width, thickness) and
composition (concrete composition, steel
reinforcement content). After careful consideration
of the range of precast products produced in
Tamworth for infrastructure applications, it was
decided that the best product groupings are based
on the type of product (box culverts and
headwalls), application (rail and road) and for box
culverts, their size (large and small).

This grouping reduces the variation within each group's

environmental profile while providing a clear delineation
for users of the EPD. This approach leads to six groups:

Box culverts for rail applications, small (600 - 1200
mm)

Box culverts for rail applications, large (>1200
mm)

Headwalls for rail applications

Box culverts for road applications, small (600 -
1200 mm)

Box culverts for road applications, large (> 1200
mm)

Headwalls for road applications

We have determined the reference product for each
group using the weighted average concrete
composition (across all precast products over FY19) and
the weighted average steel content per product group.
The reference product therefore represents the
product group as a whole, rather than a specific
product that can be ordered from the catalogue.

Allocation

The key processes that require allocation are:

Production of precast concrete products and
precast concrete pipes: All shared processes are
attributed to concrete products based on their
mass

Use of fly ash: AIT environmental impacts of the
power plant have been allocated to the main
product: electricity; fly ash has only received the
burdens of the transport to our sites

Use of steel scrap in reinforcement steel wire:
Recycling allocation has followed the polluter pays
principle in line with EN 15804 and the PCR. See
OneSteel's EPD (S-P-00855) of reinforcing rod, bar
and wire (OneSteel 2016).

EPD for Tamworth precast products for infrastructure applications
Cut-off Criteria

e The contribution of capital goods
(production equipment and infrastructure)
and personnel is outside the scope of the

LCA, in line with the PCR (Environdec 2018a).

e The amount of packaging used for
admixtures, lifters, bar chairs and mould oil
is well below the materiality cut-off, so
packaging materials and quantities have
therefore been estimated only.

Key Assumptions

This EPD covers all Self Compacting Concrete
(SCC) used at the Tamworth plant for
infrastructure products. The concrete composition
is taken from Humes’'s internal operating systems.
Some (<10%) of the SCC is supplied by a
neighbouring concrete plant that is not owned by
Humes. We have used the weighted average
composition for all SCC concrete used in FY19.

Precast Concrete

9

>
en
©
©
D
©
=
nd
@
€
<
O
—

Life Cycle Assessment (LCA) results

The background LCA serves as the foundation for this
EPD. An LCA analyses the environmental processes in
the value chain of a product. It provides a

The Tamworth products are generally manufactured
using one or two concrete mixes with little variation.

un
=
=)
n
(]
[a
<
O
2

The key variable is in the quantity of reinforcement

comprehensive evaluation of all upstream and steel used per tonne of final precast product.

downstream material and energy inputs and outputs. A large number of permutations have been included
The results are provided for a range of environmental

impact categories, in line with EN 15804 (CEN 2013).

based on the following declared unit:

1 tonne of precast reinforced concrete product
manufactured in Tamworth (NSW) for infrastructure
applications

Declared unit

After careful consideration, we ascertained that
| | | presenting the results for six distinct product groups
Precast reinforced concrete products are available in . . .
| j - using the above declared unit - would best limit any
numerous shapes and sizes. Multiple products can be
presented collectively (groupedl) if the variation

between their environmental profiles is within +10%.

variations in environmental profiles while providing a
clear delineation for users of the EPD. This means that
the variation range for some indicators exceeds the
10% threshold (see page 15).

Table 3: Environmental indicators

Global warming impact of greenhouse gases such as carbon
dioxide (CO2), measured in kg CO2 equivalents using a global
warming potential over a 100-year time horizon.

Global Warming

Potential EU kg CO: eq

Relative impact that the product can cause to the stratospheric

Ozone Depletion ODP kg CFC-11 eq ozone layer, measured in kg trichlorofluoromethane (CFC-11)

Potential

equivalents
Acidification AP ka SO, € Increase of soil and water acidity that the product can cause,
Potential J9726q measured in kg sulphur dioxide (SO2) equivalents.
eo . Potential impact of nutrification by nitrogen and phosphorus to
Eutrophication 3- - :
. EP kg PO: eq  aquatic and terrestrial ecosystems, for example through algal
Potential . 3- :
blooms, measured in kg phosphate (PO4”) equivalents.
. Also known as summer smog, the potential impact from
Photochemical nn - : .
- oxidising of volatile compounds in the presence of nitrogen
Ozone Creation POCP kg C2H4 eq - - .
. oxides (NO,) which frees ozone in the low atmosphere,
Potential - .
measured in kg ethene (C2Hz) equivalents.
oi - Techno-economic impact from the depletion of scarce non-
Abiotic Depletion . :
- ADPE kg Sb eq renewable resources such as metals, measured in kg antimony
Potential (Elements) .
equivalents.
Abiotic Depletion Techno-economic impact from depletion of fossil fuel
Potential (Fossil ADPF M) resources such as oil or natural gas, expressed using their net
Fuels) calorific value.

Precast Concrdte 11
Table 4: Parameters describing resource use, waste and output flows

Parameters describing resource use
Use of renewable primary energy excluding renewable primary energy resources
used as raw materials
Use of renewable primary energy resources used as raw materials
Total use of renewable primary energy resources

Use of non-renewable primary energy excluding non-renewable primary energy
resources used as raw materials

Use of non-renewable primary energy resources used as raw materials
Total use of non-renewable primary energy resources

Use of secondary material

Use of renewable secondary fuels

Use of non-renewable secondary fuels

Use of net fresh water
Waste categories

Hazardous waste disposed
Non-hazardous waste disposed

Radioactive waste disposed
Output flows

Components for re-use
Materials for recycling
Materials for energy recovery

Exported energy

12 EPD for Tamworth precast products for infrastructure applications

PERE

PERM
PERT

PENRE

PENRM
PENRT
SM
RSF
NRSF
FW

HWD
NHWD
RWD

CRU

MER

MER
EE

Mincv

Mincv
Mincv

Mincv

Mincv
Mincv
kg
Mincv
Mincv

kg
kg
kg

kg
kg
kg
MJ
Environmental profiles

Cradle-to-gate (A1-A3)
Box culverts for rail applications, small (600 - 1200 mm)

Box culverts for rail applications, large (>1200 mm)
The cradle-to-gate environmental indicators of

un
=
=)
n
(o]
[a
<
O
2

Head walls for rail applications
each product group are expressed per tonne of

Box culverts for road applications, small (600 - 1200 mm)

average precast product for: Box culverts for road applications, large (>1200 mm)

VNVYNNVYNN NV

Head walls for road applications

Table 5: Environmental indicators, precast concrete products for rail applications, stages A1-A3,
per tonne

GWP [kg CO: eq] 2.75E+02 3.27E+02 3.25E+02
ODP [kg CFC11 eq] 3.70E-06 3.68E-06 3.68E-06
AP [kg SO: eq] 7.29E-01 9.18E-01 9.13E-01
EP [kg PO4Ÿ eq] 1.27E-01 1.45E-01 1.44E-01
POCP [kg C2H4 eq] 6.48E-02 9.12E-02 9.05E-02
ADPE [kg Sb eq] 2.49E-05 3.78E-05 3.75E-05
ADPF [MJncv] 2.36E+03 2.97E+03 2.96E +03
PERE [MJncv] 7.12E+01 1.05E+02 1.04E+02
PERM [Minc] 1.28E-02 1.23E-02 1.23E-02
PERT [Mincv] 7.12E+01 1.05E+02 1.04E+02
PENRE [Mincv] 2.44E+03 3.09E+03 3.07E+03
PENRM [Minc] 8.06E+00 7.74E+00 7.75E+00
PENRT [Mincv] 2.44E+03 3.10E+03 3.08E+03
SM [kg] 4.37E+01 7.98E+01 7.88E+01
RSF [MJncv] 1.05E-08 1.05E-08 1.05E-08
NRSF [Minc] 3.00E+00 5.49E+00 5.43E+00
FW [mi] 1.99E+00 2.20E+00 2.19E+00
HW [kg] 2.55E-05 3.69E-05 3.66E-05
NHW [kg] 1.69E+01 2.99E+01 2.96E +01
RW [kg] 3.64E-03 5.15E-03 5.11E-03

CRU [kg] (0) 0 (0)
MER [kg] 3.58E+00 3.87E+00 3.86E+00
MER [kg] 1.36E-02 2.44E-02 241E-02

EE [MJ] (0) 0 (0)

Precast Concrete 13
Table 6: Environmental indicators, precast concrete products for road applications, stages A1-A3,

per tonne

GWP [kg CO: eq] 2.52E+02 2.95E+02 2.74E+02
ODP [kg CFC11 eq] 3.70E-06 3.69E-06 3.70E-06
AP [kg SO eq] 6.A5E-01 8.00E-01 7.25E-01
EP [kg PO4* eq] 1.19E-01 1.34E-01 1.27E-01
POCP [kg C2H4 eq] 5.30E-02 7 ATE-02 6.43E-02
ADPE [kg Sb eq] 1.92E-05 2.97E-05 2.47E-05
ADPF [Mincv] 2.08E+03 2.59E+03 2.35E+03
PÈRE [Mincv] 5.59E+01 8.39E +01 7.04E+01
PERM [MJncv] 1.31E-02 1.27E-02 1.29E-02
PERT [MJncv] 5.59E+01 8.39E+01 7.05E+01
PENRE [Mncv] 2.14E+03 2.68E+03 2.42E+03
PENRM [Mincv] 8.21E+00 7.94E+00 8.07E+00
PENRT [MJncv] 2.15E+03 2.69E +03 2.43E+03
SM [kg] 2.77E+01 5.72E+01 4.30E +01
RSF [Minc] 1.05E-08 1.05E-08 1.05E-08
NRSF [Mncv] 1.89E+00 3.93E+00 2.95E+00
FW [mi] 1.89E+00 2.07E+00 1.98E+00
HW [kg] 2.04E-05 2.98E-05 2.52E-05
NHW [kg] 1.11E+01 2.17E+01 1.66E+01
RW [kg] 2.97E-03 4.20E-03 3.61E-03
CRU [kg] 0 0 0

MER [kg] 3.A6E +00 3.69E+00 3.58E+00
MER [kg] 8.84E-03 1.76E-02 1.34E-02
EE [MI] 0 0 0

14 EPD for Tamworth precast products for infrastructure applications
Variation (A1-A3) per impact category

The LCA results shown in the previous tables represent a weighted average product produced in Tamworth.
No product exceeds the global warming potential of the weighted average product by more than 10%. Some
individual products do exceed a variation from the weighted average product by more than +10%, most
likely for Photochemical Ozone Creation Potential (POCP) and Abiotic Depletion Potential (Elements) (ADPE)
indicators. For transparency, Table 7 displays the maximum variation found in the environmental profile of

un
=
=)
n
(]
[a
<
O
2

each product group. Note: the minimum/maximum range indicates the extremes. The vast majority of our
products are within 410% of the environmental profiles presented in this EPD.

Table 7: Range in LCA results (stages A1-A3)

GWP [kg CO» eq] -9% 0% -11% 8% -11% 8%
ODP [kg CFC11 eq] 0% 0% 0% 0% 0% 0%
AP [kg SO> eq] -12% 1% -14% 10% -14% 11%
EP [kg PO4 eq] -7% 0% -8% 6% -8% 7%
POCP [kg CH eq] -19% 1% -20% 14% -20% 16%
ADPE [kg Sb eq] -24% 1% -23% 17% -23% 18%
ADPF [Mincv] -12% 1% -14% 10% -14% 11%
GWP [kg CO» eq] -5% 7% -2% 7% -10% 4%
ODP [kg CFC11 eq] 0% 0% 0% 0% 0% 0%
AP [kg SO eq] -8% 10% -3% 9% -14% 6%
EP [kg PO4* eq] 4% 5% -2% 5% -7% 3%
POCP [kg C2H4 eq] -13% 16% -5% 13% -21% 9%
ADPE [kg Sb eq] -17% 22% -6% 16% -27% 12%
ADPF [Mincv] -8% 10% -3% 9% -14% 6%

Precast Concrete 15
Other environmental information

Our safety, health and environment (SHE) management system aims to achieve high environmental
standards. The Holcim executive committee closely monitors our performance in managing workplace safety
and protection of the environment. The environmental component of the management system helps identify
and manage potential environmental risks. Operations are assessed against the requirements and
improvements made.

Infrastructure Sustainability

The Infrastructure Sustainability Council of Australia (ISCA) is the peak industry body for advancing
sustainability in Australia's infrastructure. As a division of Holcim Australia, Humes is a member of ISCA and
takes an interest and role in developing sustainable practises across design, construction and operation of
infrastructure.

ISCA has developed the Infrastructure Sustainability (IS) rating scheme which is Australia's only
comprehensive rating scheme for evaluating sustainability for infrastructure. IS evaluates the sustainability of
infrastructure projects and assets and assigns credits across a number of categories which incentivise the use
of sustainable practises.

Humes helps its customers optimise their IS ratings through smart selection and design of precast products.

This is our second Environmental Product Declaration. In 2016, we developed an ISO 14025 and EN 15804
compliant EPD for our reinforced concrete pipe products. That EPD is publicly available on the EPD
Australasia website: https://epd-australasia.com/epd/reinforced-concrete-pipe-rcp/

|

D. "à "ANNE

“à | |
nn ce _

16 EPD for Tamworth precast products for infrastructure applications
Product Specification

The following tables are provided so the potential environmental impact can be calculated for a specific
product weight. The value in the table represents the product's weight in tonnes so that the results of the
LCA can be converted to product units. Please note that these product weights represent products for the
P2N section of the Inland Rail Project. Further sections or other infrastructure applications may have varying
designs that may alter the unit's weight.

[es
2
re

[ae]

©
=

O

U

[en
un
+

e]

>
TD

[e]

nn
[…s

Table 8: Product Mass Guide, Small Box Culvert Railway Load Class 300LA, Tamworth,
tonnes per unit

— Span Height | Length

Precast Concrete 17
Table 9: Product Mass Guide, Large Box Culvert Railway Load Class 300LA, Tamworth,

tonnes per unit

1500 x 600 x 2400mm Box Culvert c/w 600 x 250 Ballast Wall - 300LA 1500 600 2400 4.688
1500 x 600 x 2400mm Box Culvert -300LA 1500 600 2400 4.002
1800 x 600 x 2400mm Box Culvert c/w 600 x 250 Ballast Wall - 300LA 1800 600 2400 5.478
1800 x 600 x 2400mm Box Culvert - 300LA 1800 600 2400 4.730
1800 x 800 x 2400mm Box Culvert c/w 600 x 250 Ballast Wall - 300LA 1800 800 2400 5.400
1800 x 900 x 2400mm Box Culvert c/w 600 x 250 Ballast Wall - 300LA 1800 900 2400 5.586
1800 x 900 x 2400mm Box Culvert - 300LA 1800 900 2400 4.776
1800 x 1200 x 2400mm Box Culvert c/w 600 x 250 Ballast Wall - 3OOLA 1800 1200 2400 6.870
1800 x 1200 x 2400mm Box Culvert - 300LA 1800 1200 2400 6.050
2400 x 800 x 2400mm Box Culvert c/w 600 x 250 Ballast Wall - 3O0LA 2400 800 2400 8.345
2400 x 800 x 2400mm Box Culvert - 300LA 2400 800 2400 7.267
2400 x 900 x 2400mm Box Culvert c/w 600 x 250 Ballast Wall - 300LA 2400 900 2400 8.500
2400 x 900 x 2400mm Box Culvert - 300LA 2400 900 2400 7.400
2400 x 1200 x 2400mm Box Culvert c/w 600 x 250 Ballast Wall - 300LA 2400 1200 2400 9.000
2400 x 1200 x 2400mm Box Culvert - 300LA 2400 1200 2400 7.900
2400 x 1500 x 2400mm Box Culvert c/w 600 x 250 Ballast Wall - 300LA 2400 1500 2400 9.900
2400 x 1500 x 2400mm Box Culvert - 300LA 2400 1500 2400 8.800
2400 x 1800 x 2400mm Box Culvert c/w 600 x 250 Ballast Wall - 300LA 2400 1800 2400 10.970
3000 x 1100 x 2400mm Box Culvert c/w 600 x 250 Ballast Wall - 300LA 3000 1100 2400 11.700
3000 x 1200 x 2400mm Box Culvert c/w 600 x 250 Ballast Wall - 300LA 3000 1200 2400 11.880
3000 x 1200 x 2400mm Box Culvert - 300LA 3000 1200 2400 10.600
3000 x 1500 x 2400mm Box Culvert c/w 600 x 250 Ballast Wall - 300LA 3000 1500 2400 12.700
3000 x 1800 x 2400mm Box Culvert c/w 600 x 250 Ballast Wall - 300LA 3000 1800 2400 13.500
3000 x 2100 x 2400mm Box Culvert c/w 600 x 250 Ballast Wall - 300LA 3000 2100 2400 14.700
3000 x 2400 x 2400mm Box Culvert c/w 600 x 250 Ballast Wall - 300LA 3000 2400 2400 15.500

18 EPD for Tamworth precast products for infrastructure applications
Table 10: Product Mass Guide, Headwall / Wingwall Railway Load Class 300LA, Tamworth,

tonnes per unit

Wing Wall 450mm High Segment 1 - 300LA
Wing Wall 450mm High Segment 2 - 300LA
Wing Wall 600mm High Segment 1 - 300LA
Wing Wall 600mm High Segment 2 - 300LA
Wing Wall 800mm High Segment 1 - 300LA
Wing Wall 800mm High Segment 2 - 300LA
Wing Wall 800mm High Segment 3 - 300LA
Wing Wall 900mm High Segment 1 - 300LA
Wing Wall 900mm High Segment 2 - 300LA
Wing Wall 900mm High Segment 3 - 300LA
Wing Wall 1100mm High Segment 1 - 300LA
Wing Wall 1100mm High Segment 2 - 300LA
Wing Wall 1100mm High Segment 3 - 300LA
Wing Wall 1200mm High Segment 1 - 300LA
Wing Wall 1200mm High Segment 2 - 300LA
Wing Wall 1200mm High Segment 3 - 300LA
Wing Wall 1500mm High Segment 1 - 300LA
Wing Wall 1500mm High Segment 2 - 300LA
Wing Wall 1500mm High Segment 3 - 300LA
Wing Wall 2100mm High Segment 1 - 300LA
Wing Wall 2100mm High Segment 2 - 300LA
Wing Wall 2100mm High Segment 3 - 300LA
Wing Wall 2100mm High Segment 4 - 300LA
Wing Wall 2400mm High Segment 1 - 300LA
Wing Wall 2400mm High Segment 2 - 300LA
Wing Wall 2400mm High Segment 3 - 300LA

Wing Wall 2400mm High Segment 4 - 300LA

2.760

1.950

2.930

2.500

3.120

2.650

0.550

3.190

2.750

0.700

3.380

3.070

1.170

3.460

3.250

1.400

5.500

4.170

2.100

8.441

6.675

3.074

0.987

8.850

7.100

3.500

1.700

Precast Concrete

19
Table 11: Product Mass Guide, Small Box Culvert Road Load Class SM1600, Tamworth,
tonnes per unit

_. Span Height | Length

Table 12: Product Mass Guide, Large Box Culvert Road Load Class SM1600, Tamworth,
tonnes per unit

_. Span Height | Length

20 EPD for Tamworth precast products for infrastructure applications
Table 13: Product Mass Guide, Headwall / Wingwall Road Load Class SM1600, Tamworth,

tonnes per unit

Headwall to suit box culverts 600 x 450 single cell
Headwall to suit box culverts 600 x 300 single cell
Headwall to suit 750 diameter pipe two cell
Headwall to suit 600 diameter pipe two cell
Headwall to suit box culverts 900 x 600 two cell
Headwall to suit box culverts 1800 x 600 single cell
Headwall to suit box culverts 900 x 600 three cell
Headwall to suit box culverts 1200 x 600 two cell
Headwall to suit 750 diameter pipe three cell
Headwall to suit box culverts 600 x 450 four cell
Headwall to suit 750 diameter pipe four cell
Headwall to suit box culverts 1800 x 900 single cell
Headwall to suit box culverts 2400 x 900 single cell
Wing wall to suit 1595 high in situ cast headwall
Wing wall to suit 995 high in situ cast headwall

Wing wall to suit 1255 high in situ cast headwall

0.584

0.573

2.000

2.190

1.712

1.737

4.056

2.107

2.578

1.914

3.426

3.693

3.459

0.940

0.524

0.528

Precast Concrete

21
References

CEN 2013

EFCA 2015a

EFCA 2015b

EFCA 2015c

EFCA 20154

EFCA 2015e

Environdec 2018a

Environdec 2018b

ISO 2006a

ISO 2006b

ISO 2006c

EN 15804:2012+A1:2013, Sustainability of construction works — Environmental
product declarations — Core rules for the product category of construction
products, European Committee for Standardization (CEN), Brussels, November
2013

EPD of Plasticizer and superplasticizer, IBU EPD Declaration number EPD-EFC-
20150091-IAG1-EN, issued 14-09-2015, based on EN 15804 and PCR for concrete
admixtures; EPD owner: EFCA - European Federation of Concrete Admixtures
Associations

EPD of Set accelerators, IBU EPD Declaration number EPD-EFC-20150087-IAG1-EN,
issued 14-09-2015, based on EN 15804 and PCR for concrete admixtures; EPD
owner: EFCA - European Federation of Concrete Admixtures Associations

EPD of Hardening accelerators, IBU EPD Declaration number EPD-EFC-20150089-
IAG1-EN, issued 14-09-2015, based on EN 15804 and PCR for concrete admixtures;
EPD owner: EFCA - European Federation of Concrete Admixtures Associations

EPD of Air entrainers, IBU EPD Declaration number EPD-EFC-20150086-IAG1-EN,
issued 14-09-2015, based on EN 15804 and PCR for concrete admixtures; EPD
owner: EFCA - European Federation of Concrete Admixtures Associations

EPD of Retarders, IBU EPD Declaration number EPD-EFC-20150088-IAG1-EN,
issued 14-09-2015, based on EN 15804 and PCR for concrete admixtures; EPD
owner: EFCA - European Federation of Concrete Admixtures Associations

PCR2012:01 (version 2.3), Product category rules according to ISO 14025 and EN
15804, Combined PCR and PCR Basic Module for Construction products and
Construction services, registration number 2012:01, published on 15 November
2018

PCR2012:01-SUB-PCR-G (version 2.3), Product category rules according to ISO
14025 and EN 15804, Concrete and concrete elements (EN 16757:2017),
registration number 2012:01, published on 22 November 2018

ISO 14040:2006 Environmental management - Life cycle assessment - Principles
and framework. International Organization for Standardization, Geneva,
Switzerland, 2006

IS014044:2006, Environmental management - Life cycle assessment -
Requirements and guidelines. International Organization for Standardization,
Geneva, Switzerland, 2006

IS014025:2006, Environmental labels and declarations - Type Ill environmental
declarations - Principles and procedures. International Organization for
Standardization, Geneva, Switzerland, 2006

22 EPD for Tamworth precast products for infrastructure applications
NOHSC 2004 Approved criteria for classifying hazardous substances [NOHSC: 1008(2004)], 3" .
Edition, National Occupational Health and Safety Commission, Canberra, October =
2004 ©
©
[a 4
OneSteel 2016 EPD of Reinforcing Rod, Bar & Wire, EPD Declaration number EPD-S-P-00855,

issued 14-11-2016, based on EN 15804 and PCR for construction products and
services; EPD owner: OneSteel

SA 2000 AS 1478.1:2000 Chemical admixtures for concrete, mortar and grout, Part 1:
Admixtures for concrete, published on 4 October 2000 by Standards Australia,
Sydney

SA 2001 AS/NZS 4671:2001 Steel reinforcing materials, published on 2 April 2001 by

Standards Australia, Sydney

SA 2010 AS 3972-2010 General Purpose and blended cements, published on 22 October
2010 by Standards Australia, Sydney

SA 2014 AS 2758.1:2014 Aggregates and rock for engineering purposes Part 1: Concrete
aggregates, published on 7 November 2014 by Standards Australia, Sydney

SA 2016 AS/NZS 3582.1:2016 Supplementary cementitious materials Part 1: Fly Ash,
published on 12 February 2016 by Standard Australia, Sydney

Precast Concrete 23
Contact information

National sales 1300 361 601

humes.com.au
info@humes.com.au

Head Office

18 Little Cribb St
Milton 4064 OLD
Ph: (07) 3364 2800
Fax: (07) 3364 2963

Queensland

Ipswich/Brisbane
Ph: (07) 3814 9000
Fax: (07) 3814 9014

Rockhampton
Ph: (07) 4924 7900
Fax: (07) 4924 7901

Townsville
Ph: (07) 4758 6000
Fax: (07) 4758 6001

24 EPD for Tamworth precast products for infrastructure applications

New South Wales

Grafton
Ph: (02) 6644 7666
Fax: (02) 6644 7313

Newcastle
Ph: (02) 4032 6800
Fax: (02) 4032 6822

Sydney
Ph: (02)9832 5555
Fax: (02) 9625 5200

Tamworth
Ph: (02) 6763 7300
Fax: (02) 6763 7301

Victoria

Echuca
Ph: (03) 5480 2371
Fax: (03) 5482 3090

Melbourne
Ph: (03) 9360 3888
Fax: (03) 9360 3887

South Australia

Adelaide
Ph: (08) 8168 4544
Fax: (08) 8168 4549

Western Australia

Gnangara
Ph: (08) 9302 8000
Fax: (08) 9309 1625

Perth
Ph: (08) 9351 6999
Fax: (08) 9351 6977

Northern Territory

Darwin
Ph: (08) 8984 1600
Fax: (08) 8984 1614
National sales 1300 361 601
humes.com.au
info@humes.com.au

A Division of Holcim Australia

This publication supersedes all previous literature on this subject. As the specifications and details contained in this publication may change
please check with Humes Customer Service for confirmation of current issue. This publication provides general information only and is no
substitute for professional engineering advice. No representations or warranties are made regarding the accuracy, completeness or relevance
of the information provided. Users must make their own determination as to the suitability of this information or any Humes’ product for their
specific circumstances. Humes accepts no liability for any loss or damage resulting from any reliance on the information provided in this
publication. Humes is a registered business name and registered trademark of Holcim (Australia) Pty Ltd (Holcim). “Strength. Performance.
Passion.” is a trademark of Holcim.

© January 2020 Holcim (Australia) Pty Ltd ABN 87 099 732 297. Al rights reserved. This guide or any part of it may not be reproduced without
prior written consent of Holcim.
