® ECO PLATFORM
] o AUSTRALASIA pre ml 2 P D E D D
O C l Ï Ï Ï ENVIRONMENTAL PRODUCT DECLARATION

Ê:

ViroDecs'" Aggregates

Holcim Australia Aggregates

Environmental Product Declaration

In accordance with ISO 14025 and EN 15804+A1

Programme: The International EPD® System | www.environdec.com
Programme operator: EPD Australasia Limited | www.epd-australasia.com
EPD registration No. S-P-02332

Valid from 18 May 2021 | Valid until 17 May 2026

Version Date: 11 May 2023

Version: 2

Geographical scope: Australia

Contents

Introduction 3
About Holcim 4
ViroDecsT" - à first for raw aggregates in Australia 5
Why have we developed this EPD? 6
Aggregate products 7
Strategy 2025 — “Accelerating Green Growth” 8
Supporting sustainable construction 9
How the EPD can be used in the IS and Green Star rating schemes 10
Holcim’s management systems 11
LCA information 12
EPD product description 16
Environmental performance 18
Interpretation 22
References 24
Programme - related information and verification 25
Contact information 26

Version Revision Date Description of Changes

Environmental impact results have been updated following a correction to the calculation
2.0 11 May 2023 formulas, resulting in an increase to the overall environmental impact of the products.
Recycled aggregate products have been removed from this EPD.

ViroDecs'" Aggregates EPD | Holcim 2
Introduction

All around the world, the expectation for Governments
and organisations to provide enhanced transparency
and disclosure of environmental impacts, such as
greenhouse gas (GHG) emissions, has been growing.
This follows the landmark COP 21 Paris Agreement in
2015 in which all nations agreed to ambitiously pursue
efforts to combat climate change and its effects.

Atthe same time, the global demand for construction
materials is also growing due to worldwide population
growth and an increase in urbanisation.

This clearly demonstrates both the essential need for
construction materials now and in the future, as well
as the necessity for the construction materials industry
to be a leading part of the solution addressing climate
change.

At Holcim, we recognise our responsibility to
contribute to global emissions reduction targets and
we have developed a roadmap with a number of
actions to direct our efforts.

Our ViroDecs'" range of aggregates represented by
an Environmental Product Declaration (EPD) is one
such initiative for Holcim in Australia.

ViroDecs'" Aggregates EPD | Holcim

=
Q
2
©
5
D
©
Lu
L 2
=

About Holcim

Western
Australia

e Perth

AUSTRALIAN OPERATIONS

Quarries
| 190" Concrete

Precast pipe and product

*Darwin
Northern [nn]
Territory
Queensland [3
e Brisbane
South
Australia
rs. New South |.
Wales] ACT FA
a
e Adelaide e Canberra ES
Victoria
* Melbourne Un.
Tasmania E

eHobart

*The breakdown of Australian quarry operations is based on 2019 site data used for the EPD Life Cycle Assessment modelling.
1 The breakdown of Australian concrete operations is based on the 2019 ViroDecs/" ready-mix concrete EPD). It includes tolling sites and excludes mobile or temporary sites.

About Holcim

Holcim Australia is a leading supplier of construction
materials in Australia, dating back to 1901. Today
Holcim continues to supply essential construction
materials including aggregates, sand, ready-mix
concrete, engineered precast concrete and
prestressed concrete solutions to a range of
customers and projects throughout Australia.

Holcim operates right across the Australian continent
supplying concrete from a network of concrete plants,
quarries, precast and concrete pipe places, and
mobile and on-site project facilities.

Sustainability is at the core of our global strategy, with
our industry's first 2050 net-zero targets, endorsed by
the Science Based Targets initiative (SBTi).

Globally, Holcim is 60,000 people around the world
who are passionate about building progress for people
and the planet through four business segments:
Cement, Ready-Mix Concrete, Aggregates and
Solutions & Products.

Holcim builds progress for people and the planet. As a
global leader in innovative and sustainable building
solutions, Holcim is enabling greener cities, smarter
infrastructure and improving living standards around
the world. With sustainability at the core of its strategy
Holcim is becoming a net zero company, with its
people and communities at the heart of its success.
The company is driving circular construction as a
world leader in recycling to build more with less.

ViroDecs'" Aggregates EPD | Holcim 4
Holcim ViroDecs'"" Aggregates - a first
for raw aggregates in Australia

ViroDecs"" Aggregates at a glance

The Holcim ViroDecs'" Aggregates initiative for
Environmental Product Declarations (EPDs)
constitutes a major investment in comprehensively
analysing and communicating to customers the
embodied environmental impacts of Holcim's
products.

Data collected from across Holcim's Australian
operations, including 41 quarries, was fed into an
1S014044-compliant Life Cycle Assessment (LCA)
model by specialist practitioners to generate an
Environmental Product Declaration (EPD) to ISO
14025 and EN 15804, which have been independently
reviewed by an approved, third-party verifier.

The development of a raw aggregates EPD is a
“missing” piece to having all key infrastructure and
building materials represented by an EPD in Australia.
Its publication will support our customers to drive
improved sustainable procurement and materials
selection. Holcim's ViroDecs'" also have the potential
to challenge common beliefs of environmental
sustainability, by supporting the standardisation and
transparency of environmental claims.

Holcim's ViroDecsTM will help shape the way the
construction industry analyses the environmental
impact of buildings and infrastructure now and in the
future. Advancing from generic environmental
information to product, company and geographically-
specific information will allow for deeper, broader
and more customised analysis with greater
confidence in the results.

Beyond providing greater transparency, Holcim's
ViroDecs'" also provide a rigorous, science-based
framework for driving environmental improvement
throughout Holcim's sites and supply chains.

As a result, Holcim's ViroDecs'T" will offer an
advantage to customers wanting to be leaders in the
sustainable infrastructure and building industry.
Holcim hopes it will lead the way for other providers
to follow suit, fostering a whole-of-life approach in
the Australian construction materials industry.

ViroDecs'" Aggregates EPD | Holcim

5

Why have we developed this EPD?

EPD and project life cycle models

Landfill Decommissioning

Recovery & | Demand
processing

Raw material
extraction (A1)

Demolition
Operation = Optioneering
Use &maintenance Project

ViroDecs” # ‘| life cycle /

Transport ofraw
materials (A2)

Manufacture (A3) crane Concept&approvals

FT * Transport Pa NN
tosite Design

Developed in conjunction with Edge Environment

Note: ViroDecs TM Aggregates EPD only covers EPD lifecycle stages A1 to A3

One significant means of providing transparency at
the product level is the publication of Environmental
Product Declarations.

In simple terms, an EPD is a comprehensive
disclosure of a product's environmental impacts. An
EPD can cover the different stages of a products life
cycle, from its creation and use to disposal, as well as
other relevant information in accordance with
recognised international standards.

The ViroDecs'" Aggregates EPD covers EPD
lifecycle stages from raw material extraction (Stage
A1), through to manufacturing of the aggregates
(Stage A3).

EPDSs provide credible transparency because they rely
on an objective, scientifically accepted approach,
defined in international and European standards, and
are third party verified and publicly available.

ViroDecs'" Aggregates EPD | Holcim 6
Aggregate products

Load and Haul

Crushing and
Screening

Stockpiling and Distribution

Summary of aggregate products

In simple terms, Aggregates, generally consisting of
crushed stone, gravel, and sand, are mainly used in
the construction of roads, rail track beds, the
manufacturing of concrete, concrete products, and
asphalt. Aggregates are rock fragments extracted
from earth deposits as in the case of natural sand and
gravel or quarried from hard rock formations. The
extracted materials are then processed by crushing,
shaping, and screening, including washing where
required, into final products. The processed
aggregates can be combined with cementitious
materials in the manufacturing of concrete or bitumen
as a binder in the production of asphalt.

Concrete aggregates

Concrete aggregates are an integral component of
producing quality concrete. These aggregates and
subsequent concrete supply support our community in
meeting its requirements of roads, housing,
commercial and infrastructure needs.

Asphalt aggregates

The production of high quality asphalt aggregates is a
critical component in the production of quality asphailt.
Holcim quarrying operations supports its customers in
producing quality aggregates throughout each region.

Roadbase materials

Are an integral part of the construction of road
projects including, major infrastructure, road
duplications, residential sub-divisions, commercial
developments and local councils/shires.

Armour rock

Weatherproofing and natural barriers need to be
created to prevent coastal and river erosion. Armour
rock is produced with specific objectives outlined in
each specification. The product typically ranges in
size from 200mm-1.0m dependent on each
specification.

Rail ballast

Holcim is a leading supplier of rail ballasts in
Australia, working closely with customers,
consultants and specifies to best suit their needs.
Rail ballast is a specifically engineered product
designed to support railway sleepers underneath a
rail line. The product is produced to a high
performance specification.

ViroDecs'" Aggregates EPD | Holcim

7

n
fa
(s)
_
G
©
Le
©
rm
ré
œ
ü
D
2
D
D
<

Strategy 2025 - “Accelerating Green Growth”

si

£0ù
ND

Accelerating Expanding
SOLUTIONS &
Shi PRODUCTS

To Become the Global Leader in
Innovative & Sustainable Building
Solutions

Sustainability is not new to Holcim. For decades,
Holcim has embedded the triple bottom line approach
to sustainability with a focus on responsible utilisation
of our planet's natural resources, safety and
environmental performance, and social.

Globally Holcim, is reinventing how the world builds
for people and the planet. On our way to becoming a
net zero company, We are accelerating green
construction by joining the net zero pledge with
science-based targets.

With “Strategy 2025 — Accelerating Green Growth,”

Holcim will become the global leader in innovative and

sustainable building solutions.

With “Accelerating Green Growth,” Holcim will achieve

growth across all our businesses, fueled by
sustainability and innovation. We will accelerate the
expansion of our Solutions & Products business to
reach 30% of Group sales.

(7$

Leading in
INNOVATION &
SUSTAINABILITY

Delivering
SUPERIOR
PERFORMANCE

Sustainability is at the core of our global strategy, with
our industry's first 2050 net-zero targets, endorsed by
the Science Based Targets initiative (SBTi). Holcim
will remain at the forefront of green building solutions,
with at least 25% of ready-mix net sales coming from
ECOPact, ranging from 30% to 100% lower CO;
footprint.

Holcim is part of a global response to these
challenges through sustainable products and
solutions, supported by four fields of action — climate,
circular economy, water, and nature — in order to
improve quality of life for communities and employees.

ViroDecs'" Aggregates EPD | Holcim

8

En)
x
=

œ
=

ü
+

ü

5
2]
où
£
©

(Q]
pe

Supporting sustainable construction

Supporting sustainable construction

The Holcim Foundation for Sustainable Construction
was created in 2003 to raise awareness of the
important role that architecture, engineering, urban
planning and the building industry have in achieving a
more sustainable future. It is the mission of the
Foundation to select and support initiatives that
combine sustainable construction solutions with
architectural excellence and enhanced quality of life
beyond technical solutions.

Through the non-commercial promotion and
development of sustainable construction at national,
regional, and global levels, the Holcim Foundation
encourages sustainable responses to the
technological, environmental, socioeconomic, and
cultural issues affecting building and construction.
The Foundation is an independent legal entity that is
supported by Holcim.

Holcim Forum

The Holcim Forum is a tri-annual series of
conferences on the topic of sustainable construction
conducted by the Foundation. The multi-day Forum,
including workshops and site visits, is an academic
platform for architects, engineers, construction
professionals and specialists of all generations to
exchange information on creating a sustainable built
environment and thus advancing sustainable
development.

The Forum supports sustainable construction in the
scientific field, among experts in the construction
sector, business and society, and promotes
interdisciplinary dialogue, brings forward new ideas,
and examines potential solutions.

Holcim Awards for Sustainable
Construction

The Flagship of the Foundation is the Holcim Awards
for Sustainable Construction. It is a significant
worldwide competition for sustainable design. It
rewards projects and visionary concepts that go
beyond balancing environmental performance, social
responsibility, and economic growth, thereby
exemplifying architectural excellence and a high
degree of transferability.

A total of USD 1 million in prize money is awarded
and projects and visionary concepts in the fields of
architecture, engineering, urban planning, material
and construction technology and related fields are
eligible for entry.

ViroDecs'" Aggregates EPD | Holcim

9

En)
=
©

œ
=

œ
+

o

5
(2)
où
£
©

O
ue

How the EPD can be used in the
IS and Green Star rating schemes

The Infrastructure Sustainability (IS) and Green Star rating schemes are the most commonly applied
sustainability rating schemes for infrastructure and property assets in Australia, respectively. Both schemes are
run by industry bodies the Infrastructure Sustainability Council and the Green Building Council of Australia with
strong support from the built environment sector, government and academia.

Rating schemes

TheIS rating scheme

TheIS rating scheme scores infrastructure assets on a broad range of sustainability areas, from
greenhouse gas (GHG) emissions to community health and well-being, for each major project stage. Holcim's
ViroDecs'" may help IS registered projects gain points in four key credits:

- - IS rating - IS rating -
Credit topic Purpose
vi.1 and 1.2 ZA

Material environmental impacts Mat-1 Rso-6 LIGA EEE nets
p environmental impacts associated with materials

: To reward the use of materials with

Environmental labels Mat-2 Rso-7 environmental labels

Innovation — improving on To reward pioneering initiatives in sustainable

Inn-1 Inn-1

credit benchmarks design, process or advocacy
Innovation — market Inn-1 Inn-1 To reward pioneering initiatives in sustainable
transformation design, process or advocacy

Green Star

The Green Star rating scheme provides a framework for understanding and | communicating the sustainability
performance of a property, master plan or building re-fit. Holcim's ViroDecs" may help Green Star registered
projects gain points in three key credits:

Green Star - Green Star _

To reward the reduction of life cycle

Life Cycle Assessment environmental impact

To reward the use of products with

Environmental labels 21C 21 environmental labels

Innovation challenge:
sustainable sourcing of 19B.1 =
concrete aggregates

To reward the sustainable sourcing of concrete
aggregates

ViroDecs " Aggregates EPD | Holcim 10
Holcim’'s management systems

Safety, Health & Environment Management System

Introduction to the SHEMS

Risk Management Safety Specific

Accountability
Planning & People

Holcim Australia is committed to providing positive
contributions to the community, the environment,
and our business by continuously improving
environmental performance and focusing on
sustainable development.

Holcim's Safety, Health and Environment
Management System (SHEM) has been developed
in alignment with the fundamental management
principles as set out in the following International
Standards:

e ASINZS 4801: Occupational Health and
Safety Management Systems - Specification
with guidance for use

e ASINZS 4804: Occupational Health and
Safety Management Systems - General
Guidelines on principles, systems and
supporting techniques

e ASINZS ISO 14001: Environmental
Management Systems - Requirements with
guidance for use*

e ASINZS ISO 14004: Environmental
Management Systems - General Guidelines
on principles, systems and support
techniques.

e ASINZS 1S0O 31000: Risk management —
Principles and guidelines*

Environment
Specific

Health Specific Review & Improve

Holcim's SHEM is used to support sites and areas
across Holcim Australia and New Zealand to
implement, maintain and continually improve an
effective Safety, Health and Environment program.
The SHEM is an interrelated collection of policies,
processes, programs, procedures, accountabilities
and activities designed to provide the foundation for
successful safety, health and environment
management. Holcim sets corporate objectives and
targets and undertake regular audits of
environmental performance to monitor progress.

*Note: Holcim's Safety, Health and Environment Management System (SHEM) is not certified to ISO 14001 or ISO 31000 etc.

ViroDecs " Aggregates EPD | Holcim 11

er)
=
©
£
a
>”
A
=
=
©
=
©
D
œ
=
G
=

LCA information

Declared unit Allocation

on
o
>
œ
=
<
2
©
>
©
£
=

1 tonne of aggregate. Allocation was necessary to proportion inputs and
outputs to intermediate flows at the quarry level.
As much as possible, intermediate flows were

Reference service life (RSL) allocated physically based on weight. At the quarry
level, whenever physical allocation was not possible,

The RSL is not specified as the scope is from cradle economic allocation was carried out based on

to gate, and there is a variety of applications of Holcim's internal cost system.

aggregates with different anticipated RSLSs.
Regarding inputs, it was assumed that fly ash is a
waste product and therefore burden-free. Please refer

Time representativeness to the “Recycled Material” section for further detail.
The primary data for the LCA is based on 2019 |
calendar year production data. Product grouping
A total of 762 products were modelled and grouped
Databases and LCA software used according to Holcim's product classification system. …A
representative product was selected from each
SimaPro (v9.1.1.1) was used for the LCA modelling, product group to represent the group in the LCA
using background data from: results section.
1. The Australian National Life Cycle Inventory
Database (AusLCI) (2019); and The representative product was selected through the
2. ecoinvent 3.6 (2019). following process:
1. Calculate the median global warming potential
The following impact categories were calculated (GWP) value for each product group.
manually for the foreground data: 2. Identify the product/s with the median GWP
e Use of renewable primary energy resources value.
used as raw materials. 3. lfthe median GWP value corresponds to only
e Use of non-renewable primary energy one product, that product is selected as the
excluding non-renewable primary representative product and the process ends.
energy resources used as raw materials. 4. lfthe median GWP value corresponds to
° Use of secondary material. multiple products, the product with the highest
° Use of renewable secondary fuels. value in one or more of the other impact

categories was selected and the process
ends.

5. lfthe median does not correlate to a specific
product (due to an even dataset) then the
product with the next GWP value higher than
the median was selected.

e Use of non-renewable secondary fuels.

Cut-off criteria

No flows were excluded on the basis of cut-off criteria.

ViroDecs " Aggregates EPD | Holcim 12
Data quality

Data quality for the foreground data was assessed in terms of geographic and temporal representativeness.
All data sources were scored at medium or higher. Background data sources were also assessed with respect
to their timeliness, with all data sources being last updated within the 10 years required under the PCR

2012:01.

AT
Fine aggregate
Coarse
Aggregate
Cement
Cement Flyash
Blend
Precoat oil

Internal
transport

Transport of
precoat oil

Transport of
cementitious
materials

Transport of
explosives

Aggregate
production
plant

Electricity

Diesel
Petrol

Pollutants

Explosives (gravel
only)

Modelled data used
— selected
representative
product for results of
this LCA sudy

Background data
used to model

Diesel

Background data
used to model

Background data
used to model

Electricity

Diesel
Petrol
Mains water

Water — other
sources (lakes,
groundwater,
rainwater)

Water discharge
from site

Solid waste

Electricity provider
invoices

Supplier invoices

National Pollution
Inventory (NPI) data

Invoices

Holcim Breakdown of
Materials (BOM)
inventory used for QTY
of material blended with
aggregates.

Holcim Breakdown of
Materials (BOM)
inventory used for QTY
of material blended with
aggregates

Diesel burned by site
vehicles for internal
transport within the

aggregate site is
included in the site
resource use data based
on supplier invoices

Background data
includes ‘transport to
customer’

Conservative
assumptions on distance
and transport mode as
provided by Holcim
technical team

Electricity provider
invoices

Supplier invoices

Water utility invoices

Estimate based on water
balance

Estimate based on
Holcim site performance
metrics

Waste data reports
based on waste service
provider invoices

2019 All states High
2019 All states High
2019 All states High
All states (excluding
the Kalgoorlie
Quarry in WA which ;
arS purchases raw feed QEL
from an external
source)
2019 All states High
2019 All states High
2019 All states High
2019 All states Medium
2019 All states Medium
2019 All states High
2019 All states High
2019 All states High
2019 All states Medium
2019 All states Medium
2019 All states High

ViroDecs " Aggregates EPD | Holcim 13

on
o
>
œ
=
<
2
©
>
©
£
=

Assumptions and Limitations

The key assumptions and limitations of the study are summarised in the table below.

Impact on LCA

Assumption or limitation
results

Cost of production data was assessed to be the most accurate proxy for
the physical relationships underlying the processes. Cost of production

Use of internal cost of data is linked to Holcim's cost of production data and is therefore unlikely
production data to allocate Medium to have significant errors. Outliers in the results were investigated and
energy inputs determined to be justified based on real differences between sites, such

as the different degrees of rock blasting and quarrying activity at each

Transport distances
assumed or generic for all
raw materials barring quarry
materials

Low

System diagram

site.

Conservative assumptions regarding transport distance were made

based on country of origin and transport mode information.

The processes included in the LCA are presented in a process diagram in the figure below.

Raw material extraction

Cement plant

On-site
transport

Processing
and
blending

Quarrying

On-site
transport

Processing
and
blending

ViroDecs " Aggregates EPD | Holcim

14

on
o
>
œ
=
<
2
©
>
©
£
=

Description of system boundaries and excluded lifecycle stages

The scope of the LCA and EPD is from crade to gate. Life cycle stages beyond Holcim's gate are excluded
from the LCA (see figure below).

on
o
>
œ
=
<
2
©
>
©
£
=

Environmental impacts relating to personnel, infrastructure and production equipment not directly consumed in
the process are excluded from the system boundary as per the Product Category Rules (2012:01 Construction
products and construction services).

Benefits &

Construction Use Stage End of Life Stage loads for the

Product Stage

Stage next product

system

u
u
= =
> = Q E Q a a = =
S S Œ © a L D 3 e D &
œ > = G es G c > = E = = En
3 © © = 2 Ë È [e)] © D = me o
(9) € E € = — = + . = = TD e O a M —
— © 5 e] œ — œ Ts D 2 Q ES © D El ©
G Q 2 Q = œ D = O e = Z Q @ es
Sn ra) œ ra) S D £ = £E £ CR = D E = 2 5
— —

LS SN CN MEN ON MOMENT ME Eu MON LE Ne 88
> FF  & # = S = Ê E ELLE E) F 7 C D +
= = © e S ] S & œ à d il œ
ü © 2 © e = G a] C œ d
œ D = œ = Le es © S Ca

E à D 5 O  ? œ

D I © 5 © & si]

= (4 D 8 œ

O
AT A2 A3 A4 A5 B1 B2 B3 B4 B5 B6 B7 C1 C2 CS C4 D
X X X ND ND ND ND ND ND ND ND ND ND ND ND ND ND

* Not declared (ND)

ViroDecs " Aggregates EPD | Holcim 15
EPD product description

This EPD covers Holcim's range of aggregates sold in Australia. The following table outlines the

product groups covered in this EPD.

Aggregate
type

Cement
treated

Product Group

Natural Sand

Manufactured
Sand

Drainage Filter

Dust

Customer Spec.
Roadbase

Other Roadbase

Recycled
Products

Ballast

Concrete
Aggregates

Asphalt
Aggregates

Sealing
Aggregates

Other Aggregates

Precoat
Aggregates

Cement-treated
Products

Component Products

Fine sand
Mortar sand
Coarse sand
Fill sand

Manufactured sand

Drainage filter

Dust

Asphalt dust

NSW Roads and Maritime Services (RMS) Densely Graded Base (DGB)
QLD Transport and Main Roads (TMR) Unbound Pavement (UBP)
VicRoads specified aggregate product

WA Main Roads Department (MRD) specified aggregate product
SA Department for Infrastructure and Transport specified aggregate
product

Base material

Crusher run

Scalps

Processed fill

Subbase material

Recycled fill

Recycled concrete

Ballast

Concrete aggregate 5mm
Concrete aggregate 7 mm
Concrete aggregate 10 mm
Concrete aggregate 14mm
Concrete aggregate 20mm
Concrete aggregate other

Asphalt aggregate 5mm
Asphalt aggregate 7 mm
Asphalt aggregate 10 mm
Asphalt aggregate 14mm
Asphalt aggregate other
Sealing aggregate 7 mm
Sealing aggregate 10 mm
Sealing aggregate 14mm
Sealing aggregate other
Armour rock

Decorative rock

Round pebbles
Overburden

Shot rock

Size graded rock

Spalls

Precoat aggregate 5mm
Precoat aggregate 7 mm
Precoat aggregate 10 mm
Precoat aggregate 14mm
Precoat aggregate other
Cement-treated roadbase
Cement-treated dust

ViroDecs " Aggregates EPD | Holcim

[=
S
£

©.
"EC

O

(A

©
T
e

e

_
T

[e)

Le
CE

16
Content declaration

The following table provides a summary of the materials included in Holcim's aggregate
products groups and their relative composition by weight.

[=
(e]
=
©.
=
©
7]
cQ
L°)
—
©
=]
T
[e)
=
©

Aggregate 94%-100%
Cementitious material 0-6%
Pre-coat oil 0-2%
Packaging Default background data from LCA databases was

used to model fly ash. The AusLCI process for fly ash
treats it as a waste material and only includes

Holcim aggregate is delivered in bulk with no -
transport impacts.

packaging.

The allocation approach of the AusLCI LCA database
was adopted as a default for secondary data and
processes (e.g. secondary fuel in cement production).
The AusLCI dataset conforms to EN 15804 when

Recycled material

BS EN 16757:2017 specifically lists the following applying allocation to its various processes and sub-
materials relevant to the study as co-products: processes.
e Fly ash;

As such, the above materials are considered as co-
products of their production process and the impacts
for their production process are allocated according to
PCR 2012:01 Construction Products and Construction
Services (co-produced goods, multi-output allocation).

ViroDecs " Aggregates EPD | Holcim 17
Environmental performance

The environmental impacts considered in this EPD are listed in the table below. AIl further
tables from this point will contain the abbreviation only.

Impact Category Abbreviation Measurement Unit

Global warming potential WP kg CO equivalents (GWP100)
Ozone depletion potential ODP kg CEC 11 equivalents
Acidification potential AP kg SO2 equivalents
Eutrophication Potential EP kg PO4S- equivalents
Photochemical ozone creation potential POCP kg C2H2 equivalents
Abiotic depletion potential (elements) ADPE kg Sb equivalents
Abiotic depletion potential (fossil fuels) ADPF MJ net calorific value

Use of renewable primary energy excluding renewable primary energy

. PERE M9, net calorific value
resources used as raw materials
Use of renewable primary energy r r raw material ”
p y gyresources usedas)ra alerlars PERM MJ, net calorific value
Total use of renewable primary energy r rl rimary ener n ee
| p ÿ gy esources Guen EU PERT MJ, net calorific value
primary energy resources used as raw materials)
Use of non-renewable primary ener xcluding non-renewable prim u
p ÿ ergy € een neneneselR names PENRE MJ, net calorific value
energy resources used as raw materials
f non- renewable primar i e
Use of non- renewable primary energy resources used as raw materials PENRM dE mi eite ve lue

Total use of non- renewable primary energy resources (primary energy

and primary energy resources used as raw materials) PENRT M9, net calorific value
Use of secondary material SM kg
Use of renewable secondary fuels RSF M9, net calorific value
Use of non-renewable secondary fuels NRSF M9, net calorific value
Use of net fresh water FW m3
RTE
Hazardous waste disposed HWD kg
Non-hazardous waste disposed NHWD kg
Radioactive waste disposed/stored RWD kg
Components for reuse CRU kg
Materials for recycling MER kg
Materials for energy recovery MER kg
Exported energy EE MJ per energy carrier

A representative product was selected from each product group to represent the group in the environmental impact
results. The criteria for selection are outlined in the LCA information section. Variability for results within the product
groups was greater than + 10%.

ViroDecs " Aggregates EPD | Holcim 18

@
(=)
=
œ
=
©
€
©
©
œ
fe
=
©
=
=
[e]
=
>
€
LU

Australia Wide

Holcim ViroDecs'" Aggregates - Fine (1 tonne) $
8
GWP kg CO, eq. 6.52 3.10 6.01 5.98

ODP kg CFC 11 eq. 6.51E-08 3.59E-10 2.29E-08 4.15E-08

AP kg SO, eq. 4.46E-02 1.86E-02 3.22E-02 2.87E-02

EP kg PO. eq. 1.23E-02 4.83E-03 8.67E-03 7.60E-03

POCP kg C,H, eq. 1.38E-03 3.64E-04 7.74E-04 7.62E-04

ADPE kg Sb eq. 6.19E-06 8.31E-08 2.46E-06 3.12E-06

ADPF MJ 7.77E+01 4.58E+01 7.56E+01 6.48E+01

Resource Use

PERE MINCV 2.47E+00 2.65E-02 1.92E+00 1.42E+00
PERM MINCV 0.00E +00 0.00E+00 0.00E+00 0.00E+00
PERT MINCV 2.47E+00 2.65E-02 1.92E+00 1.42E+00
PENRE MINCV 7.78E+01 4.58E+01 7.56E+01 6.48E+01
PENRM MINCV 0.00E +00 0.00E+00 0.00E+00 0.00E+00
PENRT MINCV 7.78E+01 4.58E+01 7.56E+01 6.48E+01
SM Le] 0.00E +00 0.00E+00 0.00E+00 7.4T7E-01
RSF MINCV 0.00E +00 0.00E+00 0.00E+00 0.00E+00
NRSF MINCV 0.00E +00 0.00E+00 0.00E+00 0.00E+00
FW m° 3.46E-02 4.38E-04 8.61E-03 1.01E-02

Output categories

HWD Le] 4.68E-04 3.09E-07 1.36E-04 1.69E-04
NHWD Le] 3.55E-01 4.26E-03 2.82E-01 2.17E-01
RWD Le] 3.83E-07 3.45E-09 1.28E-07 1.62E-07
CRU Le] 0.00E +00 0.00E +00 0.00E+00 0.00E+00
MER kg 0.00E+00 0.00E+00 0.00E+00 0.00E+00
MER kg 0.00E+00 0.00E+00 0.00E+00 0.00E+00
EE MJ 0.00E+00 0.00E+00 0.00E +00 0.00E+00

ViroDecs " Aggregates EPD | Holcim 19
Holcim ViroDecs'" Aggregates - Course (1 tonne)

8

Impact Ballast Other Asphalt Sealing Concrete Precoat Other Spec. £

Category Aggregates Aggregates Aggregates Aggregates Aggregates Roadbase Roadbase cs

Potential Environmental Impacts BR 3

GWP kg CO, eq. 7.81 6.12 9.24 8.16 7.98 31.71 6.17 3.26 a

ODP kg CFC 11 eq. 3.97E-08 2.62E-08 3.94E-08 1.67E-08 2.51E-08 4.15E-08 2.38E-08 6.26E-09 8
AP kg SO, eq. 2.22E-02 2.82E-02 3.85E-02 4.86E-02 4.21E-02 1.52E-01 2.66E-02 2.65E-02
EP kg PO* eq. 6.29E-03 7.59E-03 1.05E-02 1.28E-02 1.13E-02 1.74E-02 7.25E-03 6.97E-03
POCP kg C,H, eq. 7.16E-04 7.11E-04 9.78E-04 1.08E-03 9.16E-04 6.64E-03 6.58E-04 5.48E-04
ADPE kg Sb eq. 4.11E-06 2.44E-06 4.17E-06 1.89E-06 2.76E-06 6.51E-06 2.63E-06 7.10E-07
ADPE MJ 9.78E+01 8.51E+01 1.13E+02 1.17E+02 1.05E+02 2.78E+03 7.75E+01 4.46E+01
PÈRE MINCV 2.47E+00 6.97E-01 2.23E+00 9.23E-01 1.45E+00 1.04E+00 1.96E+00 5.14E-01
PERM MINCV 0.00E+00 0.00E+00 0.00E+00 0.00E+00 0.00E+00 1.76E+00 0.00E+00 0.00E+00
PERT MINCV 2.47E+00 6.97E-01 2.23E+00 9.23E-01 1.45E+00 2.81E+00 1.96E+00 5.14E-01
PENRE MINCV 9.78E+01 8.51E+01 1.13E+02 1.17E+02 1.05E+02 5.46E+01 7.75E+01 4.46E+01
PENRM MINCV 0.00E+00 0.00E+00 0.00E+00 0.00E+00 0.00E+00 2.73E+03 0.00E+00 0.00E+00
PENRT MINCV 9.78E+01 8.51E+01 1.13E+02 1.17E+02 1.05E+02 2.78E+03 7.75E+01 4.46E+01
SM kg 0.00E+00 0.00E+00 0.00E+00 0.00E+00 0.00E+00 9.51E-05 0.00E+00 0.00E+00
RSF MINCV 0.00E+00 0.00E+00 0.00E+00 0.00E+00 0.00E+00 0.00E+00 0.00E+00 0.00E+00
NRSF MINCV 0.00E+00 0.00E+00 0.00E+00 0.00E+00 0.00E+00 0.00E+00 0.00E+00 0.00E+00
1.27E-02 6.12E-03 2.02E-02 8.27E-03 3.43E-02 1.02E-01 9.00E-03 2.57E-03

EE

2.67E-04 1.91E-04 2.10E-04 1.15E-04 1.52E-04 1.36E-04 1.51E-04 3.79E-05
NHWD Le] 3.60E-01 9.90E-02 4.55E-01 7.45E-02 2.57E-01 4.62E-01 2.87E-01 7.62E-02
RWD Le] 2.33E-07 1.56E-07 8.10E-07 1.06E-07 1.41E-07 3.41E-07 1.39E-07 3.69E-08
CRU Le] 0.00E+00 0.00E+00 0.00E+00 0.00E+00 0.00E+00 0.00E+00 0.00E+00 0.00E+00
MER Le] 0.00E+00 0.00E+00 0.00E+00 0.00E+00 0.00E+00 0.00E+00 0.00E+00 0.00E+00
MER kg 0.00E+00 0.00E+00 0.00E+00 0.00E+00 0.00E+00 0.00E+00 0.00E+00 0.00E+00
EE MJ 0.00E+00 0.00E+00 0.00E+00 0.00E+00 0.00E+00 0.00E+00 0.00E+00 0.00E+00

ViroDecs " Aggregates EPD | Holcim 20
Holcim ViroDecs'" Aggregates - Cement Treated (1 tonne)

rl

2

œ

D

Cement- £

0.5% Cement- 1% 1.5% 2% 2.5% treated 3% 3.5% 4% 5% 6% Ex

Impact Cement- treated Cement- Cement- Cement- Cement- Creternen Cement- Cement- Cement- Cement- Cement- Cement- «

Category treated Other treated treated treated treated AT treated treated treated treated Dust treated treated Fe

Roadbase | Roadbase | Roadbase | Roadbase | Roadbase | Roadbase Ro bise Roadbase | Roadbase | Roadbase Roadbase | Roadbase 7

©

€

GWP kg CO, eq. 7.77 8.12 10.11 12.51 13.67 14.74 14.74 17.52 19.21 22.21 21.16 24.34 33.88 Ê

ODP kg CFC 11 6.01E-08 3.88E-08 8.60E-08 1.13E-07 1.21E-07 1.31E-07 1.31E-07 1.30E-07 1.81E-07 1.68E-07 1.69E-07 2.25E-07 2.71E-07 ô
AP kg SO, eq. 2.52E-02 4.89E-02 3.06E-02 3.55E-02 3.78E-02 4.00E-02 4.00E-02 4.58E-02 4.90E-02 5.53E-02 4.98E-02 5.93E-02 7.84E-02
EP kg PO,” eq. 6.40E-03 1.23E-02 7.64E-03 8.69E-03 9.19E-03 9.66E-03 9.66E-03 1.08E-02 1.16E-02 1.28E-02 1.15E-02 1.38E-02 1.80E-02
POCP kg C,H, eq. 6.98E-04 1.01E-03 8.53E-04 9.90E-04 1.05E-03 1.11E-03 1.11E-03 1.24E-03 1.37E-03 1.49E-03 1.36E-03 1.64E-03 2.10E-03
ADPE kg Sb eq. 3.61E-06 1.86E-06 4.69E-06 5.75E-06 6.15E-06 6.59E-06 6.59E-06 7.61E-06 8.57E-06 9.35E-06 8.59E-06 1.05E-05 1.33E-05
ADPF MJ 7.06E+01 7.80E+01 8.69E+01 1.02E+02 1.08E+02 1.15E+02 1.15E+02 1.28E+02 1.43E+02 1.56E+02 1.40E+02 1.73E+02 2.26E+02
PERE MINCV 1.49E+00 5.20E-01 1.77E+00 2.01E+00 2.12E+00 2.23E+00 2.23E+00 4.78E+00 2.67E+00 5.22E+00 2.67E+00 3.17E+00 4.10E+00
PERM MINCV 0.00E+00 0.00E+00 0.00E+00 0.00E+00 0.00E+00 0.00E+00 0.00E+00 0.00E+00 0.00E+00 0.00E+00 0.00E+00 0.00E+00 0.00E+00
PERT MINCV 1.49E+00 5.20E-01 1.77E+00 2.01E+00 2.12E+00 2.23E+00 2.23E+00 4.78E+00 2.67E+00 5.22E+00 2.67E+00 3.17E+00 4.10E+00
PENRE MINCV 7.06E+01 7.80E+01 8.69E+01 1.02E+02 1.08E+02 1.15E+02 1.15E+02 1.28E+02 1.43E+02 1.56E+02 1.40E+02 1.73E+02 2.26E+02
PENRM MINCV 0.00E+00 0.00E+00 0.00E+00 0.00E+00 0.00E+00 0.00E+00 0.00E+00 0.00E+00 0.00E+00 0.00E+00 0.00E+00 0.00E+00 0.00E+00
PENRT MINCV 7.06E+01 7.80E+01 8.69E+01 1.02E+02 1.08E+02 1.15E+02 1.15E+02 1.28E+02 1.43E+02 1.56E+02 1.40E+02 1.73E+02 2.26E+02
SM kg 0.00E+00 0.00E+00 1.50E+00 3.00E+00 2.75E+00 3.13E+00 3.13E+00 0.00E+00 6.00E+00 0.00E+00 0.00E+00 6.50E+00 0.00E+00
RSF MINCV 0.00E+00 0.00E+00 0.00E+00 0.00E+00 0.00E+00 0.00E+00 0.00E+00 0.00E+00 0.00E+00 0.00E+00 0.00E+00 0.00E+00 0.00E+00
NRSF MINCV 0.00E+00 0.00E+00 0.00E+00 0.00E+00 0.00E+00 0.00E+00 0.00E+00 0.00E+00 0.00E+00 0.00E+00 0.00E+00 0.00E+00 0.00E+00

3.70E-02 7.48E-03 4.24E-02 4.59E-02 4.75E-02 4.90E-02 4.90E-02 3.15E-02 5.57E-02 3.83E-02 3.26E-02 6.27E-02 7.51E-02

nee RS PS PS PS PE PS PE

1.43E-04 9.85E-06 1.57E-04 1.62E-04 1.64E-04 1.66E-04 1.66E-04 1.19E-04 1.75E-04 1.27E-04 1.46E-04 1.83E-04 1.97E-04

NHWD kg 1.84E-01 9.84E-02 2.39E-01 2.92E-01 3.12E-01 3.34E-01 3.34E-01 3.52E-01 4.33E-01 4.41E-01 4.76E-01 5.33E-01 6.80E-01
RWD Kg 1.68E-07 5.81E-08 2.05E-07 2.36E-07 2.48E-07 2.61E-07 2.61E-07 5.15E-07 3.19E-07 5.65E-07 3.53E-07 3.78E-07 4.67E-07
CRU kg 0.00E+00 0.00E+00 0.00E+00 0.00E+00 0.00E+00 0.00E+00 0.00E+00 0.00E+00 0.00E+00 0.00E+00 0.00E+00 0.00E+00 0.00E+00
MER Le] 0.00E+00 0.00E+00 0.00E+00 0.00E+00 0.00E+00 0.00E+00 0.00E+00 0.00E+00 0.00E+00 0.00E+00 0.00E+00 0.00E+00 0.00E+00
MER Le] 0.00E+00 0.00E+00 0.00E+00 0.00E+00 0.00E+00 0.00E+00 0.00E+00 0.00E+00 0.00E+00 0.00E+00 0.00E+00 0.00E+00 0.00E+00

EE MJ 0.00E+00 0.00E+00 0.00E+00 0.00E+00 0.00E+00 0.00E+00 0.00E+00 0.00E+00 0.00E+00 0.00E+00 0.00E+00 0.00E+00 0.00E+00

ViroDecs " Aggregates EPD | Holcim 21
Interpretation

Holcim ViroDecs'" Aggregates

Care should be taken when comparing EPDs. The EPD of construction products may not be comparable if they
do not comply with the requirements of comparability set in EN 15804. EPDs within the same product category
but from different programmes may not be comparable.

Holcim's aggregates have a range of greenhouse gas (GHG) emissions, across the different product groups
covered by the EPD. The following section presents the GHG emissions associated with 1 tonne of Holcim
aggregates in Australia. To evaluate the performance of Holcim's ViroDecsTM Aggregates range, the EPD results
can be benchmarked against the IS materials calculator default base case aggregates and the Australian National
Life Cycle Inventory Database (AusLCI). Benchmarking in Green Star can be done as per the guidance for credit
19B.1 (Life Cycle Impacts).

The global warming potential data produced by the study indicate varying degrees of impact across the 24
product groups modelled in this LCA study. Medium sized coarse aggregates such as ballast, other aggregates
and asphalt aggregates had the lowest median global warming potential impacts per tonne of aggregate (as
determined by the ‘representative product’ selected for each product group per the process outlined earlier in this
EPD). This is likely due to the reduced processing requirements for these products. The cementitious products
had a significantly higher impact (even at 0.5% cement content). Graphs of the cradle to gate global warming
potential results for the representative product of each product group are presented in figures below.

7.0
5.98
6.0
5.0
4.0

3.0

2.0

Greenhouse gas emissions (kg CO.-e / tonne aggregate)

1.0

0.0
Drainage Filter Natural Sand Manufactured Sand Dust

Holcim ViroDecs'" Aggregates - Fine - Cradle to gate global warming potential (kg CO-e / per tonne)

ViroDecs " Aggregates EPD | Holcim 22

=
(°]
=
©
&
©
=
Q
=
©
o
=

35.0

31.71

uone)91d19ju]

a
S
m

Customer

Other
Roadbase

6.17
E .

Precoat
Aggregates

7.98

Concrete
Aggregates

8.16
Sealing
Aggregates

9.24
Asphalt

Aggregates

6.12
Other

Aggregates

7.81
Ballast

Holcim ViroDecs'" Aggregates — Coarse - Cradle to gate global warming potential (kg CO-e / per tonne)

a o a o a a
LOQ [e] LQ [®] LO [e]
[NI NN El i

(ex6a166e auuo] / 28-709 6x) suoissiuse se esnouuse1o

Spec.
Roadbase

33.88

aseqpeoy palea1]-JU2LU8D 9

aseqpeoy pareal-JUOUU2D 96G

24.34

1snq perau-Juauua

21.16

22.21

aseqpeoy pareal-JUOUUSD

aseqpeoy parea1]-JUOU8D 9SG'E

19.21

aseqpeoy pareal-JUOU2D €

17.52

eseqpeoy ‘2edS 18L0]SN9 p212211-JU8I99

aseqpeoy pareal-lUOU8D SZ

14.74

14.74

aseqpeoy pareal-JUOUUSD 2

aseqpeoy parea1-JUOUU8D GT

12.51

13.67

aseqpeoy palea1}-JUELUED TI

10.11

eseqpeoy 19UJO Palea1j-IUSLUSD

8.12

FF
R eseqpeox pa]ea1]-JUSU9) %G'0
FF

Q Q Q Q Q Q Q Q

LO [e] LO [e] LQ [e] LO [e}

om om [IN NN Lau) Lau)

(exe6a166e euuo] / 3-09 6x) suoissiuse se ssnoyuss1s

Holcim ViroDecs'" Aggregates - Cement Treated - Cradle to gate global warming potential (kg CO-e / per tonne)

23

ViroDecs " Aggregates EPD | Holcim
References

Australasian EPD Programme. (2017). Guidance
on the use of INA in EPDs.

Australasian EPD Programme. (2018). Guidance
on the use of background LCI data.

Australasian EPD Programme. (2018). Instructions
of the Australasian EPD Programme V3.0.

Australian Life Cycle Inventory Database Initiative
(AuSLCI). (2015). Guidelines for Data Development for
an Australian Life Cycle Inventory Database, Data
Standard.

British Standards Institution. (2014). Sustainability of
construction works. Environmental product
declarations. Core rules for the product category of
construction products, BS EN 15804:2012+A1:2013.
British Standards Institution.

British Standards Institution. (2017). Sustainability of
construction works — Environmental product
declarations

— Product Category Rules for concrete and concrete
elements, BS EN 16757:2017. British Standards
Institution.

Ecoinvent Centre. (2019). ecoinvent version 3
database. Zurich: ETH, Agroscope, EMPA, EPFL,
PSI. Retrieved from www.ecoinvent.org

EPD International. (2017). General Programme
Instructions (GP) for the International EPD System
V3.0. Retrieved from www.environdec.com

References

EPD International. (2018). Product Category
Rules for Construction Products and
Construction Services, PCR2012:01 v2.3.
Stockholm: EPD International.

ISO. (2006). Environmental labels and declarations

-- Type Ill environmental declarations -- Principles
and procedures, ISO 14025:2006. Geneva:
International Organization for Standardization.

ISO. (2006). Environmental management -- Life cycle
assessment -- Principles and framework, ISO
14040:2006. Geneva: International Organization for
Standardization.

ISO. (2018). Environmental management. Life cycle
assessment. Requirements and guidelines, ISO
14044:2006+A1:2018. Geneva: International
Organization for Standardization.

AusLCI (2019). AusLCI Database. Retrieved from
AUSLCI: www.auslci.com.au/

ViroDecs " Aggregates EPD | Holcim 24
Programme-related information and verification

Holcim

sms" E PD

Declaration Owner

EPD Programme Operator

EPD Produced by

Product category rules

Product group classification
Geographical Scope

Reference Year for Data

Holcim (Australia) Pty Ltd
Level 7 Tower B,

799 Pacific Highway
Chatswood NSW 2067,
Australia

Web: www.holcim.com.au
Phone: +61 2 9412 6600

EPD Australasia Limited

315a Hardy Street Nelson

7010

New Zealand

Web: www.epd-australasia.com Email:
info@epd-australasia.com Phone: 02
8005 8206

ENVIRONMENTAL PRODUCT DECLARATION

(à EDGE

PCR 2012:01 Construction Products and Construction Services, Version
2.3, 2018-11-15

UN CPC 54

Edge Environment Pty Ltd

Web: www.edgeenvironment.com
Phone: +612 9438 0100

Email: info@edgeenvironment.com

SP-02332

2021-05-18

2.0 Version | Revision date 2023-05-11
2026-05-17

Australia

2019

CEN standard EN 15804:2012+A1:2013 served as the core PCR

Product category rules

PCR review was conducted by

Independent third-party
verification of the declaration
and data, according to ISO
14025:2006:

Third Party Verifier

Procedure for follow-up of
data during EPD validity
involves third party verifier:

PCR 2012:01 Construction Products and Construction Services, Version
2.3, 2018-11-15

The Technical Committee of the International EPD® System. Chair:
Massimo Marino. Contact via info@environdec.com

CO] EPD process certification
X EPD verification

Jane Anderson ConstructionLCA
Limited Approved by: EPD
Australasia

ConstructionLCA

Programme-related information and verification:

The EPD owner has the sole ownership, liability, and responsibility for the EPD. EPDs within the same product
category but from different programmes may not be comparable. EPDSs of construction products may not be
comparable if they do not comply with EN 15804.

ViroDecs " Aggregates EPD | Holcim 25
Holcim

Contact your local customer service team Australia-wide on 1300 555 277

Holcim (Australia) Pty Ltd

Level 7 Tower B, 799 Pacific Highway
Chatswood NSW 2067 Australia

ABN 87 099 732 297

www.holcim.com.au

This publication supersedes all previous literature on this subject. As the specifications
and details contained in this publication may change please check with Holcim Customer
Service for confirmation of current issue. This publication provides general information
only and is no substitute for professional technical engineering advice. Users must make
their own determination as to the suitability of this information or any Holcim product for
their specific circumstances. Holcim accepts no liability for any loss or damage resulting
from any reliance on the information provided in this publication. Holcim is a registered
trademark of Holcim Ltd. “Strength. Performance. Passion.” and “ViroDecs” are
trademarks of Holcim (Australia) Pty Ltd.

© 2023 Holcim (Australia) Pty Ltd ABN 87 099 732 297. All rights reserved. This guide or
any part of it may not be reproduced without prior written consent of Holcim.
