Ÿ ECO PLATFORM ]

| ®
] e AUSTRALASIA
l | O C | m ENVIRONMENTAL PRODUCT DECLARATION EN 15804 VERIFIED

Table of Contents

Introduction ................................................................. eee 3
About Holcim.................................................................. si 4
ViroDecs'" Special — a first for ready-mix concrete in Australia 5
ViroDecs'" Special at a glance................................................................. 5
Ready-mix concrete ..….......................................................... eee 6
LCA Information... iiisiiiiiiieeeeeeeeeeeeeeereeeeeeeeeeeeereeeeeeeeeeneeeenennee 7
EPD Product Description and Use... sise 11
Environmental Performance... sise 13
Other life cycle stages not included in this EPD....................... 16
References... iiisiieeeeeeeeeeeeeeeeeeeeeeeeeeeeeneeeeeeeeeneeeeeennnnee 17
Programme-related information and verification 18

Version Number Version Date Description of Changes

v1.0 N/A N/A

ViroDecs'" EPD | Holcim 2
Introduction

All around the world, the expectation for Governments
and organisations to provide enhanced transparency
and disclosure of environmental impacts, such as
greenhouse gas (GHG) emissions, has been growing.
This follows the landmark COP 21 Paris Agreement in
2015 in which all nations agreed to ambitiously pursue
efforts to combat climate change andits effects.

Atthe same time, the global demand for construction
materials is also growing due to worldwide population
growth and an increase in urbanisation. In fact, concrete
is the second most used commodity in the world behind
water, and typically a major contributor to the embodied
GHG emissions of an infrastructure or property asset.

This clearly demonstrates both the essential need for
construction materials now and in the future, as well as
the necessity for the construction materials industry to
be a leading part of the solution addressing climate
change.

At Holcim, we recognise our responsibility to contribute
to global emissions reduction targets and we have
developed a roadmap with a number of actions to direct
our efforts.

Our ViroDecs " range of ready-mix concrete
represented by an Environmental Product Declaration
(EPD) is one suchinitiative for Holcim in Australia.

ViroDecs'" EPD | Holcim
About Holcim

Western
Australia

ePerth

AUSTRALIAN OPERATIONS

ET Precast pipe and product

*Darwin

Northern ET
Territory
Queensland [3
e Brisbane
South
En Australia
Co. New South jo |
Wales / ACT
Era e Sydney 7:
e Adelaide e Canberra ES
Victoria
* Melbourne EX
Tasmania E
e Hobart [a

“The breakdown of Australian operations is based on 2017 site data used for the EPD Life Cycle
Assessment modelling and includes tolling sites and excludes mobile or temporary sites

About Holcim

Holcim is a leading supplier of construction materials in
Australia, originally serving the industry under the well-
known Readymix and Humes brands dating back to
1901. Today Holcim continues to supply essential
construction materials including aggregates, sand,
ready-mix concrete, engineered precast concrete and
prestressed concrete solutions to a range of customers
and projects throughout Australia.

Holcim operates right across the Australian continent
supplying concrete from a network of concrete plants,
quarries, precast and concrete pipe places, and mobile
and on-site project facilities.

As part of LafargeHolcim, Holcim Australia can be
counted on for state-of-the-art product development,
reliable service, and advanced technical expertise for
your next project.

ViroDecs'" EPD | Holcim

About LafargeHolcim

LafargeHolcim is the global leader in building materials
and solutions and active in four business segments:
Cement, Aggregates, Ready-mix Concrete and
Solutions & Products.

With leading positions in all regions of the world and a
balanced portfolio between developing and mature
markets, LafargeHolcim offers a broad range of high-
quality building materials and solutions.

LafargeHolcim experts solve the challenges that
customers face around the world, whether they are
building individual homes or major infrastructure
projects.

Demand for LafargeHolcim materials and solutions is
driven by global population growth, urbanisation,
improved living standards and sustainable construction.
Around 75,000 people work for the company in around
80 countries.
ViroDecs'" Special — a first for ready-mix

concrete in Australia

The Holcim ViroDecs!" Special provides project-specific,
on-demand Environmental Product Declarations (EPDs) to
Holcim'’s customers. This capability represents a
significant step in Holcim's sustainability journey and
embodies our multi-disciplinary approach to embedding
sustainability into our organisation and operations. With
the introduction of our ViroDecs " Special, third-party
verified data will underpin our capability to work with our
customers from tender through to design and construction
to optimise ready-mix concrete mix designs and report on
sustainability performance.

The publication of the original ViroDecs " EPD in 2019
introduced quality, third-party verified embodied life cycle
impact data for ready-mix concrete into the Australian
market for the first time. Holcim has been pleased by the
positive response from the industry. The message was
loud and clear: “we want transparency and we want a
evidence-based approach to specification, procurement
and reporting”. With the introduction of our ViroDecs "
Special, Holcim's customers can specify concrete
sustainability performance in terms of CO--e, with the
confidence that our claims are backed by our third-party
verified EPD Process Certification.

Holcim ViroDecs'" Special is backed by an EPD
Process Certification. It's not only a first for concrete but
a first for any product in Australia. Our EPD Process
Certification is a stamp of approval to produce compliant
EPDSs in-house, opening up significant capability and
flexibility in producing and using life cycle impact data to
inform our operations and our customers.

To gain our EPD Process Certification, Holcim invested
in embedding Life Cycle Assessment (LCA) into our
systems and processes. We have satisfied a rigorous,
third-party evaluation in accordance with the relevant
ISO standards and guidelines of the International EPD
Programme and EPD Australasia.

This EPD has been developed using our EPD Process
Certification for the project ECOPact Range in Far South
Coast NSW with production occurring at Holcim
Bateman'’s Bay and Holcim Ulladulla.

Ready-mix concrete

Aggregrates
Load and Haul Crushing and Screening Stockpiling and Distribution

Concrete
Batching

Material Handling and Storage
+, Ë

Summary of properties and classes

Concrete is prepared by mixing cement, ° Normal-class — designed for residential
coarse and fine aggregates, and water, with applications, low rise buildings, paving
or without the addition of auxiliary agents and driveways etc. Its specification and
and additives. The fresh concrete is placed ordering have been simplified as far as
on the building site or prefabricated in practicable.

factory moulds, compacted and hardened in + Special-class — allows the purchaser to
the desired shape by the hydration of incorporate into the project specification
cement to form concrete. any special requirements for the project.

Special-class concrete is typically
supplied to major and high-end
construction projects from high rise
buildings, dams and spillways, roads and
bridges to public works infrastructure etc.
Special-class concrete is typically
specified in accordance with the technical
parameters and performance
requirements, which can include high-
strength/high-performances concrete,
high durability or marine application, post-
tensioned, high-pumpability, super
workable, piling concrete, architectural
off-form finishes and other decorative
applications.

General Australian Standard AS 1379 sets
down a number of different ways of
specifying and ordering concrete to
promote uniformity, efficiency and economy
in production and delivery. It refers to two
classes of concrete: normal-class and
special-class.

ViroDecs'" EPD | Holcim

<
O
2
où
X
E
>
©
œ
©
œ

LCA Information

Declared Unit

1 m° of ready-mix concrete.

Reference Service Life (RSL)

The RSL is not specified as the scope is from cradle to
gate.

Time Representativeness

The plant data for the LCA is based on 2017 calendar
year production data. The mix data for the LCA is based
on 2021 calendar year production data.

Databases and LCA Software Used

SimaPro (v8.4) was used for the LCA modelling which
developed the LCA Calculator, used as per the certified
EPD Process. It uses background data from:

1. The Australian National Life Cycle Inventory
Database (AusLCI) (2017)

2. Ecoinvent 3.4 (2017)

83. World Business Council for Sustainable
Development (WBCSD) Cement Sustainability
Initiative (CSI) Tool Project Database
(International Version) (2018); and

4. Product specific EPDs for admixtures and fibres.

The environmental impacts modelled from the CSI tool
and existing EPDs do not include impacts for the
additional Green Star (v1.2) impact categories included
in the environmental impact tables. The following impact
categories were calculated manually for the foreground
data:
e Use of renewable primary energy resources
used as raw materials
e Use of non-renewable primary energy excluding
non-renewable primary energy resources used
as raw materials
e Use of secondary material
e Use of renewable secondary fuels
e Use of non-renewable secondary fuels

ViroDecs'" EPD | Holcim

Allocation

Allocation was necessary to proportion inputs and
outputs to intermediate flows at the quarry and
processes at the batching plant level.

As much as possible, intermediate flows were allocated
physically based on weight (quarries) or based on m 2 of
concrete (at the batching plant). At the quarry level,
whenever physical allocation was not possible,
economic allocation was carried out based on Holcim'’s
internal cost system.

Regarding inputs, it was assumed that fly ash and silica
fumes are waste products and therefore burden-free.
Ground granulated blast furnace slag from steel blast
furnace production was allocated economically. Please
refer to the “Recycled Material” section for further detail.

=
©
ds
œ
=
Lu
©
=
=
<
©
er

Cut-Off Criteria
No flows were excluded on the basis of cut-off criteria.

Address and Contact Information

Holcim (Australia) Pty Ltd
Level 8, 799 Pacific Highway, Chatswood
NSW 2067, Australia

Web: www.holcim.com.au
Phone: +61 2 9412 6600
Data Quality

Data quality for the foreground data was assessed in terms of geographic and temporal representativeness. All data

>
sources were scored medium or higher. =
=]
(e]
œ
Q
. Electricity provider :
Electricity ose 2017 All states High
Diesel Supplier invoices 2017 All states High
National Pollution .
Pollutants Inventory (NPI) data 2017 All states High
Mains water Water utility invoices 2017 All states barring NSW Medium
Water — other
Coarse sources FCI AMNLEMEL ITS All states barring NSW Medium
aggregate (lakes, data
groundwater,
Manufactured rainwater)
sen Water discharge . .
. ; Measured site data 2017 All states barring NSW Medium
Fine aggregate from site
te d All states (excluding the Kalgoorlie
Invoices 2017 Quarry in WA which purchases High
sand and
raw feed from an external source)
Coarse
aggregate only)
Gravel CRIE ar | sr All states High
production amount
Spoil pet O 2017 All states High
records
All states
Aggregate Background data es censpot 2017 | | Hiah
transport Mederodel istances an (excluding Lynwood Quarry which 1g
loads per trip transports by freight rail)
. Electricity provider ;
Electricity Ho 2017 All states High
Diesel Supplier invoices 2017 All states High
Water metres,
Mains water with utility invoices 2017 All states High
as a
back-up
. dise Water — other
atchin ant i
gp sources Estimate based on 2017 All states Medium
(lakes, water balance
groundwater,
rainwater)
Water discharde Estimate based on
narg Holcim site 2017 All states Medium
from site
performance
metrics
Lubricating oil
d ATEILOI enerEts 2015 National Medium
Conveyor belt process
Holcim internal
Concrete mix Background data technical .
designs used to model database 207 QUCECE High
containing mix
designs
Estimate based on
Packaging Background data researched N/A N/A Medium
waste used to model packaging
material
and sizes

Background data sources were also assessed with respect to their timeliness, with all data sources being updated
within the 10 years required under PCR 2012:01.
System Diagram

The processes included in the LCA are presented in a process diagram in the figure below.

=
œ
el
D
.G
Q
=
©
a
>
ao

| Personnel | Raw material extraction
| impacts |
masses

E |
| go

On-site transport

A 1 Processing Steel manufacturing

Ê Chemical plant

Admixture production

Aggregates not for Aggregates not for aggregate
concrete concrete not for,
concrete

Additives manufacturing

_—_ Transport by transoceanic freight ship,
A2 nspor by roitucE rigid truck and/or domestic freight ship

A3

— 0
Lubricating oil goporete Packaging waste

Transport to site

ViroDecs'" EPD | Holcim 9
Description of System Boundaries and Excluded Lifecycle Stages

The scope of the LCA and EPD is from cradle to gate. Life cycle stages beyond Holcim's gate are excluded from the
LCA (see figure below).

=
G
Lu
D
S
Q
=
2
a
>
o

Environmental impacts relating to personnel, infrastructure and production equipment not directly consumed in the
process are excluded from the system boundary as per the Product Category Rules (2012:01 Construction Production
and Construction Services).

Benefits &

Construction Use Stage End of Life Stage loads for the

Product Stage next

product
system

Stage

a

8 5 5 5 on S P

[e] lei Q DA d = =
> s e es o a $ o 5 ©
| |. - Ne NN 5 Ne 2 = à
=] € A = fa 3 = O [0] d = œ re
o & = = = . = “ = 5 = TD = O ë _
_ © 5 ] ES D D ra) se] = où © E ©. >.
SE OS 8 $ 8 gg À © À LE Où + < 9 8 » où =
o = Œ = o > © © E € F w 2 = © Q 8 2
= g 5 g = © £ & © = = © S a re S 8
= +  & F = = E = = S 2 D F 5 el ge
= Z 2 = Et ® & & œ © d (re -
ü © 2 © G a © s} = œ col
(rs D £ (re G. 5 pes = a Œ

© E © 5 O O à 2

6 œ Œ Q me

O
A1 A2 A3 A4 A5 Bi B2 B3 B4 B5 B6 B7 Ci C2 C3 C4 D
X X X  MND MND MND MND MND MND MND MND MND MND MND MND MND MND

*Module not declared (MND)

ViroDecs'" EPD | Holcim 10
EPD Product Description and Use

ViroDecs'" Ready-mix concrete - NSW - Far South Coast —- ECOPact Range

@
o
=)
où
=
©
LL d
cs
É
©
tr)
©
Q
ds
©
5
D
©
Le
(Su

A detailed breakdown of the functional properties of the ready-mix concrete included in this EPD are provided below.
Product environmental information should only be compared with consideration of the product's requisite function.

MIX
DESCRIPTIONS NSW - Far South Coast - ECOPact Range

Strength (MPa) Mix code Description of use
NE202E159 / S20 20mm 100mm SLUMP
NZ202E 159 ECOPACT CONCRETE
NE202E359 / S20 20mm 140mm SLUMP
NZ202E359 ECOPACT CONCRETE
NE252E159 / S25 20mm 100mm SLUMP
NZ252E 159 ECOPACT CONCRETE
NE252E359 / S25 20mm 140mm SLUMP
NZ252E359 ECOPACT CONCRETE
NE322E159 / S32 20mm 100mm SLUMP
NZ322E 159 ECOPACT CONCRETE
NE322E359 / S32 20mm 140mm SLUMP
NZ322E359 ECOPACT CONCRETE
NE402E159 / S40 20mm 100mm SLUMP
NZ402E 159 ECOPACT CONCRETE
NE402E359 / S40 20mm 140mm SLUMP
NZ402E359 ECOPACT CONCRETE
NE201E159 / S20 10mm 100mm SLUMP
NZ201E159 ECOPACT CONCRETE
NE201E359 / S20 10mm 140mm SLUMP
NZ201E359 ECOPACT CONCRETE
NE251E159 / S25 10mm 100mm SLUMP
NZ251E159 ECOPACT CONCRETE
NE251E359 / S25 10mm 140mm SLUMP
NZ251E359 ECOPACT CONCRETE
NE321E159 / S32 10mm 100mm SLUMP
NZ321E159 ECOPACT CONCRETE
NE321E359 / S32 10mm 140mm SLUMP
NZ321E359 ECOPACT CONCRETE
NE401E159 / S40 10mm 100mm SLUMP
NZ401E159 ECOPACT CONCRETE
NE401E359 / S40 10mm 140mm SLUMP
NZ401E359 ECOPACT CONCRETE

ViroDecs'" EPD | Holcim 11
Content Declaration

The following table provides a summary of the materials included in Holcim ready-mix concrete and their relative

composition by weight.

General purpose cement

Aggregate

Supplementary cementitious materials
Water

Admixtures

5-21%
67-84%
0-11%
11.6-12%

0.01-0.02%

[]
o
æ)
où
[=
©
=
[os
En
©
(A
©
Q
—
©
=]
T
[e)
Le
Q.

Holcim Ready-mix concrete is classified as Non-Dangerous Goods according to the Australian Code for the Transport
of Dangerous Goods by Road and Rail. The safety data sheet for pre-mixed concrete lists all associated hazard

phrases.

The gross weight of this declared material makes up a minimum of 99% of the products covered by this EPD.

Packaging

Holcim ready-mix concrete is delivered in bulk with no
packaging.

Recycled Material

BS EN 16757:2017 specifically lists the following
materials relevant to the study as co-products:

e Fly ash;
° Ground granulated blast furnace slag; and
°  Silica fume

As such, the above materials are considered as co-

products of their production process and the impacts for
their production process are allocated according to PCR

2012:01 Construction Products and Construction
Services (co-produced goods, multi-output allocation).

ViroDecs'" EPD | Holcim

Default background data from LCA databases was used

to model the above co-products:

° Fly ash: AusLCI process for fly ash treats it as a

waste material and only includes transport
impacts.
° Ground granulated blast furnace slag: the

AusLCI process for slag is allocated based on
economic value, as the product has a significant

economic value at the point of collection.

° _ Silica fume: the ecoinvent process for silica
fume treat it as a waste material and only
includes transport impacts.

The allocation approach of the AusLCI LCA database

was adopted as a default for secondary data and

The AusLCI dataset conforms to EN 15804 when
applying allocation to its various processes and sub-
processes.

processes (e.g. secondary fuel in cement production).
Environmental Performance

The environmental impacts considered in this EPD are listed in the table below. All further tables from this point will

contain abbreviation only.

Impact Category Abbreviation Measurement Unit

Potential Environmental Impacts
Global warming potential

Ozone depletion potential

Acidification potential

Eutrophication Potential

Photochemical ozone creation potential
Abiotic depletion potential (elements)
Abiotic depletion potential (fossil fuels)
Resource use

Use of renewable primary energy excluding renewable primary
energy resources used as raw materials

Use of renewable primary energy resources used as raw
materials

Total use of renewable primary energy resources (primary
energy and primary energy resources used as raw materials)

Use of non-renewable primary energy excluding non-renewable
primary energy resources used as raw materials

Use of non- renewable primary energy resources used as raw
materials

Total use of non- renewable primary energy resources (primary
energy and primary energy resources used as raw materials)

Use of secondary material

Use of renewable secondary fuels
Use of non-renewable secondary fuels
Use of net fresh water

Output categories

Hazardous waste disposed
Non-hazardous waste disposed
Radioactive waste disposed/stored
Components for reuse

Materials for recycling

Materials for energy recovery
Exported energy

Optional Green Star (v1.2) indicators
Human Toxicity

Land use

Water stress indicator

lonising radiation

Particulate matter

ViroDecs'" EPD | Holcim

GWP
ODP
AP
EP
POCP
ADPE
ADPF

PERE

PERM

PERT

PENRE

PENRM

PENRT

SM
RSF
NRSF
FW

HWD
NHWD
RWD
CRU
MFR
MER
EE

HT
LU
WSI

PM

kg CO, equivalents (GWP100)

kg CFC 11 equivalents
kg SO; equivalents
kg POS equivalents
kg C-H, equivalents
kg Sb equivalents
MJ net calorific value

MJ, net calorific value
MJ, net calorific value
MJ, net calorific value
MJ, net calorific value
MJ, net calorific value

MY, net calorific value

Kg
MJ, net calorific value
MJ, net calorific value
m3

kg
kg
kg
kg
kg
kg
MJ per energy carrier

CTUh
m2
m3
kBq U235 eq
kg PM2.5 eq

@
©
=
œ
=
Lu
©
=
Lu
©
(su
œ
ne
=
©
=
=
©
È
>
€
ui

NSW - Far South Coast —- ECOPact Range

NSW - Far South Coast - ECOPact Range: 1m° of ViroDecs’" ready-mix concrete — Primary indicators

_——. + RES > DE

@
©
=
œ
=
Lu
©
=
Lu
©
(su
rc
+
=
©
=
=
©
È
>
€
ui

kg CO» eq kg CFC-11 eq kg SO: eq kg PO.Ÿ eq kg C2H4 eq kg Sb eq

RO 16202150 202.13 3.12E-06 4.64E-01 1.08E-01 1.64E-02 1.21E-04 1.49E+03
RON 12026550 203.16 3.12E-06 4.66E-01 1.04E-01 1.66E-02 1.21E-04 1.51E+03
RP 16252150 222.07 3.31E-06 5.04E-01 1.12E-01 1.76E-02 1.30E-04 1.62E+03
RE 12526550 223.24 3.31E-06 5.06E-01 1.18E-01 1.78E-02 1.31E-04 1.64E+03
REC 15225150 254.08 3.61E-06 5.67E-01 1.26E-01 1.94E-02 1.45E-04 1.82E+03
REP 13226550 255.46 3.62E-06 5.70E-01 1.27E-01 1.96E-02 1.46E-04 1.84E+03
RO 1202150 300.03 4.05E-06 6.58E-01 1.46E-01 2.20E-02 1.67E-04 2.11E+03
ST 1E402E550 301.67 4.05E-06 6.61E-01 1.47E-01 2.23E-02 1.67E-04 2.13E+03
PO 1201150 202.73 3.14E-06 4.67E-01 1.04E-01 1.66E-02 1.22E-04 1.50E+03
RON 1E201E550 203.69 3.14E-06 4.69E-01 1.05E-01 1.68E-02 1.22E-04 1.52E+03
RC 165615 222.69 3.33E-06 5.07E-01 1.18E-01 1.78E-02 1.31E-04 1.63E+03
RE 1625165350 223.76 3.33E-06 5.08E-01 1.13E-01 1.79E-02 1.31E-04 1.64E+03
RE 1E22E150 254.73 3.64E-06 5.70E-01 1.27E-01 1.96E-02 1.46E-04 1.83E+03
REP 1623216550 255.98 3.64E-06 5.72E-01 1.27E-01 1.98E-02 1.46E-04 1.85E+03
RO 101150 300.67 4.07E-06 6.61E-01 1.46E-01 2.22E-02 1.67E-04 2.12E+03
ROM 12016550 302.17 4.08E-06 6.63E-01 1.47E-01 2.25E-02 1.68E-04 2.14E+03

NSW - Far South Coast - ECOPact Range: 1m° of ViroDecs'" ready-mix concrete — Resource use parameters

ue . qu Lun … DEEE

Mincv MiNncv Mincv MiNncv Mincv MiNncv MiNncv MiNncv

NE202E159 2.14E+01 O.00E+00 2.14E+01 8.15E+02 1.52E+02 9.67E+02 9.50E+01  O0.00E+00 0.00E+00  5.90E-01
NE202E359 2.14E+01 O.00E+00 2.14E+01 8.32E+02 1.54E+02 9.87E+02 9.50E+01  O0.00E+00 0.00E+00  5.89E-01
NE252E159 2.34E+01 O0.00E+00 2.34E+01 8.83E+02 1.47E+02  1.03E+03  1.05E+02 O0.00E+00 0.00E+00 6.18E-01
NE252E359 2.34E+01 O0.00E+00 2.34E+01 9.03E+02 1.50E+02  1.05E+03 1.05E+02  O0.00E+00 0.00E+00 6.18E-01
NE322E159 2.65E+01  O0.00E+00 2.65E+01 9.94E+02 1.39E+02  1.13E+03  1.23E+02  O0.00E+00 0.00E+00  6.65E-01
NE322E359 2.65E+01 O0.00E+00 2.65E+01  1.02E+03 1.42E+02  1.16E+03  1.23E+02 O0.00E+00 0.00E+00  6.65E-01
NE402E159  3.10E+01  O0.00E+00 3.10E+01 1.15E+03 1.27E+02 1.28E+03 1.47E+02  O0.00E+00 0.00E+00 7.31E-01
NE402E359  3.11E+01 O0.00E+00 3.11E+01  1.18E+03 1.30E+02 1.31E+03  1.47E+02  O0.00E+00 0.00E+00 7.31E-01
NE201E159 2.14E+01 O.00E+00 2.14E+01 8.17E+02 1.60E+02 9.77E+02 9.50E+01  O0.00E+00 0.00E+00  5.91E-01
NE201E359 2.14E+01 O0.00E+00 2.14E+01 8.35E+02 1.60E+02 9.96E+02 9.50E+01  0.00E+00 0.00E+00 5.91E-01
NE251E159 2.33E+01 O0.00E+00 2.33E+01 8.86E+02 1.56E+02 1.04E+03  1.05E+02  0.00E+00 0.00E+00  6.20E-01
NE251E359 2.34E+01 O0.00E+00 2.34E+01 9.06E+02 1.56E+02  1.06E+03 1.05E+02  O0.00E+00 0.00E+00  6.20E-01
NE321E159 2.65E+01  O0.00E+00 2.65E+01 9.96E+02 1.47E+02 1.14E+03  1.23E+02  O0.00E+00 0.00E+00  6.66E-01
NE321E359 2.66E+01  O0.00E+00 2.66E+01  1.02E+03 1.47E+02 1.17E+03  1.23E+02  O0.00E+00 0.00E+00  6.66E-01
NE401E159 3.11E+01 O.00E+00 3.11E+01 1.15E+03  1.35E+02  1.29E+03 1.47E+02  O0.00E+00 0.00E+00  7.32E-01
NE401E359 3.11E+01 O0.00E+00 3.11E+01  1.18E+03  1.35E+02  1.32E+03  1.47E+02  0.00E+00 0.00E+00  7.32E-01

PARAMETERS
DESCRIBING
RESOURCE USE

Strength
(MPa)

ViroDecs'" EPD | Holcim 14
NSW - Far South Coast - ECOPact Range: 1m° of ViroDecs" ready-mix concrete —- Waste categories and output

flows
kg kg kg Le] kg MJ

WASTE CATEGORIES AND
OUTPUT FLOWS

ROM 1202150 7.02E-04 5.70E+00 5.22E-06 0.00E+00 0.00E+00 0.00E+00 0.00E+00
ROM 1E202E550 6.99E-04 5.70E+00 5.20E-06 0.00E+00 0.00E+00 0.00E+00 0.00E+00
REC 12525150 7.46E-04 6.10E+00 5.45E-06 0.00E+00 0.00E+00 0.00E+00 0.00E+00
RE 12526550 7.43E-04 6.10E+00 5.44E-06 0.00E+00 0.00E+00 0.00E+00 0.00E+00
RE 12225150 8.18E-04 6.75E+00 5.83E-06 0.00E+00 0.00E+00 0.00E+00 0.00E+00
REP 13226550 8.14E-04 6.75E+00 5.82E-06 0.00E+00 0.00E+00 0.00E+00 0.00E+00
RO 15202150 9.19E-04 7.67E+00 6.36E-06 0.00E+00 0.00E+00 0.00E+00 0.00E+00
RO 1520265350 9.15E-04 7.67E+00 6.35E-06 0.00E+00 0.00E+00 0.00E+00 0.00E+00
RP 12015 7.01E-04 5.72E+00 5.23E-06 0.00E+00 0.00E+00 0.00E+00 0.00E+00
ROM 1E201E550 7.01E-04 5.73E+00 5.23E-06 0.00E+00 0.00E+00 0.00E+00 0.00E+00
RC 15150 7.44E-04 6.12E+00 5.46E-06 0.00E+00 0.00E+00 0.00E+00 0.00E+00
RE 16251E550 7.44E-04 6.13E+00 5.46E-06 0.00E+00 0.00E+00 0.00E+00 0.00E+00
RE 2150 8.16E-04 6.77E+00 5.84E-06 0.00E+00 0.00E+00 0.00E+00 0.00E+00
REP 1E221E550 8.17E-04 6.78E+00 5.84E-06 0.00E+00 0.00E+00 0.00E+00 0.00E+00
ROM 16401150 9.18E-04 7.70E+00 6.38E-06 0.00E+00 0.00E+00 0.00E+00 0.00E+00
BST 1E401E5350 9.19E-04 7.70E+00 6.38E-06 0.00E+00 0.00E+00 0.00E+00 0.00E+00

NSW - Far South Coast - ECOPact Range: 1m° of ViroDecs’" ready-mix concrete — Green Star As Built v1.2 optional
indicators

2 m°

CTUh m kBq U235 eq kg PM2.5 eq
RU 162025 150 6.50E-09 1.14E-02 6.48E-01 3.77E-02 2.89E-01
TN 12025359 6.50E-09 1.14E-02 6.44E-01 3.76E-02 2.90E-01
RE 162525 150 7.16E-09 1.21E-02 7.02E-01 3.93E-02 2.94E-01
12525350 7.16E-09 1.21E-02 7.02E-01 3.92E-02 2.96E-01
RE 13227150 8.22E-09 1.33E-02 7.96E-01 4.20E-02 3.01E-01
TN 1153225350 8.22E-09 1.33E-02 7.97E-01 4.19E-02 3.03E-01
ST  1E402€150 9.75E-09 1.50E-02 9.31E-01 4.58E-02 3.12E-01
TN  1E402E350 9.75E-09 1.50E-02 9.32E-01 4.57E-02 3.15E-01
RE  1E201E 150 6.51E-09 1.15E-02 6.46E-01 3.78E-02 2.96E-01
TN  1E201E350 6.51E-09 1.15E-02 6.46E-01 3.78E-02 2.96E-01
RE  1E251E 150 7.17E-09 1.22E-02 7.05E-01 3.94E-02 3.01E-01
NN  1E251E350 7.17E-09 1.22E-02 7.05E-01 3.94E-02 3.01E-01
RE  1E521E150 8.23E-09 1.34E-02 7.99E-01 4.21E-02 3.09E-01
ET 13215350 8.23E-09 1.34E-02 7.99E-01 4.21E-02 3.09E-01
ST 1401150 9.76E-09 1.51E-02 9.34E-01 4.60E-02 3.20E-01
TN  1E401E359 9.76E-09 1.51E-02 9.34E-01 4.60E-02 3.20E-01

ViroDecs'" EPD | Holcim 15
Other life cycle stages not included in
this EPD

u
©
D
©
ni
ao
©
o
>
©
(
=
=
LD
©
£
Ld
O

While the LCA study and EPD only consider the cradle to gate environmental impacts of Holcim’s ready-mix concrete,
practitioners using the EPD for the purpose of whole-of-life building studies or the functional comparison of different
building products on a whole-of-life basis will consider concrete’s other life cycle stages. Some of the environmental
impacts of benefits associated with other life cycle stages not included in this EPD are described in the following
sections.

Lifetime absorption of CO:

Carbonation is a natural process whereby concrete absorbs carbon dioxide (CO) from the atmosphere through a
chemical reaction between the CO; in the ambient air and hydration products within the concrete (CaOH:). Ready-mix
concrete can be subject to carbonation from the use stage onward (i.e. after construction and curing). From a life cycle
impact accounting perspective, this process can also be referred to as ‘reabsorption’, since the CO; emitted during the
cement manufacturing process can be paritly offset by the lifetime absorption of CO», therefore reducing the net CO;
emissions associated with concrete over its lifetime.

The carbonisation process is a commonly known process in building design and is typically taken into consideration by
engineers when specifying special-class concrete.

The total amount of CO; absorption during the life cycle of concrete is subject to a range of factors and varies over
time. The calculation has been standardised in the British and European Standard BS EN 16757:2017 Sustainability
of construction works — Environmental Product Declarations — Product Category Rules for concrete and concrete
elements. It is recommended that practitioners make use of this standard when conducting whole-of-life building
studies and if the building materials include substantial amounts of concrete. Please note that CO: absorption has not
been considered in this EPD andis not reflected in the EPD results tables.

End of life scenarios

BS EN 16757:2017 presents four end of life scenarios for concrete:

1. Disposal of concrete at a landfill site,

2. Reuse of recovered concrete elements in new construction works,

83. Use of concrete debris, e.g. In land restoration, or

4.  Crushing/recycling of concrete:
a. Crushed concrete substitutes primary material without further processing, or
b. Substitution of natural aggregates in fresh concrete.

Scenarios 2, 3 and 4 can all result in benefits and loads outside the system boundary and thus should be considered
in a whole-of-life building study or when comparing concrete products on a functional basis in line with BS EN
16757:2017.

ViroDecs'" EPD | Holcim 16
References

Australasian EPD Programme. (2017). Guidance on the use of INA in EPDs.

References

Australasian EPD Programme. (2018). Guidance on the use of background LCI data.
Australasian EPD Programme (2018) Instructions of the Australasian EPD Programme V3.0.

Australian Life Cycle Inventory Database Initiative (AusLCI). (2015). Guidelines for Data Development for an
Australian Life Cycle Inventory Database, Data Standard.

British Standards Institution. (2014). Sustainability of construction works. Environmental product declarations. Core
rules for the product category of construction products, BS EN 15804:2012+A1:2015. British Standards Institution.

British Standards Institution. (2017). Sustainability of construction works — Environmental product declarations —
Product Category Rules for concrete and concrete elements, BS EN 16757:2017. British Standards Institution.

Ecoinvent Centre. (2017). Ecoinvent version 3 database. Zurich: ETH, Agroscope, EMPA, EPFL, PSI. Retrieved from
www.ecoinvent.org.

EPD International. (2017). General Programme Instructions (GPI) for the International EPD System V3.0. Retrieved
from www.envirodec.com.

EPD International. (2018). Product Category Rules for Construction Products and Construction Services, PCR2012:01
v2.3. Stockholm: EPD International.

ISO. (2006). Environmental labels and declarations — Type III environmental declarations — Principles and procedures,
ISO 14025:2006. Geneva: International Organization for Standardization.

ISO. (2006). Environmental management — Life cycle assessment — Principles and framework, ISO 14040:2006.
Geneva: International Organization for Standardization.

ISO. (2018). Environmental management. Life cycle assessment. Requirements and guidelines, ISO
14044:2006+A1 :2018. Geneva: International Organization for Standardization.

AusLCI. (2017) AusLCI Database. Retrieved from AusLCI: www.auslei.com.au/

Man Yu, Thomes Wiedmann, Robert Crawford, Catriona Tait, ‘The Carbon Footprint of Australia’s Construction
Sector, Procedia Engineering, Volume 180, 2017, Pages 211-220, ISSN 1877-7058,

(http;/www.sciencedirect.com/science/article/pi/S1877705817316879)

ViroDecs'" EPD | Holcim 17
Programme-related information and verification

Holcim (Australia) Pty Ltd Level 8,
799 Pacific Highway

Chatswood NSW 2067, Australia

Web: www.holcim.com.au Phone:
+61 2 9412 6600

Declaration Owner

olcim

EPD Australasia Limited

315a Hardy Street Nelson

7010 a ®
EPD Programme Operator AUSTRALASIA

New Zealand

Web: www.epd-australasia.com Email:
info@epd-australasia.com Phone: 02
8005 8206

ENVIRONMENTAL PRODUCT DECLARATION

Ÿ,

epstengroup

Holcim (Australia) Pty Ltd Level 8,
799 Pacific Highway

Chatswood NSW 2067, Australia
Web: www.holcim.com.au Phone: +61 2 9412
6600

EPD Produced by

olcim

Epsten Group

Suite 2600, 101 Marietta St NW, Atlanta,
EPD Process Certified by Georgia 30303, USA

Web: www.epstengroup.com

EPD Registration Number S-P-03714

Valid From 2021-10-18
Version
Valid Until 2026-10-18

PCR 2012:01 Construction Products and Construction Services, Version 2.3,

Product category rules 2018-11-15

Product group classification UN CPC 54

Australia

Geographical Scope

Reference Year for Data 2017 Plant Data, 2021 Mix/Materials Data

_
Oo

CEN standard EN 15804:2012+a1:2013 served as the core PCR

PCR 2012:01 Construction Products and Construction Services, Version

Product category rules 2.3, 2018-11-15

PCR review was conducted The Technical Committee of the International EPD® System.
by Chair: Massimo Marino. Contact via info@environdec.com

Independent third-party

verification of the declaration EPD process certification
and data, according to ISO EPD verification
14025:2006:

Third Party Verifier Epsten Group, Inc., Katherine McFeaters:
Accredited by: A2LA, Certificate #3142.03

Procedure for follow-up of
data during EPD validity
involves third party verifier:

Programme-related information and verification:

The EPD owner has the sole ownership, liability, and responsibility for the EPD. EPDs within the same product
category but from different programmes may not be comparable. EPDs of construction products may not be
comparable if they do not comply with EN 15804.

ViroDecs'" EPD | Holcim

18
Holcim

This publication supersedes all previous literature on this subject. As the
specifications and details contained in this publication may change, please check
with Holcim Customer Service for confirmation of current issue. This publication
provides general information only and is no substitute for professional technical
engineering advice. Users must make their own determination as to the suitability of
this information or any Holcim product for their specific circumstances. Holcim
accepts no liability for any loss or damage resulting from their specific circumstances.
Holcim accepts no liability for an loss or damage resulting from any reliance on the
information provided in this publication. Holcim is a registered trademark of
LafargeHolcim Ltd. “Strength. Performance. Passion.” and “ViroDecs” are trademarks
of Holcim (Australia) Pty Ltd.

© October 2021 Holcim (Australia) Pty Lid ABN 87 732 297. All rights reserved. This
guide or any part of it may not be reproduced without prior written consent of Holcim.
