Ÿ = ©
| ° AUSTRALASIA E P D EPD
H O C [ m ENVIRONMENTAL PRODUCT DECLARATION

Table of Contents

Introduction ................................................................. eee 3
About Holcim.................................................................. sie 4
ViroDecs' M Special — a first for ready-mix concrete in Australia 5
ViroDecs'" Special at a glance.................................................................. 5
Ready-mix concrete ..…............................................................ eee 6
LCA Information... sssssssssssssseeeeeeenennennnnnnnnennnnnsnnsnnnsensnennneeneee 7
EPD Product Description and Use... sssssssseseneeeeeeeeeeeeeeeeeennnnes 11
Environmental Performance... sise 13
Other life cycle stages not included in this EPD........................ 19
References... isiiiieeeeeeeeeeeeeeeeeeeeeeeeeeeeeeeeeeeeeneeeeeennnee 20
Programme-related information and verification 21
Version Number Revision Date Description of Changes

1.0 N/A N/A

ViroDecs'" EPD | Holcim 2
Introduction

All around the world, the expectation for Governments
and organisations to provide enhanced transparency
and disclosure of environmental impacts, such as
greenhouse gas (GHG) emissions, has been growing.
This follows the landmark COP 21 Paris Agreement in
2015 in which all nations agreed to ambitiously pursue
efforts to combat climate change and its effects.

At the same time, the global demand for construction
materials is also growing due to worldwide population
growth and an increase in urbanisation. In fact, concrete
is the second most used commodity in the world behind
water, and typically a major contributor to the embodied
GHG emissions of an infrastructure or property asset.

This clearly demonstrates both the essential need for
construction materials now and in the future, as well as
the necessity for the construction materials industry to
be a leading part of the solution addressing climate
change.

At Holcim, we recognise our responsibility to contribute
to global emissions reduction targets and we have
developed a roadmap with a number of actions to direct
our efforts.

Our ViroDecs'" range of ready-mix concrete
represented by an Environmental Product Declaration
(EPD) is one such initiative for Holcim in Australia.

ViroDecs " EPD | Holcim
About Holcim

Western
Australia

ePerth

AUSTRALIAN OPERATIONS

ET Precast pipe and product

L2 °
Darwin

Northern ET
Territory
Queensland [3
e Brisbane
South
En Australia
Co. New South jo |
Wales / ACT
Era e Sydney 7:
e Adelaide e Canberra ES
Victoria
* Melbourne EX
Tasmania E
e Hobart [a

“The breakdown of Australian operations is based on 2017 site data used for the EPD Life Cycle
Assessment modelling and includes tolling sites and excludes mobile or temporary sites

About Holcim

Holcim Australia is a leading supplier of construction
materials in Australia, dating back to 1901. Today
Holcim continues to supply essential construction
materials including aggregates, sand, ready-mix
concrete, engineered precast concrete and prestressed
concrete solutions to a range of customers and projects
throughout Australia.

Holcim operates right across the Australian continent
supplying concrete from a network of concrete plants,
quarries, precast and concrete pipe places, and mobile
and on-site project facilities.

Sustainability is at the core of our strategy, with our

industry's first 2050 net-zero targets, endorsed by the
Science Based Targets initiative (SBTi).

ViroDecs'" EPD | Holcim

Globally, Holcim is 70,000 people around the world who
are passionate about building progress for people and
the planet through four business segments: Cement,
Ready-Mix Concrete, Aggregates and Solutions &
Products.

Holcim builds progress for people and the planet. As a
global leader in innovative and sustainable building
solutions, Holcim is enabling greener cities, smarter
infrastructure and improving living standards around the
world. With sustainability at the core of its strategy
Holcim is becoming a net zero company, with its people
and communities at the heart of its success. The
company is driving circular construction as a world
leader in recycling to build more with less.
ViroDecs " Special — a first for ready-mix

concrete in Australia

The Holcim ViroDecs'" Special provides project-specific,
on-demand Environmental Product Declarations (EPDs) to
Holcim's customers. This capability represents a
significant step in Holcim's sustainability journey and
embodies our multi-disciplinary approach to embedding
sustainability into our organisation and operations. With
the introduction of our ViroDecs " Special, third-party
verified data will underpin our capability to work with our
customers from tender through to design and construction
to optimise ready-mix concrete mix designs and report on
sustainability performance.

The publication of the original ViroDecs'" EPD in 2019
introduced quality, third-party verified embodied life cycle
impact data for ready-mix concrete into the Australian
market for the first time. Holcim has been pleased by the
positive response from the industry. The message was
loud and clear: “we want transparency and we want a
evidence-based approach to specification, procurement
and reporting”. With the introduction of our ViroDecs
Special, Holcim’s customers can now specify concrete
sustainability performance in terms of CO-e, with the
confidence that our claims are backed by our third-party
verified EPD Process Certification.

ViroDecs'" EPD | Holcim

Holcim ViroDecs'" Special is backed by an EPD
Process Certification. Its not only a first for concrete but
a first for any product in Australia. Our EPD Process
Certification is a stamp of approval to produce compliant
EPDs in-house, opening up significant capability and
flexibility in producing and using life cycle impact data to
inform our operations and our customers.

To gain our EPD Process Certification, Holcim invested
in embedding Life Cycle Assessment (LCA) into our
systems and processes. We have satisfied a rigorous,
third-party evaluation in accordance with the relevant
ISO standards and guidelines of the International EPD
Programme and EPD Australasia.

This EPD has been developed using our EPD Process
Certification for Plungie Brisbane General Supply with
production occurring at various locations in the Brisbane
area.

Ready-mix concrete

Aggregrates
Load and Haul Crushing and Screening Stockpiling and Distribution

(
2
o
=
©
=
©
(a)
x
E
>
T
G
®
[ee

Concrete
Batching

Material Handling and Storage
+, e

Summary of properties and classes

Concrete is prepared by mixing cement, ° Normal-class — designed for residential
coarse and fine aggregates, and water, with applications, low rise buildings, paving
or without the addition of auxiliary agents and driveways etc. Its specification and
and additives. The fresh concrete is placed ordering have been simplified as far as
on the building site or prefabricated in practicable.

factory moulds, compacted and hardened in e Special-class — allows the purchaser to
the desired shape by the hydration of incorporate into the project specification
cement to form concrete. any special requirements for the project.

Special-class concrete is typically
supplied to major and high-end
construction projects from high rise
buildings, dams and spillways, roads and
bridges to public works infrastructure etc.
Special-class concrete is typically
specified in accordance with the technical
parameters and performance
requirements, which can include high-
strength/high-performances concrete,
high durability or marine application, post-
tensioned, high-pumpability, super
workable, piling concrete, architectural
off-form finishes and other decorative
applications.

General Australian Standard AS 1379 sets
down a number of different ways of
specifying and ordering concrete to
promote uniformity, efficiency and economy
in production and delivery. It refers to two
classes of concrete: normal-class and
special-class.

ViroDecs " EPD | Holcim 6
LCA Information

Declared Unit
1 m° of ready-mix concrete.

Reference Service Life (RSL)

The RSL is not specified as the scope is from cradle to
gate.

Time Representativeness

The plant data for the LCA is based on 2017 calendar
year production data. The mix data for the LCA is based
on 2022 calendar year production data.

Databases and LCA Software Used

SimaPro® LCA software (v 9.1) was used for the LCA
modelling which developed the LCA Calculator, used as
per the certified EPD Process. It uses background data
from:

1. The Australian National Life Cycle Inventory
Database (AusLCI) (2018)

2. Ecoinvent 3.6 (2019)

3. Global Cement and Concrete (GCCA) EPD Tool
Project Database version 3.1 (International
Version) (2021); and

4. Product specific EPDs for pigments and fibres.

The environmental impacts modelled from the existing
EPDs do not include impacts for the additional Green
Star (v1.2) impact categories included in the
environmental impact tables. The following impact
categories were calculated manually for the foreground
data:

e Use of renewable primary energy resources
used as raw materials

e Use of non-renewable primary energy excluding
non-renewable primary energy resources used
as raw materials

e Use of secondary material

e Use of renewable secondary fuels

e Use of non-renewable secondary fuels

ViroDecs'" EPD | Holcim

Allocation

Allocation was necessary to proportion inputs and
outputs to intermediate flows at the quarry and
processes at the batching plant level.

As much as possible, intermediate flows were allocated
physically based on weight (quarries) or based on m? of
concrete (at the batching plant). At the quarry level,
whenever physical allocation was not possible,
economic allocation was carried out based on Holcim's
internal cost system.

Regarding inputs, it was assumed that fly ash and silica
fumes are waste products and therefore burden-free.
Ground granulated blast furnace slag from steel blast
furnace production was allocated economically. Please
refer to the “Recycled Material” section for further detail.

c
2
ds
&
E
Lu
©
&
=
<
©
=

Cut-Off Criteria
No flows were excluded on the basis of cut-off criteria.

Address and Contact Information

Holcim (Australia) Pty Ltd
Level 7, 799 Pacific Highway, Chatswood
NSW 2067, Australia

Web: www.holcim.com.au
Phone: +61 2 9412 6600
Data Quality

Data quality for the foreground data was assessed in terms of geographic and temporal representativeness. All data
sources were scored medium or higher.

Temporal
Input/outputs Sub-processes Data source scope Geographic scope Quality

>
=
œ
3
(e]
œ
ds
œ
Q

Electricity provider

Electricity invoices 2017 All states High
Diesel Supplier invoices 2017 All states High
National Pollution |
Pollutants Inventory (NPI) data 2017 All states High
Mains water Water utility invoices 2017 All states barring NSW Medium
SOA Water — other
aggregate
SeUreS (ALES, Metered withdrawal
groundwater, EE 2017 All states barring NSW Medium
rainwater)
Manufactured .
nd Water discharge . . .
sa from site Measured site data 2017 All states barring NSW Medium
. Explosives All states (excluding the
Fine aggregate (Manufactured 2017 Kalgoorlie Quarry in WA which
sand and Coarse Invoices purchases raw feed from an High
aggregate only) external source)
Calculated — spoil + |
Gravel production amount 2017 All states High
Spoil Holcim waste records 2017 All states High
Actual transport All states
Acte je EE ae distances and loads 2017 (excluding Lynwood Quarry High
ranspor use 10 moge per trip which transports by freight rail)
. Electricity provider .
Electricity invoices 2017 All states High
Diesel Supplier invoices 2017 All states High
Water metres, with
: utility invoices as a .
Mains water back-up 2017 All states High
Concrete Water — other
batching plant sure (ES, Estimate based on |
groundwater, water balance 2017 All states Medium
rainwater)
MED CRC Estimate based on
EE GISGNENGE Holcim site .
from site performance metrics 2017 All states Medium
Lubricating oil AusLCI concrete
Conveyor belt process 2015 National Medium
Holcim internal
Concrete mix Background data technical database 2017 All states High
designs used to model containing mix
designs
Estimate based on
Packaging Background data researched N/A N/A Medium
waste used to model packaging material
and sizes

Background data sources were also assessed with respect to their timeliness, with all data sources being updated
within the 10 years required under PCR 2019:14.

ViroDecs'" EPD | Holcim
System Diagram

The processes included in the LCA are presented in a process diagram in the figure below.

Raw material extraction

=
œ
Lu
D
eo
Q
=
©
a
>
[2]

Gravel }

Diesel EEE
Explosives

Water r—
| Diesel}? On-site transport

Coarse
aggregate for
concrete Electricity

Processing

Aggregates for ggregate fo

Manufactured Diesel concrete

Diesel Aggregates not for Aggregates not for aggregate
concrete concrete not for
concrete

Additives manufacturing

ini Transport by transoceanic freight ship,
ranepor doi rues rigid truck and/or domestic freight ship

——— ET mm +—
ne
Admixtures
{rentes
| Adaïties |
[| _Wastewater |

Ready-mix
concrete Packaging waste

Transport to site

ViroDecs " EPD | Holcim 9
Description of System Boundaries and Excluded Lifecycle Stages

The scope of the LCA and EPD is from crade to gate. Life cycle stages beyond Holcim'’s gate are excluded from the
LCA (see figure below).

=
œ
Lu
D)
G
Q
=
©
2
o
>
[2]

Environmental impacts relating to personnel, infrastructure and production equipment not directly consumed in the
process are excluded from the system boundary as per the Product Category Rules (2019:14 Construction Production
and Construction Services).

Benefits &
Construction Use Stage End of Life Stage loads for the
next
product
System

Product Stage

Stage

ao

FD c

8 5 5 $ £ EP
È S À &S 2 9 $ 2% © ©
[en a Fi O € [es D D É _ >
Q D = œ eo a g > = É _ ®
3 = .Q Ë e = + (eo) œ £ = sa L
(0) + Æ + = Er = © = 5 = + © do =
= © 5 © Æ G Fu © O c % re] E ©. >.S
S 5 2 à ® À + £ £ ww = < 9 $ »e 5 =
© C GS C D S © D = = en TG © C _ A à 2
E SG 3 g E O £ G © c = © Œ 8 ü oo
S É S = = = = = [= .O 5 : F D © L +
= Z 2 © a S 5 w : ü (a) fre .
& © a © G 5 © © = œ ro)
œ = £ (rs ©. = Q a e in)

© S © 3 (@) O & oi)

6 Œ œ Q œ

O
A1 A2 A3 A4 A5 Bi B2 B3 B4 B5 B6 B7 (C1 C2 C3 C4 D
X X X MND  MND MND MND MND MND MND MND MND MND MND MND MND MND

“Module not declared (MND)

ViroDecs'" EPD | Holcim 10
EPD Product Description and Use

ViroDecs'" Ready-mix concrete —- Queensland -— Brisbane — Plungie General Supply

À detailed breakdown of the functional properties of the ready-mix concrete included in this EPD are provided below.

Product environmental information should only be compared with consideration of the product's requisite function.

S50/10/750 AGILIA VERTICAL

Note: Some customer invoices may have a Z as the second charterer in their mix code (e.g. QZ202E). This indicates that the mix was sold as a
carbon neutral ready-mix concrete (i.e. the residual Global Warming Potential was offset). To find the applicable mix code, please substitute the
seconded charter in the mix code with an E (e.g. QE202E).

ViroDecs'" EPD | Holcim 11

o
n
=)
où
(=.
©
=
cs
A
[a]
n
d
Q
L
a)
p])
D
©
Le
Q

Content Declaration

The following table provides a summary of the materials included in Holcim ready-mix concrete and their relative
composition by weight.

@
o
=)
où
c
©
5
2
É
©
a
©
Q
>
©
5
D
©
Le
[u

General purpose cement 5-21%
Aggregate 67-84%
Supplementary cementitious materials 0-11%
Water 11.6-12%
Admixtures 0.01-0.02%

Holcim Ready-mix concrete is classified as Non-Dangerous Goods according to the Australian Code for the Transport
of Dangerous Goods by Road and Rail. The safety data sheet for pre-mixed concrete lists all associated hazard
phrases.

The gross weight of this declared material makes up a minimum of 99% of the products covered by this EPD.

Packagin

| gIng Default background data from LCA databases was used
Holcim ready-mix concrete is delivered in bulk with no to model the above co-products:
packaging.

° Fly ash: AusLCI process for fly ash treats it as a
Recycled Material waste material and only includes transport

BS EN 16757:2017 specifically lists the following Impacts.

materials relevan h | e Ground granulated blast furnace slag: the
aterials relevant to the study as co-products AusLCI process for slag is allocated based on

economic value, as the product has a significant
economic value at the point of collection.

°  Flyash: e  Silica fume: the ecoinvent process for silica
e Ground granulated blast furnace slag; and fume treat it as a waste material and only
°  Silica fume includes transport impacts.

The allocation approach of the AusLCI LCA database
As such, the above materials are considered as co- was adopted as a default for secondary data and
products of their production process and the impacts for processes (e.g. secondary fuel in cement production).
their production process are allocated according to PCR The AusLCI dataset conforms to EN 15804 when
2019:14 Construction Products and Construction applying allocation to its various processes and sub-
Services (co-produced goods, multi-output allocation). processes.

ViroDecs'" EPD | Holcim 12
Environmental Performance

The environmental impacts considered in this EPD are listed in the table below. All further tables from this point will

contain abbreviation only.

@
©
=
œ
=
Lu
©

£
Lu
©

(su
œ
L 4
=
©
=
=
©

_
>
€

Li

Impact Category Abbreviation Measurement Unit

Potential Environmental Impacts
Total global warming potential

Global warming potential (fossil)

Global warming potential (biogenic)
Global warming potential (land use/ land transformation)
Ozone depletion potential

Acidification potential

Eutrophication — aquatic freshwater
Eutrophication — aquatic freshwater
Eutrophication — aquatic marine
Eutrophication — terrestrial
Photochemical ozone creation potential
Abiotic depletion potential (elements)
Abiotic depletion potential (fossil fuels)
Water Depletion Potential

Resource use

Use of renewable primary energy excluding renewable primary

energy resources used as raw materials

Use of renewable primary energy resources used as raw
materials

Total use of renewable primary energy resources (primary
energy and primary energy resources used as raw materials)
Use of non-renewable primary energy excluding non-
renewable primary energy resources used as raw materials

Use of non-renewable primary energy resources used as raw
materials

Total use of non-renewable primary energy resources (primary

energy and primary energy resources used as raw materials)
Use of secondary material

Use of renewable secondary fuels
Use of non-renewable secondary fuels

Use of net fresh water

ViroDecs'" EPD | Holcim

GWPT
GWPF
GWPB
GWPL
ODP
AP
EP - freshwater
EP - freshwater
EP - marine
EP -— terrestrial
POCP
ADPE
ADPF
WDP

PERE

PERM

PERT

PENRE

PENRM

PENRT

SM
RSF
NRSF
FW

kg CO» equivalents (GWP100
kg CO» equivalents
kg CO» equivalents
kg CO» equivalents (GWP100

GWP100

( )
( )
(GWP100)
( )
kg CFC 11 equivalents
mol H+ eq.
kg PO. equivalents
kg P equivalent
kg N equivalent
mol N equlivalent
kg NMVOC equivalents
kg Sb equivalents
MJ net calorific value

m equivalent deprived

MY, net calorific value
MY, net calorific value
MY, net calorific value
MY, net calorific value
MY, net calorific value

MY, net calorific value

kg
MY, net calorific value
MY, net calorific value

m°

13
Impact Category Abbreviation Measurement Unit

Waste categories and Output flows

@
©
=
œ
=
Lu
©
£
Lu
©
(su
œ
ne
=
©
=
=
©
È
>
€
Li

Hazardous waste disposed HWD Kg
Non-hazardous waste disposed NHWD kg
Radioactive waste disposed/stored RWD kg
Components for reuse CFR kg

Materials for recycling MER Kg

Materials for energy recovery MFEE Kg

Exported energy EE -e MJ per energy carrier
Exported energy, thermal EE -t MJ per energy carrier
Additional environmental impacts

Particulate matter PM disease incidence
lonising radiation - human health IRP kBq U-235 eq
Eco-toxicity (freshwater) ETP-fw CTUe

Human toxicity potential - cancer effects HTP-c CTUR

Human toxicity potential - non cancer effects HTP-nc CTUR

Soil quality SQP dimensionless

ViroDecs'" EPD | Holcim 14
Queensland — Brisbane — Plungie General Supply
Primary indicators - 1m° of ViroDecs" ready-mix concrete

PRIMARY EP -
ENVIRONMENTAL GWPT GWPL freshwater
INDICATORS

Strength Mix Code kg CO2 kg CO2 kg CO2 kg CO2 kg CFC mol H+ kg PO43-
(MPa) eq. eq. eq. eq. 11 eq. eq. eq.
492 492 0.32 2.51E-03 7.41E-06  1.91E+00 1.385E+00

BEN caso: vP25

ViroDecs'" EPD | Holcim

EP -
freshwater2

kg P eq.

8.23E-03

kg N eq.

5.90E-01

EP -
terrestrial

mol N eq.

6.79E+00

. Le =
kg

NMVOC kg Sb eq. MJ m3
eq.
1.68E+00 2.14E-04 1.59E+03  1.97E+03

15
Resource use parameters - 1m° of ViroDecsT" ready-mix concrete

PARAMETERS
DESCRIBING PERT PENRT
RESOURCE USE

Strength
(MPa)

CIE QA501VP25 493E+01  2.40E-03 493E+01 1.44E403 3.19E+02  1.76E+03 1.44E402 3.43E-05 O.00E+00  2.59E-01

Mix ECS MiNecv MIncv MiNecv MJNcv MIncv MyJNncv MINcv Minev

ViroDecs'" EPD | Holcim
Waste categories and output flows - 1m° of ViroDecs'" ready-mix concrete
WASTE CATEGORIES AND
OUTPUT FLOWS

= OEREs
Strength :

RON GAsoivP25  1.73E+02 1.71E+01 6.05E+00 0.00E+00 0.00E+00 0.00E+00 0.00E+00 0.00E+00

ViroDecs'" EPD | Holcim

17
Additional indicators 1m° of ViroDecsT" ready-mix concrete

ADDITIONAL ENVIRONMENTAL
EE = CES

Strength (MPa) Mix EC disease incidence kBq U-235 eq CTUe CTUh CTUh dimensionless

pue 1.20E-05 2.02E+02 2.84E +03 9.26E-08 3.28E-06 4.10E+02

ViroDecs'" EPD | Holcim

18
Other life cycle stages not included in
this EPD

r)
ri
D
œ
S
[9]
&
©
>
©
(
=
=
LD
©
£
Ld
O

While the LCA study and EPD only consider the cradle to gate environmental impacts of Holcim's ready-mix concrete,
practitioners using the EPD for the purpose of whole-of-life building studies or the functional comparison of different
building products on a whole-of-life basis will consider concrete’s other life cycle stages. Some of the environmental
impacts of benefits associated with other life cycle stages not included in this EPD are described in the following
sections.

Lifetime absorption of CO:

Carbonation is a natural process whereby concrete absorbs carbon dioxide (CO:) from the atmosphere through a
chemical reaction between the CO in the ambient air and hydration products within the concrete (CaOH:). Ready-mix
concrete can be subject to carbonation from the use stage onward (ï.e. after construction and curing). From a life cycle
impact accounting perspective, this process can also be referred to as ‘reabsorption’, since the CO, emitted during the
cement manufacturing process can be parily offset by the lifetime absorption of CO, therefore reducing the net CO:
emissions associated with concrete over its lifetime.

The carbonisation process is a commonly known process in building design and is typically taken into consideration by
engineers when specifying special-class concrete.

The total amount of CO, absorption during the life cycle of concrete is subject to a range of factors and varies over
time. The calculation has been standardised in the British and European Standard BS EN 16757:2017 Sustainability
of construction works — Environmental Product Declarations — Product Category Rules for concrete and concrete
elements. It is recommended that practitioners make use of this standard when conducting whole-of-life building
studies and if the building materials include substantial amounts of concrete. Please note that CO; absorption has not
been considered in this EPD and is not reflected in the EPD results tables.

End of life scenarios

BS EN 16757:2017 presents four end of life scenarios for concrete:

1. Disposal of concrete at a landfill site,

2. Reuse of recovered concrete elements in new construction works,

8. Use of concrete debris, e.g. In land restoration, or

4. Crushing/recycling of concrete:
a. Crushed concrete substitutes primary material without further processing, or
b. Substitution of natural aggregates in fresh concrete.

Scenarios 2, 3 and 4 can all result in benefits and loads outside the system boundary and thus should be considered
in a whole-of-life building study or when comparing concrete products on a functional basis in line with BS EN
16757:2017.

ViroDecs'" EPD | Holcim 19
References

Australasian EPD Programme. (2017). Guidance on the use of INA in EPDs.

Australasian EPD Programme. (2018). Guidance on the use of background LCI data.

References

Australasian EPD Programme (2019) Instructions of the Australasian EPD Programme V3.01.

Australian Life Cycle Inventory Database Initiative (AusLCI). (2018). Guidelines for Data Development for an
Australian Life Cycle Inventory Database, Data Standard.

British Standards Institution. (2019). Sustainability of construction works. Environmental product declarations. Core
rules for the product category of construction products, BS EN 15804:2012+A2:2019. British Standards Institution.

British Standards Institution. (2017). Sustainability of construction works — Environmental product declarations —
Product Category Rules for concrete and concrete elements, BS EN 16757:2017. British Standards Institution.

Ecoinvent Centre. (2019). Ecoinvent version 3 database. Zurich: ETH, Agroscope, EMPA, EPFL, PSI. Retrieved from
wWww.ecoinvent.orq.

EPD International. (2019). General Programme Instructions (GP) for the International EPD System V3.01. Retrieved
from www.envirodec.com.

EPD International. (2021). Product Category Rules for Construction Products and Construction Services, PCR2019:14
v1.11. Stockholm: EPD International.

ISO. (2006). Environmental labels and declarations — Type III environmental declarations — Principles and procedures,
ISO 14025:2006. Geneva: International Organization for Standardization.

ISO. (2006). Environmental management — Life cycle assessment — Principles and framework, ISO 14040:2006.
Geneva: International Organization for Standardization.

ISO. (2018). Environmental management. Life cycle assessment. Requirements and guidelines, ISO
14044:2006+A1:2018. Geneva: International Organization for Standardization.

AusLCI. (2018) AusLCI Database. Retrieved from AusLCI: www.auslei.com.au/

Man Yu, Thomes Wiedmann, Robert Crawford, Catriona Tait, ‘The Carbon Footprint of Australia’s Construction
Sector’, Procedia Engineering, Volume 180, 2017, Pages 211-220, ISSN 1877-7058,

(http;//www.sciencedirect.com/science/article/pi/S1877705817316879)

ViroDecs'" EPD | Holcim 20
Programme-related information and verification

Holcim (Australia) Pty Ltd
Level 7, 799 Pacific Highway
Declaration Owner Chatswood NSW 2067, Australia
Web: www.holcim.com.au
Phone: +61 2 9412 6600

Holcim

EPD Australasia Limited

315a Hardy Street Nelson nn | E P D ®
EPD Programme Operator ne New gear lasi AUSTRALASIA
eb: uuw.epdaustralasia.com ENVIRONMENTAL PRODUCT DECLARATION

Email: info@epd-australasia.com
Phone: +61 2 8005 8206

Holcim (Australia) Pty Ltd

Level 7, 799 Pacific Highway
EPD Produced by Chatswood NSW 2067, Australia
Web: www.holcim.com.au
Phone: +61 2 9412 6600

Holcim

Epsten Group

Suite 2600, 101 Marietta St NW, Atlanta,
EPD Process Certified by Georgia 30303, USA

Web: www.epstengroup.com

epstengroup

EPD Registration Number S-P-04662

Valid From 7 September 2022
Version 1
Valid Until 7 September 2027
Product category rules PCR 2019:14 Construction Products, Version 1.11, 2021-02-05
Product group classification UN CPC 54

Australia

Geographical Scope

Reference Year for Data 2017 Plant Data, 2022 Mix/Materials Data

CEN standard EN 15804:2012+A2:2019 served as the core PCR

Product category rules PCR 2019:14 Construction Products, Version 1.11, 2019-02-05

The Technical Committee of the International EPD® System. Chair:

PCR review was conducted b
y Massimo Marino. Contact via info@environdec.com

Independent third-party

verification of the declaration and EPD process certification
data, according to ISO EPD verification
14025:2006:

Epsten Group, Inc., Katherine McFeaters: .
EPD Process Certifed by Paouis Anfelas

Accredited by: A2LA, Certificate #3142.03

Procedure for follow-up of data
during EPD validity involves
third party verifier:

Programme-related information and verification:

The EPD owner has the sole ownership, liability, and responsibility for the EPD. EPDs within the same product
category but from different programmes may not be comparable. EPDs of construction products may not be
comparable if they do not comply with EN 15804.

ViroDecs'" EPD | Holcim 21
Holcim

This publication supersedes all previous literature on this subject. As the
specifications and details contained in this publication may change, please check
with Holcim Customer Service for confirmation of current issue. This publication
provides general information only and is no substitute for professional technical
engineering advice. Users must make their own determination as to the suitability of
this information or any Holcim product for their specific circumstances. Holcim

accepts no liability for any loss or damage resulting from their specific circumstances.

Holcim accepts no liability for an loss or damage resulting from any reliance on the
information provided in this publication. Performance. Passion.” and “ViroDecs” are

trademarks of Holcim (Australia) Pty Ltd.

© September 2022 Holcim (Australia) Pty Ltd ABN 87 732 297. All rights reserved.
This guide or any part of it may not be reproduced without prior written consent of
Holcim.

ViroDecs'" EPD | Holcim

22
