L — EPD°
"4 M O L C | M THE INTERNATIONAL EPD® SYSTEM
Pa. 4

Environmental Product Declaration

Under PCR 2019:14 Construction products (EN 15804:A2); Version 1.11; 2021-02-05

and c-PCR-001 Cement and Building Lime (EN 16908:2017) 2019-12-20

PRODUCT GROUP CLASSIFICATION: UN CPC 3744

in accordance with 15014025 and 15804:2012+A2:2019 for:

ECOPlanet

CEM III/A 42,5 N
IH/A 42,5 N/SRC

Program:

Program operator:
EPD registration number:

Issue date:
Update date:
EPD version

Validity date:

Geographical scope:

ECO PLATFORM

VERIFIED

The International EPD® System www.environdec.com

EPD International AB
REF: S-P-05185

2021-12-22
2023-11-23
3.1

2027-05-03

An EPD should provide current information and may be updated if conditions change.
The stated validity is therefore subject to the continued registration and publication at
www.environdec.com.

Global

HOLCIM ——— EPD

THE INTERNATIONAL EPD° SYSTEM

INTRODUCTION

This report contains the environmental performance of the production of the cement CEM H/A 42,5 N and III/A
42,5 N/SRC manufactured by Holcim España, S.A.U. in Spain. These products are part of the ECOPlanet range of
cements commercialized by the manufacturer. This Environmental Product Declaration (EPD) has been developed
using the Life Cycle Assessment (LCA) methodology. The environmental impact values calculated are referred to
one ton (1000 kg) of product ready to send to the customer.

This EPD has been conducted according to the International EPD® System regulation. This regulation is a system
for the international use of Type Ill Environmental Declarations, according to ISO 14025:2010. Not only the system
but also its applications are described in the General Programme Instructions (GPI 3.01). The report has been
made following the specifications given in the CEN standard EN 15804:2012+A2:2019 and the Product Category
Rule c-PCR-001 Cement and Building Lime EN16908:2017.

The assessed life cycle includes all the stages needed to manufacture the product and have it ready for the
customer at the exit gate of the factory.

The EPD owner has the sole ownership, liability, and responsibility for the EPD.

EPDs within the same product category but from different programs may not be comparable. EPDs of construction

products may not be comparable if they do not comply with EN 15804.

D D Om mm Re

2 Environmental Product Declaration of ECOPlanet CEM I/A 42,5 N and Ill/A 42,5 N/SRC
9 HOLCIM "— EPD

LE THE INTERNATIONAL EPD° SYSTEM

GENERAL INFORMATION

Programme-related information and verification

PROGRAMME

This Environmental Product Declaration has been developed under the programme:
The International EPD® System.

www.environdec.com Address: EPD International AB, Box 210 60, SE-100 31 Stockholm, Sweden.

COMPARABILITY

EPDs within the same product category but from different programmes may not be comparable. EPDs of

construction products may not be comparable if they do not comply with EN 15804.

The owner of this EPD, Holcim España, S.A.U. has the sole ownership, liability, and responsibility on this EDP.

VERIFICATION

ISO standard ISO 21930 and CEN standard EN 15804 serves as the core Product Category Rules (PCR).

Product category rule:

2019:14 Construction products (EN 15804:A2); Version 1.11; 2021-02-05 and c-PCR-001 Cement and Building Lime
(EN 16908:2017) 2019-12-20.

PCR review was conducted by:

The Technical Committee of the International EPD® System. See www.environdec.com/TC for a list of members.
Review chair: Claudia A. Peña, University of Concepcién, Chile. The review panel may be contacted via the

Secretariat www.environdec.com/contact.

Independent verification of the declaration and data, according to ISO 14025:2006:

X] External Internal
covering
EPD process certification X] EPD verification

Third party verifier:

Marcel Gômez

Accredited by:
Approved by The International EPD$ System Technical Committee, supported by the Secretariat.

Procedure for follow-up during EPD validity involves third part verifier:
X] Yes No

3 Environmental Product Declaration of ECOPlanet CEM I/A 42,5 N and Ill/A 42,5 N/SRC
HOLCIM

Contact information

“— EPD

THE INTERNATIONAL EPD° SYSTEM

EPD owner: . :
Holcim España, S.A.U.

Madrid, Spain
www.holcim.es

Tel + 91 213 31 00
marketing.spain@holcim.com

Avda. de Manoteras, 29, Edificio B, 12 Planta - 28050

LCA author: Solid Forest S.L.

Madrid, Spain
www.solidforest.com
info@solidforest.com

Plaza Santa Maria Soledad Torres Acosta 1, 42 - 28004

Programme operator: The International EPD® System

www.environdec.com
info@environdec.com

EPD International AB, Box 210 60, SE-100 31 Stockholm, Sweden.

Verifier: Marcel Gomez
info@marcelgomez.com

EPD version

This EPD is not sectorial and is version number 3.1.

Difference with previous versions:

Update of company name and logo.

Environmental Product Declaration of ECOPlanet CEM I/A 42,5 N and Ill/A 42,5 N/SRC
9 HOLCIM _ EPD

THE INTERNATIONAL EPD° SYSTEM

COMPANY INFORMATION

Product Provider

Holcim España,
S.A.U.

Avda. de Manoteras 20,
28050 — Madrid
Spain

Holcim España, S.A.U. owns five cement factories in Spain, with an installed capacity of more than seven million
tons per year, 19 concrete plants, one mortar plant, six terminals and one waste recovery plant, employing more

than 700 people.

The company has the first New Concrete and Mortars Research and Development Center, where specific products
that meet the specific needs of customers are developed, including the first laboratory with an exclusive area of
alternative fuels.

Holcim España is part of Holcim, a global leader in innovative and sustainable building solutions. Holcim is enabling
greener cities, smarter infrastructure and improving living standards around the world. With sustainability at the
core of its strategy Holcim is creating the path to become a net zero company, with its people and communities
at the heart of its success. The company is driving the circular economy as a world leader in recycling to build more
with less.

This declaration involves the activity ofthe plant located in Rambla Olivera s/n, 04140, Carboneras, Almeria, Spain.

Holcim España sustainable practices

Sustainability is at the core of our strategy. Holcim España will continue to stay at the forefront of green building
solutions. On our net-zero journey, we are decarbonizing our business end-to-end, from our operations and

products all the way to the built environment.

Decarbonizing our operations, with our Geocycle business, we are recycling materials at the end of their life
cycle as a source of alternative fuels.

5 Environmental Product Declaration of ECOPlanet CEM I/A 42,5 N and Ill/A 42,5 N/SRC
HOLCIM ——— EPD

THE INTERNATIONAL EPD° SYSTEM

Decarbonizing our products, we offer the world's broadest range of sustainable solutions, making low-carbon

construction possible at scale.

Decarbonizing our built environment, working for a net-zero built environment, we play an essential role

across a building’s entire life cycle.

We care about nature, we are working to make a positive and measurable impact on water and biodiversity, by

protecting and restoring the natural resources around us.

ECOPlanet is the world’s broadest global range of green cement, offering a low carbon footprint while delivering

equal to superior performance.

From our EcoPlanet Low-CO2 Cement to our ECOPact Low-CO2 Concrete, we offer the world's first global ranges
of low-carbon building materials. With our industry’s broadest formulation expertise, we adapt our solutions to

local needs making low-carbon building possible at scale.

Product-related or management system-
related certifications

Holcim España has an integrated management system certified according to ISO 9001:2015 “Quality

Management” and ISO 14001:2015 “Environmental Management” standards.

The greenhouse gases emissions inventory of Holcim España is verified every year according to the requirements
of the ISO 14064-1:2012 “Green House Gases” standard and is included in the Carbon Footprint National Registry
of the Ministerio para la Transiciôn Ecolégica y el Reto Demogräfico of Spain, obtaining the labels “Calculo”, for
calculated carbon footprint and “Reduzco” for achieving a substantial GHG emissions reduction in the last four

years.

6 Environmental Product Declaration of ECOPlanet CEM I/A 42,5 N and Ill/A 42,5 N/SRC
“— EPD

THE INTERNATIONAL EPD° SYSTEM

HOLCIM

PRODUCT INFORMATION

Product Identification

The system analysed in this Declaration comprises the life cycle of the production of the cements CEM II/A 42,5
N and Ill/A 42,5 N/SRC ECOPlanet manufactured by Holcim España in Spain.

Product Description

The Functional Unit of this LCA is one ton (1000 kg) of product ready to be sent to the customer. The products
included in this declaration are CEM II/A 42,5 N and INI/A 42,5 N/SRC ECOPlanet from Holcim España. These
Portland slag cements are normally used in ready-mix concrete plants for a large variety of concretes when a
normal compressive strength is required. Improve the performance of concrete in sulphate or sea water
environments (Spanish standard). Recommended for concretes with potential reactive aggregates. All

environmental impacts and use of resources, both direct and indirect, are reported to this unit.

This assessment has been done using the production data of 2020. The CEM HI/A 42,5 N and III/A 42,5 N/SRC

ECOPlanet cements and the life cycle assessment includes the production in the plant located in Carboneras, Spain.
The following composition and technical characteristics are valid for all products included in this declaration.

Composition

COMPONENT % by mass* Post-consumer Renewable
material, weight# | material, weight%
Clinker 59% 3% 0%
Blast furnace slag 39% 100% 0%
Minor additional constituents 2% 0% 0%
TOTAL 100% 41% 0%
*Including main components and additional constituents
Technical characteristics according to UNE-EN 197-1
Mechanical and physical properties Amount Unit
Compressive strength 2 days > 10 MPa
Compressive strength 28 days > 42.5 and < 62.5 MPa
Initial setting time > 60 min
Soundness < 10 mm

During the life cycle of the product any hazardous substance listed in the “Candidate List of Substances of Very
High Concern (SVHOC) for authorization” has not been used in a percentage higher than 0,1% of the weight of the
product.

7 Environmental Product Declaration of ECOPlanet CEM I/A 42,5 N and Ill/A 42,5 N/SRC
HOLCIM _— EPD

THE INTERNATIONAL EPD° SYSTEM

LCA INFORMATION

Declared Unit

This EPD represents the environmental impacts of one ton (1000 kg) of product ready to send to customers. The
products included in this declaration are CEM IH/A 42,5 N and IlI/A 42,5 N/SRC ECOPlanet from Holcim España.

A reference service life is not relevant due to this cradle-to-gate boundary conditions.

System boundaries

The LCA has a boundary “from cradle to gate”, being the end of the life cycle the exit gate of the cement factory,
covering the modules A1 to A3 (product stage).

This EPD covers all product stages from “cradle to gate” (modules A1-A3), since the product fulfils allthe conditions
required by EN 15084:2012+A2:2019 regarding the exclusion of modules B1 to D (the product is physically
integrated with other products during installation so they cannot be physically separated at the end of life, and
the product is no longer identified at the end of life as a result of a physical-chemical transformation process, and
the product does not contain biogenic carbon). This means that all processes up to the output gate of the
manufacturer are included, from quarry works and components manufacturing, to transports of materials and
fuels, factory process and final preparation. All direct and indirect environmental impacts have been calculated
and are reported in this document.

Holcim España has a complete control over all the processes within the factory and the quarry of main raw
materials.

The only processes that are not controlled directly by the company are the production of main fuels, the transport
of the raw materials, and minor inputs excluded according to the cut-off rules.

The environmental impacts related to the extraction and
production of fuels, as well as the indirect impacts related
to the production of electricity are also included in the
environmental impacts calculation. The national electricity

mix for Spain has been used.

A simplified model of the process of cement manufacturing
is described in the following diagrams, enumerating the
main activities included in the system boundaries. The
process andinstallations are also linked to the phases ofthe
product life cycle (A1-A3).

8 Environmental Product Declaration of ECOPlanet CEM I/A 42,5 N and Ill/A 42,5 N/SRC
“— EPD

In the A1 module the components and materials are
extracted in a quarry or manufactured in a third-
party location (ie. manufacture of fuels and blast

furnace slag). Raw materials that are not produced

14 THE INTERNATIONAL EPD® SYSTEM
Construction Resource
Product stage process Use stage End of life stage recovery
stage stage
S
C
[6]
©
[en
D
S £
S œ = £
£ a [0] © ©
> u = a = ©
© G > 3 (] ra
5 ÿ PS5 |: el >
o o <= € 2 TG 5 ‘ü oo]
= E + © = — a >
œ £ c o] CE ] 5 ra e]
5 E £ É SES |sl|sE 8 $
s|S5|1S8|1S81S ë s|s|Ss|Ss|15|3|315s œ
Ê à & a E ü = 0 2 & G 6 o 2 8 o
5 a D + œ S = no no a £ © o
z £ £ _ a o@ £ © © = ro] ro] © es u S. 5
© ü & g © a ü © © © [OS OS © g œ © &
œ = Z = @] D Z œ œ œ (e] (e] Q = = A œ
Module A1 A2 A3 B3 B4 | B5 | B6 B7 | C1 C2 C3 C4 D
Modules x | x | x ND | ND | ND | ND | ND | ND | ND | ND | ND ND
declared
Geography | GLO | GLO | GLO -
Specific data >95% GWP :
used
Variations - | és than 10% -
products
Variations - 1 site. L
sites No variations.

Product Stage

in the plant are transported to the plant by ship and
truck (A2 module). In the manufacturing stage (A3),
the components of the clinker are heated and once

the clinker is produced it is mixed with the additions

and crushed to produce the final cement.

There is no packaging as this product is marketed in
bulk.

Quarry operation Internal Transport Production
ER — Tr? …
Manufacturing of other raw Transport of purchased De o # Wa sd.
materials materials % J*
> S
8 Ds 9.)
AI A2 A3
Raw Materials Supply Transport Manufacturing

The scenarios included are currently in use and are representative for one of the most probable alternatives.

Technical Information

Calculation methodology

This EPD represents Type III Environmental Declarations according to ISO 14025 2010. The inherent Life Cycle
Assessment (LCA) has been developed according to ISO 14040 and ISO 14044 International Standards, and
following the International EPD System General Programme Instruction (GPI 3.01), the PCR 2019:14 Construction
products (EN 15804:A2); Version 1.11; 2021-02-05 and c-PCR-001 Cement and Building Lime (EN 16908:2017)

2019-12-20.

Environmental Product Declaration of ECOPlanet CEM I/A 42,5 N and Ill/A 42,5 N/SRC
9 HOLCIM "— EPD

LE THE INTERNATIONAL EPD° SYSTEM

Version 3.12 of software Air.e LCA" with Ecoinvent"" 3.7.1 database has been used for LCA modelling and impacts

calculations.

The following characterization models have been used:

Impact Model Unit

Baseline model of 100 years of the IPCC

Global Warming Potential (GWP Total) (based on IPCC 2013)

kg of CO2 equivalent

Baseline model of 100 years of the IPCC

Global Warming Potential (GWP Fossil) (based on IPCC 2013)

kg of CO2 equivalent

Baseline model of 100 years of the IPCC

Global Warming Potential (GWP Biogenic) (based on IPCC 2013)

kg of CO2 equivalent

Baseline model of 100 years of the IPCC

(based on IPCC 2013) kg of CO2 equivalent

Global Warming Potential (GWP LULUC)

Steady-state ODPs as in (WMO 2014 +

. . kg of CFC11 equivalent
integrations)

Ozone depletion

Accumulated Exceedance (Seppälä et al.

2006, Posch et al, 2008) mol of H+ equivalent

Acidification

EUTREN, Struijs et al., 2009b, as

-3 .
implemented in ReCiPe kg of PO4” equivalent

Eutrophication fresh water

EUTREN, Struijs et al., 2009b, as

implemented in ReCiPe kg of P equivalent

Eutrophication fresh water

EUTREN, Struijs et al., 2009b, as

implemented in ReCiPe kg of N equivalent

Eutrophication marine water

Accumulated Exceedance (Seppälä et al.

2006, Posch et al, 2008) mol of N equivalent

Eutrophication terrestrial

LOTOS-EUROS model (Van Zelm et al, 2008)

as implemented in ReCiPe 2008 kg of NMVOC equivalent

Photochemical ozone creation

CML 2002 (Guinée et al., 2002) and van

Oers et al. 2002 kg of Sb equivalent

Depletion of abiotic resources (elements)*

CML 2002 (Guinée et al., 2002) and van

Oers et al. 2002 M] net calorific value

Depletion of abiotic resources (fossil)*

Available WAter REmaining (AWARE) as

3 .
recommended by UNEP, 2016 m' world equivalent

Water scarcity*

*The result of this environmental impact indicator shall be used with care as the uncertainties on these results are high

or as there is limited experience with the indicator.

All processes related to the product have been included in the assessment.

According to EN 15804:2012+A2:2019 and EN 16908:2017, some components with less than 1% impact or use of

co-products with no significant economic value have been excluded from the assessment.

All transports of components have been included in the LCA, considering real loads and distances travelled by
materials used from January 2020 to December 2020. Main means of transport have been included for fuel

purchases and external raw materials. Operation in port has also been excluded.
Road distances calculated using Google Maps. Maritime distances calculated using MarineTraffic Voyage Planner.

The allocation was avoided when possible. Allocation was only used for the verified direct emissions ofthe furnace,

where the manufactured clinker can be later used to produce different cements.

10 Environmental Product Declaration of ECOPlanet CEM I/A 42,5 N and Ill/A 42,5 N/SRC
HOLCIM ——— EPD

THE INTERNATIONAL EPD° SYSTEM

Cut-off rules: more than 99% of the materials and energy consumption have been included. Capital equipment

production and maintenance, as well as employee transports have been excluded.
The analysed product is representative for its manufacturing plant.
The recycled components are considered from the sorting and processing plant of the recovered materials.

The Polluter Payer Principle and the Modularity Principle had been followed.

Emissions Factors and Tools

The emission factors and environmental impacts of the elements in the life cycles that are not controlled by
Holcim, or direct emissions that has not measured or calculated, come from Ecoinvent database, version 3.7.1,

using the cut-off criteria of that database.

The LCA has been carried out using the software tools Air.e LCA v3.12.

Data quality

According to the environmental footprint product category rules quality data criteria, and considering that the
data used for the processes is representative of the geography scope declared, that there was no need to
significantly modify technical aspects and that the data is from the last complete year, and considering that the
direct emissions of the manufacturing plant are third-party verified and included in the PRTR (Spanish National
Emissions and Contaminant Sources Registry) and specifically the GHG emissions are included in the EU Emissions

Trade System, the data quality is considered as high.

11 Environmental Product Declaration of ECOPlanet CEM I/A 42,5 N and Ill/A 42,5 N/SRC
HOLCIM

“— EPD

THE INTERNATIONAL EPD° SYSTEM

ENVIRONMENTAL PERFORMANCE

In the following tables, the environmental performance of the declared unit “one ton (1000 kg) of cement CEM

I/A 42,5 N produced by Holcim España and ready to send to customer” is presented totalized and for every
stage of the life cycle. The results are also valid for “one ton (1000 kg) of cement III/A 42,5 N/SRC ECOPIlanet
produced by Holcim España and ready to send to customer”. The estimated impact results are only relative

statements which do not indicate the end points of the impact categories, exceeding threshold values, safety

margins or risks.

Potential Environmental Impact

(m3 equivalent)

A1 A2 A3 Total
«À Total 20.19 10.87 459.28 490.34*
C!
Global Warming Potential Fossil 20.17 10.86 459.19 490.22**
(GWP100)
(kg of CO equivalent) Biogenic 0.02 <0.01 0.10 0.12
LULUC <0.01 <0.01 <0.01 <0.01
Ozone depletion
5 (kg of CFC11 equivalent) 2.37e-5 2.35e-6 1.79e-6 2.79e-5
@ Acidification
(mol of H+ equivalent) 0.19 0.19 0.80 1-17
Eutrophication fresh water

LR (kg of PO4® equivalent) 1.77e-2 1.69e-3 2.94e-2 4.88e-2
Eutrophication fresh water

mn (kg of P equivalent) 5.75e-3 5.52e-4 9.58e-3 1.59e-2
Eutrophication marine water

mn . 2.89e-2 4.28e-2 3.43e-1 4.15e-1
(kg of N equivalent)

LR Eutrophication terrestrial 031 0.48 3.76 4,55
(mol of N equivalent) ° ° ° :
Photochemical ozone creation

(Ce (kg of NMVOC equivalent) 0.11 0.13 0.92 1.16
Depletion of abiotic resources

-# (elements) 1.01e-4 2.41e-5 2.23e-4 3.48e-4
(kg of Sb equivalent)

Depletion of abiotic resources
(fossil) 1.44e+3 1.53e+2 1.86e+2 2.17e+3
(MJ net calorific value)
Water scarcity
voue 7.04 0.85 7.94 15.83

*Net Emissions. Gross emissions (including secondary fuels) = 533.88 kg CO,e

+*4Net Emissions. Gross emissions (including secondary fuels) = 533.72 kg CO:e

12

Environmental Product Declaration of ECOPlanet CEM I/A 42,5 N and Ill/A 42,5 N/SRC

HOLCIM

Use of resources

“— EPD

THE INTERNATIONAL EPD° SYSTEM

dd,
ee = TOTAL A1-A3
PIN
I
Use in plant of RENEWABLE primary energy excluding renewable primary energy resources 1.21e+03
used as raw materials "27e
Use in plant of RENEWABLE primary energy resources used as raw materials <0.01
Total use of RENEWABLE primary energy resources (primary energy and primary energy 1.21e+03
resources used as raw materials) “1e
Data in M, net calorific value
TOTAL A1-A3
Direct use in plant of NON- RENEWABLE primary energy excluding non- renewable primary 2.08e+03
energy resources used as raw materials :
Use in plant of NON-RENEWABLE primary energy resources used as raw materials <0.01
Total use of NON-RENEWABLE primary energy resources (primary energy and primary energy 2.08e+03
resources used as raw materials) 08e
Data in M, net calorific value
n_ hP TOTAL A1-A3
Use of secondary material 4.10+02
Data in kg
SAS TOTAL A1-A3
Use of net fresh water 0.23

Data in m3

13 Environmental Product Declaration of ECOPlanet CEM I/A 42,5 N and Ill/A 42,5 N/SRC

HOLCIM ——— EPD

THE INTERNATIONAL EPD° SYSTEM

Additional environmental information

Additional mandatory environmental impacts

Results per functional unit
Indicator Unit Tot. A1-A3
GWP-GHG* Kg CO eq. 533.88

* The indicator includes all greenhouse gases included in GWP-total but excludes biogenic carbon dioxide uptake and
emissions and biogenic carbon stored in the product. This indicator is thus almost equal to the GWP indicator originally
defined in EN 15804:2012+A1:2013. Gross emissions (including secondary fuels).

Waste production

Results per functional unit
Indicator Unit Tot. A1-A3
Hazardous waste disposed Kg <0.01
Non-hazardous waste disposed Kg 1.54
Radioactive waste disposed Kg <0.01
Output flows
Results per functional unit
Indicator Unit Tot. A1-A3
Components for re-use (CRU) Kg 0
Material for recycling (MFR) Kg 0
Materials for energy recovery (MER) Kg 0
Exported electrical energy (EEE) M] 0
Exported thermal energy (ETE) M] 0

Information on biogenic carbon content

Results per functional unit
Biogenic carbon content Unit Quantity
Biogenic carbon content in product Kg C (e)
Biogenic carbon content in packaging Kg C (e)

14 Environmental Product Declaration of ECOPlanet CEM I/A 42,5 N and Ill/A 42,5 N/SRC
HOLCIM ——— EPD

THE INTERNATIONAL EPD° SYSTEM

REFERENCES

This declaration has been developed according to the General Programme Instructions of the International EPD®

System. Version 3.01.

PCR 2019:14 Construction products (EN 15804:2012+A2:2019).

c-PCR-001 Cement and Building Lime (EN 16908:2017).

ISO 14040:2006 Environmental management - Life Cycle Assessment - Principles and framework.

ISO 14044:2006 Environmental management - Life Cycle Assessment - Requirements and guidelines.

LCA Report: Life Cycle Inventory of CEM I/A 42,5 N and II/A 42,5 N/SRC ECOplanet by Holcim España, S.A.U.
Software: Air.e LCA rev. 3.12 (www.solidforest.com).

Main database: Ecoinvent 3.7.1 (www.ecoinvent.org).

Geographical scope of the EPD: Global.

Note: Environmental declarations published within the same product category, though originating from different

programs, may not be comparable.

Y’HOLCIM

15 Environmental Product Declaration of ECOPlanet CEM I/A 42,5 N and Ill/A 42,5 N/SRC
