ECO PLATFORM

HOLCIM Se) ee EPD'

VERLFIED

EPD Doroport®TB — Holcim Romania

ISO 14020; ISO 14025; ISO 14040; ISO 14044; EN 15804; EN 16908; ISO 21930
Edition 1; Revision 2: April 2025
Environmental Product Declaration in accordance with ISO 14025:2006 and EN 15804:2012+A2:2019/AC:2021

1. Programme information

Programme Operator: The International EPDeSystem
EPD International AB

Box 210 60

SE-100 31 Stockholm

Sweden

www.environdec.com
info@environdec.com
Declaration Holder Holcim (Romania) SA
no.46D-46E-48 Pipera street,
OREGON PARK: building B, floor 6, District 2, RO 020308
Bucharest, Romania

Phone: +4021 2317708/09
Contact person: Georgiana Vatui

Email:
alexandrageorgiana.vatui@holcim.com
Company identification information:
Trade Register No: J2002000399403
VAT number: RO 12253732

LCA consultant ERM, exchequer court, 33 St Mary Axe
London EC3A 8AA, United Kingdom
WWw.erm.com

Contact person: Emma Green

Email: emma.green@erm.com
AUTO EUCHNUNTUTT, S-P-06631

Publication Date 2022-08-18
Version Date 2025-04-11
Valid Until 2027-08-17

© 2022 Holcim (Romania) SA 1
info@environdec.com

The EPD owner has the sole ownership, liability, and responsibility for the EPD. EPDs within the same product category
but from different programmes may not be comparable. EPDs of construction products may not be comparable if they do
not comply with EN 15804.

EPDSs within the same product category but registered in different EPD programmes, or not compliant with EN 15804, may not be
comparable. For two EPDs to be comparable, they must be based on the same PCR (including the same version number) or be based on
fully-aligned PCRSs or versions of PCRSs; cover products with identical functions, technical performances and use (e.g. identical
declared/functional units); have equivalent system boundaries and descriptions of data; apply equivalent data quality requirements, methods
of data collection, and allocation methods; apply identical cut-off rules and impact assessment methods (including the same version of
characterisation factors); have equivalent content declarations; and be valid at the time of comparison. For further information about
comparability, see EN 15804 and ISO 14025

2. Company Information

This cradle-to gate environmental product declaration is for 1 tonne of average Doroport®TB special road
binder production from the locations fully owned and operated by Holcim in Romania, as follows:

Alesd Cement Plant Pitesti Road Binder Plant
Street Viitorului, No.2, Postal code 417022 Postal code 110138, Str. Depozitelor 10,
Chistag Village, Bihor County, Romania Pitesti, Romania

Holcim Romania is the study commissioner and EPD owner.

To respect the principles of Sustainability strategy

sustainable development, the company Holcim Romania sustainability strategy is
implemented, maintained and continuously governed by Holcim Group commitment of
improves an effective integrated management BECoIMRPe EAN ere)
system, in accordance with the applicable peche tie tansier dau ie Lt
reference standards: SR EN ISO 9001:2015, SR Li CE ci dE ce à

EN ISO 14001:2015, SR ISO 45001 :2023: BES cet eo ini ginele Les te
6001 :2022. yc'ng-

Doroport ÊTB is one of Holcim Romania’s hydraulic road binders. Further information is publicly available
on https://econcept.holcim.ro/sustenabilitate

© 2022 Holcim (Romania) SA 1
EPD DOROPORT © TB Road Binder — Holcim Romania

3. Product Information

This EPD provides information concerning Doroport@TB special road binder produced by Holcim in
Romania as detailed in Table 1.

DOROPORTÉTB is Holcim Romania range of hydraulic road binders consisting of a combination of
hydraulic compounds, Portland cement clinker and other minor constituents, in accordance with SR EN
13282-1: 2013.

The geographical scope of this EPD is Romanian.

3.1 Technical Specification of Product

DOROPORTSTB is used to stabilize the materials used in the
execution of road layers, especially the foundation layers and the
base layers that are part of the rigid and non-rigid road systems.

DOROPORTSTB road binder range includes several products
depending on the strength class (SR EN 13282-1: 2013):

o _ DOROPORTETB 15 (type HRB E2)
o _ DOROPORTETB 25 (type HRB E3)
o_ DOROPORTETB 35 (type HRB Ed)

As given by SR EN 13282-1: 2013 Hydraulic road binders: Rapid
hardening hydraulic road binders - Composition, specifications and
conformity criteria.

e Execution of foundation layers and base layers in the
composition of non-rigid and rigid road systems

e Execution of bituminous coatings through cold recycling
technology, Expanding existing foundations, construction of
platforms and parking spaces

e  Strengthen parking lanes, framing lanes and sidewalks

Execution of clothing for local roads or low-traffic streets as
well as bituminous coatings using cold recycling technology.
Table 1: Technical specification and usage

© 2025 Holcim (Romania) SA 2
EPD DOROPORT © TB Road Binder — Holcim Romania

3.2 Content declaration

72 — 74%

20%

DVDa e 6-8%

ed cla <1%

Table 2: DOROPORTTB composition

The product composition for the product is provided in the Tables below. The binder does not meet the
criteria for PBT (Persistent, Bio-accumulative and Toxic) or vPvV (very Persistent and very Bio-
accumulative) in accordance with Annex XIII of Regulation (EC) No. 1907/2006 of the European
Parliament and of the Council on the Registration, Evaluation, Authorisation and Restriction of Chemicals
(REACH). Furthermore, cement/cementitious binders are a mixture, and it is exempted from REACH
registration.

3.3 Manufacturing Process
The main steps in the binder manufacturing process are as follows, andillustrated in Figure 1:
Quarrying and raw material preparation
Clinker production

Cement grinding and distribution.
Binder production

Figure 1: Process flow diagram

CEM - cement
Gt -Quickime
FA — Fiy Ash

BP-B8ypass dust

Quarrying
Natural raw materials used for the clinker manufacture are calcareous materials like limestone or marl,
and argillaceous materials like clay. These materials are extracted using drilling and blasting techniques.

© 2025 Holcim (Romania) SA 3
rusher
The quarried material is then reduced in size by compression and / or impact in various mechanical
crushers. Crushed rock is reduced in size from 120 cm to between 1.2 and 8 ca. Drying of raw material
may also be necessary for efficient crushing and pre-blending.

nveyor
Raw material is then transported from the quarry to the plant using conveyors.

Mixing bed
The crushed limestone and clay are homogenized by stacking and reclaiming in a long-layered stockpile.
This material is then ready for milling and drying in the kiln.

Raw Mill

The raw materials are milled and dried in a vertical roller mill in Campulung Plant and in a horizontal ball
mill in the Alesd Plant. In the case of the vertical roller mill, heavy rollers are held over a rotating table,
and in the horizontal ball mill, balls are rolled over until the coarse material is milled fine enough to be
carried by air to a homogenizing silo.

Preheater

Cyclone preheaters enable the raw material of cement production to be preheated before entry into the
kiln. This increases the energy efficiency of the kiln as the material is about 20-40% calcined at the point
of entry into the kiln. Additionally, calciners are integrated in both plants kiln systems, further increasing
the efficiency of the process.

Kiln

The kiln is designed to maximise the efficiency of heat transfer from fuel burning to the raw material. In
the preheater tower the raw materials are heated rapidly to a temperature of about 1000°C, where the
limestone decarbonisation occurs. In the rotating kiln, the temperature reaches up to 2000°C. At this
high temperature, minerals fuse together to form predominantly calcium silicate crystals — cement
clinker.

Binder Pr ion

The cement is mixed with other minor constituents in the road binder plants of Holcim Romania. The
cement produced in Alesd is mixed with additional constituents on site and the cement produced at
Campulung is transported to Pitesti for mixing.

No packaging is associated with DOROPORTS8TEB. The products are delivered only in bulk, with cement
trucks.

3.4 Additional Information

More information about binders’ environmental stewardship and occupational health and safety
aspects are detailed within the SDS made publicly available on Holcim Romania portal
https://www.holcim.ro/ro/produse-si-servicii/produse . AI SDS have been developed by Holcim
Romania in compliance with the requirements of Regulation (EU) 2020/878 amending the annex Il of
Regulation (EC) No 1907/2006 of the European Parliament and of the Council on the Registration,
Evaluation, Authorisation and Restriction of Chemicals (REACH) and according to Regulation (EC) No
1272/2008 on the Classification, Labelling and Packaging of substances and mixtures (CLP).

© 2025 Holcim (Romania) SA 4
EPD DOROPORT © TB Road Binder — Holcim Romania

4. LCA Information

4.1 Goal of Study

The goal of this study was to generate an environmental profile of DOROPORTSTB binder produced and
delivered from the locations fully owned and operated by Holcim Romania, to better understand the
associated lifecycle environmental impacts and to allow a Type III EPD to be generated and made public
via the International EPD System.

4.2 Declared Unit

The declared unit of the EPD is 1 tonne of DOROPORTSTB produced and delivered from the locations
fully owned and operated by Holcim Romania. This EPD is established for the weighted average

product of theses manufacturing plants. The average is based on the mass of binder produced

at each plant.

4.3 System Boundary

System boundaries determine the unit processes to be included in the LCA study and which data
as “input” and/or “output” to/from the system can be omitted.

This EPD covers the cradle to gate stage (Aî to A3), because other life cycle stages are
dependent on scenarios and are better developed for specific building or construction

works.

System boundaries are according to the modular approach and the cradle to gate stage is divided

into the upstream (A1) and core (A2 and A3) phases, as outlined in Figure 2. Life cycle stage that
are not covered by the EPD are indicated as MND (Module Not Declared).

Life cycle Information modules
stages a) Cradle to gate with b} Cradle to gate <) Cradle to grave and f) Construction service
module C1-C4 and with module C1-C4, module D EPD: Cradle to gate with
module D !! module D and optional modules At-A5 and
modules optional modules

tional juil
A1-A3 Product Mandatory Mandatory Mandatory Mandatony
stage
A3) Manufacturing
defaut scenario can be

A4-A5 Optional for goods Mandatory Mandatory
Construction
A5) Construction installation
defined
B Use stage — Optional Mandatory Optional
B5) Refurbishment
B8) Operational energy use
B7) Operational water use

C End of life Mandatory Mandatory Optional
stage

D Benefits and D} Reuse, recovery, recychng, Mandatory Mandatory

ioads beyond potential

the system

boundai

Deciared or functional unit

inclusion of reference service life (RSL) Optional Mandatory if any module | Mandatory
in B is included

Figure 2: Modules included in the DOROPORT®TB LCA

Mandatory for services

process stage (see alternative f}

Recommended if a

© 2025 Holcim (Romania) SA 5
EPD DOROPORT © TB Road Binder — Holcim Romania
4.4 Data sources and quality

The geographical system boundary of the LCA is Romania. All processes are valid for the production sites
in Romania. The two cement plants account for 100% of total DOROPORTSTB produced by Holcim in
Romania.

All material flows of the processes are based on company and site-specific data gathered for one
year of operation, for the period 1st January 2021 — 30 September 2021.

Modelling of the life cycle of Holcim Romania DOROPORTSTB binder was performed using SimaPro v.9.1
LCA software from PRé.

All relevant background LCI datasets are taken from the Ecolnvent database v3.8 (cut-off)
released in 2021.

The foreground data has been collected on site and validated based on mass balances. The
background data is based on reviewed data from life cycle inventories. As all datasets are
validated, the data quality for the entire study can be judged as very good.

4.5 Allocation

The foreground data has been collected on site and validated based on mass balances. The allocation is
performed according to the basic rules from EN15804:2012+A2:2019. As no co-products are produced, the
flow of materials and energy and the associated release of substances and energy into the environment is
therefore related exclusively to the binder produced.

All data is included based on measured data for each plant. To ensure high representativeness
for calculation of the DOROPORTSTB this specific data has been weighted based on the production
mass of each plant, as follows:

31,448.26 30,324.29

61,772.55

51% 49%

Table 3: Holcim Romania - DOROPORT®TB Production

4.6 Cut-off Criteria and assumptions

In the process of building an LCI it is typical to exclude items considered to have a negjligible (aka relatively
inconsequential or immaterial) contribution to results. To do this in a consistent and robust manner there
must be confidence that the exclusion is fair and reasonable. To this end, cut-off criteria were defined in
this study, which allow items to be neglected if they meet the criteria. In accordance with EN15804,
exclusions could be made if they were expected to be within the below criteria and the total neglected input
flows per module do not exceed 5% of energy usage and mass:

+ Mass: when using mass as a cut-off criterion, it is appropriate to require the inclusion in the study of
all inputs that cumulatively contribute more than a defined percentage to the mass input of the product
system being modelled.

© 2025 Holcim (Romania) SA 6
EPD DOROPORT © TB Road Binder — Holcim Romania

° Energy: similarly, an appropriate decision, when using energy as a criterion, is to require the inclusion
in the study of those inputs that cumulatively contribute more than a defined percentage of the product
system's energy inputs.

° __ Environmental significance: decisions on cut-off criteria should be made to include inputs that
contribute more than an additional defined amount of the estimated quantity of individual data of the
product system that are specially selected because of environmental relevance.

The production of the materials that have been excluded from the product system under study are listed in
Table 4. These materials are either waste derived or excluded due to their low economic value. While the
production of these materials is excluded the material masses are part of the calculation and they are
considered as secondary materials.

Material Considered as

Alternative Raw Material (slag / fly ash) Secondary Material
By-bass dust Secondary Material
Fly ash / acidic fly ash (ARSN) Secondary Material
Granulated blast furnace slag Secondary Material
Table 4: Secondary materials excluded from the product system

The clinker production process uses non-renewable secondary fuels (Table 6). According to the PCR,
secondary fuels are modelled to enter the studied system free of environmental loads. They are displayed
as a resource use and all emissions occurring during the production process are allocated to the produced
products.

Fuel Considered as

Mixed industrial waste Non-Renewable Secondary fuel
Petroleum sludges Non-Renewable Secondary fuel
Used / Waste oils Non-Renewable Secondary fuel
Other biomass Non-Renewable Secondary fuel
Sewage sludge Non-Renewable Secondary fuel
Fresh saw dust Non-Renewable Secondary fuel
Used tyres Non-Renewable Secondary fuel
Table 5: Secondary fuels excluded from the product system

In addition to the above, during the LCA several assumptions were made, which have been
documented below for transparency:

+ No waste is produced during the clinker production process.

e _ Thereis a difference between the mass of the raw meal consumed and the clinker produced which
is due to the water (remaining humidity of raw materials) that evaporates and mainly CO2that is
released from decarbonation.

4.7 Comparability

EPDs within the same product category but from different programmes may not be comparable.
EPDs of construction products may not be comparable if they do not comply with EN 15804.

© 2025 Holcim (Romania) SA 7
EPD DOROPORT © TB Road Binder — Holcim Romania

5. Environmental Performance

The environmental impacts are declared and reported using the parameters and units shown in
the Tables below. Baseline characterisation factors are taken from EF 8.0 methodology (dated November

2019)

The impact categories presented in the following table refer to 1 tonne of DOROPORT@TB
produced from the locations fully owned and operated by Holcim in Romania.

Parameter

GWP-total: Global Warming
Potential total!

GWP - GHG
GWP — Fossil: Global
Warming Potential fossil fuels

GWP-biogenic: Global
Warming Potential biogenic

GWP-luluc: Global Warming

Potential land use and land
use change?

ODP: Depletion potential of
the stratospheric ozone layer

AP: Acidification potential

EP-freshwater:
Eutrophication potential,
fraction of nutrients reaching
freshwater end compartment
(EP-freshwater)

EP-marine: Eutrophication
potential, fraction of nutrients
reaching marine end
compartment

EP-terrestrial: Eutrophication
potential, Accumulated
Exceedance

POCP: Formation potential of
tropospheric ozone

Parameters describing environmental impacts

Unit Aî A2 A3 A1-A3
kg CO: eq. 76.4 8.75 248 333.15
kg CO: eq. 75.3 8.62 248 331.9
kg COzeq. 76.5 8.72 248 333
kg CO2 eq. | -2,78E-02 | 2.02E-02 | -8.51E-02 | -9.27E-02

4.06E-03 | 5.45E-03 | 1.07E-02 2.02E-02

kg CO: eq.
kg CFC 11 _
ed. 1.74E-06 | 1.81E-06 | 4.84E-06 8.89E-06
mol H+ eq. 0.113 0.0444 0.386 0.543
kg P eq 1.80E-02 | 1.23E-03 | 7.78E-02 9.70E-02
kg N eq. 6.32E-02 | 1.42E-02 | 2.01E-01 2.78E-01
mol N eq. 0.267 0.154 0.781 1.20
kg NMVOC
ec. 0.196 0.0466 0.604 0.847

1 The total global warming potential (GWP-total) is the sum of

— GWP-fossil
— GWP-biogenic
— GWP-luluc

2Itis permitted to omit GWP-luluc as separate information if its contribution is < 5 % of GWP-total over the
declared modules excluding module D.

© 2025 Holcim (Romania) SA 8
EPD DOROPORT © TB Road Binder — Holcim Romania

ADP
Abiotic depletion potential fo kg Sb eq. 2.64E-05 | 2.48E-05 | 5.92E-05 1.10E-04
@ @ SO
ADP-fo Abiotic depletio MJ, net
or fossil reso calorific 399 132 1270 1801
pote a value
ne m$ world
QeD dailO DOIE a
denrivation-weiahted wate eq. 4.29 0.674 11.7 16.7
deprived
@ DTIO
a ele 0e D Q e O 2510 e
PER Renewable p a
energy used as energy ca MJ 22.6 3.64 113 139
primary reso ene MJ 1.37 0.558 4.66 6.59
@ e e0 a dalefla
My 28.9 4.19 118 146
DENRE. No able
D a SO eQû a d MJ
energy carie 498 135 1590 2223
BENE , able
D a eso ene MJ 0 0 0 0
@ e e0 a dalefla
P h OÏa enewabD
primary reso MJ 498 135 1590 2223
econda eria kg 346 0 0 346
! Renewab econda
: MJ 0.0872 0 0.281 0.368
h O e able
econdary fue MJ 0.129 0 0.416 0.545
a 0.744
ms
of net freshwater resource 0.151 0.02 0.573
kg 1.89E-03 | 1.17E-03 8.10E-03 1.12E-02

HWD: Hazardous
waste disposed

3 The abiotic depletion potential is calculated and declared in two different indicators:
— ADP -minerals&metals include all non-renewable, abiotic material resources (i.e. excepting
fossilresources);

— ADP-fossil include all fossil resources and includes uranium.

4 ultimate reserve model of the ADP- minerals & metals model

© 2025 Holcim (Romania) SA 9

EPD DOROPORT © TB Road Binder — Holcim Romania

Parameter

NHWD: Non-hazardous
waste disposed 0.871 10.1 3.19 14.2

RWD: Radioactive waste
disposal

1.76E-03 | 8.58E-04 7.75E-03 1.04E-02

Parameters describing outputs flows

CRU: Components for reuse

MR: Material for recycling

MER: Materials for energy
recovery

ÉËÉE: Exported energy,
electrical

EET: Exported energy,
thermal

© 2025 Holcim (Romania) SA 10
6. REFERENCES

Boulay et al (2017). The WULCA consensus characterization model for water scarcity footprint: assessing impacts of
water consumption bases on available water remaining (AWARE). Water Use in LCA, 23.

Centrum voor Milieuwetenschappen Leiden (CML) (2012). CML-IA baseline v4.1 / EU25 characterisation factors. CML,
Leiden.

PCR 2019_14 Construction Products (EN 15804+2)

Cement and Building Lime (EN 16908:2017) C-PCR-001 (To PCR 2019:14) Version: 2019-12-20

Ecoinvent (2017). Ecoinvent v3.4, Swiss Centre for Life Cycle Inventories. Available from www.ecoinvent.ch

Guo (2012). Life Cycle Assessment (LCA) of Light-Weight Eco-composites. Springer, Berlin

Huijbregts, Steinmann, Elshout, Stam, Verones, Vieira, Zijp, Hollander, van Zelm. ReCiPe 2016: a harmonizeld life cycle
impact assessment method at midpoint and endpoint level. International Journal of LCA, DOI 10.1007/s11367-016-
1246-Y.

ISO (2000), ISO 14020:2000, Environmental labels and declarations —- General principles

ISO (2004), ISO 8601:2004 Data elements and interchange formats — Information interchange — Representation of
dates and times

ISO (2006a), ISO 14025:2006, Environmental labels and declarations — Type Ill environmental declarations — Principles
and procedures

ISO (2006b), ISO 14040:2006, Environmental management — Life cycle assessment — Principles and framework ISO
(2006c)

ISO 14044: 2006, Environmental management — Life cycle assessment — Requirements and guidelines ISO (2013)

ISO/TS 14067:2013, Greenhouse gases — Carbon footprint of products — Requirements and guidelines for
quantification and communication

ISO (2014), ISO 14046:2014, Environmental management — Water footprint — Principles, requirements and guidelines

IPCC (2007). Working Group I Contribution to the IPCC Fourth Assessment Report Climate Change 2007: The Physical
Science Basis, Summary for Policymakers. Intergovernmental Panel on Climate Change, Geneva

IPCC (2006). 2006 IPCC Guidelines for National Greenhouse Gas Inventories, Volume 4: Agriculture, Forestry and
Other Land Use. IPCC, Geneva

JRC (2011). ILCD Handbook: recommendations for life cycle impact assessment in the European context. European
Commission Joint Research Centre Institute for Environment and Sustainability.
http://eplca.jrc.ec.europa.eu/?page id=86

Pre Consultants (2019). SimaPro v9. Pre Consultant, Amersfoort
Weidema BP, Bauer C, Hischier R, Mutel C, NemecekT, Reinhard J, Vandenbo C O, Wernet G (2013). Overview and

methodology: data quality guideline for the ecoinvent database version 3 (final). Swiss Centre for Life Cycle
Inventories: St Gallen

© 2025 Holcim (Romania) SA 11
