ECO PLATFORM

Y? HOLCIM SAR) = EPD'

VERIFIED

EPD Dorosol®- Holcim Romania

ISO 14020; ISO 14025; ISO 14040; ISO 14044; EN 15804; EN 16908; ISO 21930
Edition 1; Revision 2: April 2025
Environmental Product Declaration in accordance with ISO 14025:2006 and EN 15804:2012+A2:2019/AC:2021

1. Programme information

Programme Operator: The International EPDe System
EPD International AB

Box 210 60

SE-100 31 Stockholm
Sweden
www.environdec.com
info@environdec.com

Declaration Holder Holcim (Romania) SA

no.46D-46E-48 Pipera street,

OREGON PARK: building B, floor 6, District 2, RO 020308
Bucharest, Romania

Phone: +4021 2317708/09
Contact person: Georgiana Vatui
Email: alexandrageorgiana.vatui@holcim.com

Company identification information:
Trade Register No: J2002000399403
VAT number: RO 12253732

nn

LCA consultant ERM, exchequer court, 33 St Mary Axe,
London EC3A 8AA, United Kingdom
Www.erm.com

Contact person: Emma Green
Email'emma.green@erm.com

EPD:Registration number. Een TCyer:

Publication Date 2022-08-18
Version Date 2025-04-11
Valid Until 2027-08-17

© 2022 Holcim (Romania) SA

L
EPD DOROSOLS® Road Binder — Holcim Romania

Product group classification: UN CPC 3744 CEMENT

Product category rules (PCR): CEN Standard EN 15804:2012+A2:2019 served as the core
PCR. PCR 2019:14-c-PCR-001 c-PCR-001 Cement and building lime (EN 16908) (2022-05-
18)

PCR review was conducted by: The Technical Committee of the International EPD System.
Chair:
Massimo Marino. Contact via

Independent third-party verification of the declaration and data, according to ISO 14025:2006:
C1 EPD process certification X EPD verification

Third party verifier: Dr Hüdai Kara PhD
Approved by: The International EPDe System

Procedure for follow-up of data during EPD validity involves third party verifier:

[ Yes x No

The EPD owner has the sole ownership, liability, and responsibility for the EPD. EPDs within the same product category
but from different programmes may not be comparable. EPDs of construction products may not be comparable if they do
not comply with EN 15804.

EPDSs within the same product category but registered in different EPD programmes, or not compliant with EN 15804, may not be
comparable. For two EPDs to be comparable, they must be based on the same PCR (including the same version number) or be based on
fully-aligned PCRSs or versions of PCRSs; cover products with identical functions, technical performances and use (e.g. identical
declared/functional units); have equivalent system boundaries and descriptions of data; apply equivalent data quality requirements, methods
of data collection, and allocation methods; apply identical cut-off rules and impact assessment methods (including the same version of
characterisation factors); have equivalent content declarations; and be valid at the time of comparison. For further information about
comparability, see EN 15804 and ISO 14025.

2. Company Information

This cradle-to gate environmental product declaration is for 1 tonne of average Dorosol® special binder
production from the locations fully owned and operated by Holcim in Romania, as follows:

Alesd Cement Plant Pitesti Road Binder Plant
Street Viitorului, No.2, Postal code 417022 Postal code 110138, Str. Depozitelor 10,
Chistag Village, Bihor County, Romania Pitesti, Romania

Holcim Romania is the study commissioner and EPD owner.

To respect the principles of Sustainability strategy
sustainable development, the company Holcim Romania sustainability strategy is
implemented, maintained and continuously gevennes by ol Claus este ei
improves an effective integrated management becoming a NET ZERO company and
system, in accordance with the applicable spearheading the transition towards low-
reference standards: SR EN ISO 9001:2015, SR ROMEO

EN ISO 14001:2015, SR ISO 45001:2023: BES circular none from alternative fuels to
concrete recycling.
6001:2022.

Dorosol® is one of Holcim Romania’s hydraulic road binders. Further information is publicly available on
https://econcept.holcim.ro/sustenabilitate

© 2022 Holcim (Romania) SA 1
EPD DOROSOL® Binder — Holcim Romania

3. Product Information

This EPD provides information concerning Dorosol® special binder produced by Holcim in Romania as
detailed in Table 1.

DOROSOLS are Holcim Romania special binders for improving cohesive soils. produced as a
combination of hydraulic compounds, Portland cement clinker and quicklime, in accordance with the
technical specifications in force.

The geographical scope of this EPD is Romanian.

3.1 Technical Specification of Product

Table 1: Technical specification and usage

Details

For improving and stabilizing the cohesive soils used for the
construction of embankments, foundation layers and form layers in
geotechnical works and road construction.

The range of DOROSOLS special binders includes several
products, depending on their CaO content:

e  DOROSOL® C30
e  DOROSOLS C50
e  DOROSOLSF

Technical and As stipulated in the Technical Agreement
Functional

Characteristics

Identification

For special geotechnical works, civil works, and communication
Ways to:

e improve the soil with reduced mechanical strength (soil

Intended Application sensitive to humidity, compressible, swampy etc.)

e _stabilize embankments and slopes

e increase the bearing capacity of capping layers for road
construction

© 2025 Holcim (Romania) SA 2
EPD DOROSOL® Binder — Holcim Romania

3.2 Content declaration

53— 57%

10—11%

drated Lime 17-18%
Bypass 15 - 20%

Table 2: DOROSOL® composition

The product composition for the product is provided in the Tables below. The binder does not meet the
criteria for PBT (Persistent, Bio-accumulative and Toxic) or vPvV (very Persistent and very Bio-
accumulative) in accordance with Annex XIII of Regulation (EC) No. 1907/2006 of the European
Parliament and of the Council on the Registration, Evaluation, Authorisation and Restriction of Chemicals
(REACH). Furthermore, cement/cementitious binders are a mixture, and it is exempted from REACH
registration.

3.3 Manufacturing Process

The main steps in the binder manufacturing process are as follows, andillustrated in Figure 1:
Quarrying and raw material preparation

Clinker production

Cement grinding and distribution.
Binder production

Figure 1: Process flow diagram

CEM — cement
Qt -Quickirne
FA — Fiy Ash

BP-Bypass aust

© 2025 Holcim (Romania) SA 3
Quarrvyinqg
Natural raw materials used for the clinker manufacture are calcareous materials like limestone or marl,
and argillaceous materials like clay. These materials are extracted using drilling and blasting techniques.

rusher
The quarried material is then reduced in size by compression and / or impact in various mechanical
crushers. Crushed rock is reduced in size from 120 cm to between 1.2 and 8 ca. Drying of raw material
may also be necessary for efficient crushing and pre-blending.

nveyor
Raw material is then transported from the quarry to the plant using conveyors.

Mixing bed
The crushed limestone and clay is homogenized by stacking and reclaiming in a long layered stockpile.
This material is then ready for milling and drying in the kiln.

Raw Mill

The raw materials are milled and dried in a vertical roller mill in Campulung Plant and in a horizontal ball
mill in the Alesd Plant. In the case of the vertical roller mill, heavy rollers are held over a rotating table,
and in the horizontal ball mill, balls are rolled over until the coarse material is milled fine enough to be
carried by air to a homogenizing silo.

Preheater

Cyclone preheaters enable the raw material of cement production to be preheated before entry into the
kiln. This increases the energy efficiency of the kiln as the material is about 20-40% calcined at the point
of entry into the kiln. Additionally, calciners are integrated in both plants kiln systems, further increasing
the efficiency of the process.

Kiln

The kiln is designed to maximise the efficiency of heat transfer from fuel burning to the raw material. In
the preheater tower the raw materials are heated rapidly to a temperature of about 10000C, where the
limestone decarbonisation occurs. In the rotating kiln, the temperature reaches up to 20000C. At this
high temperature, minerals fuse together to form predominantly calcium silicate crystals — cement
clinker.

Binder Pr ion

The cement is mixed with other minor constituents in the road binder plants of Holcim Romania. The
cement produced in Alesd is mixed with additional constituents on site and the cement produced at
Campulung is transported to Pitesti for mixing.

No packaging is associated with Dorosol®. The products are delivered only in bulk, with cement trucks.
3.4 Additional Information

More information about binders’ environmental stewardship and occupational health and safety
aspects are detailed within the SDS made publicly available on Holcim Romania portal
https://www.holcim.ro/ro/produse-si-servicii/produse . AI SDS have been developed by Holcim
Romania in compliance with the requirements of Regulation (EU) 2020/878 amending the annex Il of
Regulation (EC) No 1907/2006 of the European Parliament and of the Council on the Registration,
Evaluation, Authorisation and Restriction of Chemicals (REACH) and according to Regulation (EC) No
1272/2008 on the Classification, Labelling and Packaging of substances and mixtures (CLP).

© 2025 Holcim (Romania) SA 4
EPD DOROSOL® Binder — Holcim Romania

4.LCA Information
4.1 Goal of Study

The goal of this study was to generate an environmental profile of DOROSOLS binder produced and
delivered from the locations fully owned and operated by Holcim Romania, to better understand the
associated lifecycle environmental impacts and to allow a Type III EPD to be generated and made public
via the International EPD System.

4.2 Declared Unit

The declared unit of the EPD is 1 tonne of DOROSOLS produced and delivered from the locations
fully owned and operated by Holcim Romania. This EPD is established for the weighted average
product of theses manufacturing plants. The average is based on the mass of binder produced

at each plant.

4.3 System Boundary

System boundaries determine the unit processes to be included in the LCA study and which data
as “input” and/or “output” to/from the system can be omitted.

This EPD covers the cradle to gate stage (A to A3), because other life cycle stages are
dependent on scenarios and are better developed for specific building or construction
works.

System boundaries are according to the modular approach and the cradle to gate stage is divided
into the upstream (A1) and core (A2 and A3) phases, as outlined in Figure 2. Life cycle stage that
are not covered by the EPD are indicated as MND (Module Not Declared).
Information modules pet EPD |

a) Cradle to gate with b} Cradle to gate <) Cradle to grave and f) Construction service

module C1-C4 and with module C1-C4, module D EPD: Cradle to gate with

module D !! module D and optional modules At-A5 and
optional modules

modules ional
A1-A3 Product Mandatory Mandatory Mandatory Mandatony
stage

A4-A5 Optional for goods Mandatory Mandatory
Construction Mandatory for services
process stage A5) Construction installation (see alternative A

Recommended if a

defaut scenario can be

defined

B Use stage — Optional Mandatory Optional
B4) Replacement
B5) Refurbishment
B8) Operational energy use
B7) Operational water use

C End of life C1) Deconstruction. demolition Mandatory Mandatory Optional
stage

D Benefits and D} Reuse, recovery, recychng, Mandatory Mandatory

ioads beyond potential

the system

boun:

Deciared or functional unit

inclusion of reference service life (RSL) Optional Mandatory if any module | Mandatory

in B is included

Figure 2: Modules included in the DOROSOLS® LCA

© 2025 Holcim (Romania) SA 5
EPD DOROSOL® Binder — Holcim Romania
4.4 Data sources and quality

The geographical system boundary of the LCA is Romania. All processes are valid for the production sites
in Romania. The two cement plants account for 100% of total DOROSOLS produced by Holcim in
Romania.

All material flows of the processes are based on company and site-specific data gathered for one
year of operation, for the period 1st January 2021 — 30 September 2021.

Modelling of the life cycle of Holcim Romania DOROSOL® binder was performed using SimaPro v.9.1 LCA
software from PRé.

All relevant background LCI datasets are taken from the Ecolnvent database v3.8 (cut-off)
released in 2021.

The foreground data has been collected on site and validated based on mass balances. The
background data is based on reviewed data from life cycle inventories. As all datasets are
validated, the data quality for the entire study can be judged as very good.

4.5 Allocation

The foreground data has been collected on site and validated based on mass balances. The allocation is
performed according to the basic rules from EN15804:2012+A2:2019. As no co-products are produced, the
flow of materials and energy and also the associated release of substances and energy into the
environment is therefore related exclusively to the binder produced.

All data is included based on measured data for each plant. To ensure high representativeness
for calculation of the DOROSOL® this specific data has been weighted based on the production
mass of each plant, as follows:

36,077.77

43,607.32

79,685.09

55% 45%

Table 3: Holcim Romania —- DOROSOL® Production

4.6 Cut-off Criteria and assumptions

In the process of building an LCI it is typical to exclude items considered to have a negjligible (aka relatively
inconsequential or immaterial) contribution to results. To do this in a consistent and robust manner there
must be confidence that the exclusion is fair and reasonable. To this end, cut-off criteria were defined in
this study, which allow items to be neglected if they meet the criteria. In accordance with EN15804,
exclusions could be made if they were expected to be within the below criteria and the total neglected input
flows per module do not exceed 5% of energy usage and mass:

+ Mass: when using mass as a cut-off criterion, it is appropriate to require the inclusion in the study of
all inputs that cumulatively contribute more than a defined percentage to the mass input of the product
system being modelled.

© 2025 Holcim (Romania) SA 6
EPD DOROSOL® Binder — Holcim Romania

° _ Energy: similarly, an appropriate decision, when using energy as a criterion, is to require the inclusion
in the study of those inputs that cumulatively contribute more than a defined percentage of the product
system's energy inputs.

° __ Environmental significance: decisions on cut-off criteria should be made to include inputs that
contribute more than an additional defined amount of the estimated quantity of individual data of the
product system that are specially selected because of environmental relevance.

The production of the materials that have been excluded from the product system under study are listed in
Table 4. These materials are either waste derived or excluded due to their low economic value. While the
production of these materials are excluded the material masses are part of the calculation and they are
considered as secondary materials.

Material Considered as

Alternative Raw Material (slag / fly ash) Secondary Material
By-bass dust Secondary Material
Fly ash / acidic fly ash (ARSN) Secondary Material
Granulated blast furnace slag Secondary Material
Table 4: Secondary materials excluded from the product system

The clinker production process uses non-renewable secondary fuels (Table 6). According to the PCR,
secondary fuels are modelled to enter the studied system free of environmental loads. They are displayed
as a resource use and all emissions occurring during the production process are allocated to the produced
products.

Fuel Considered as

Mixed industrial waste Non-Renewable Secondary fuel
Petroleum sludges Non-Renewable Secondary fuel
Used / Waste oils Non-Renewable Secondary fuel
Other biomass Non-Renewable Secondary fuel
Sewage sludge Non-Renewable Secondary fuel
Fresh saw dust Non-Renewable Secondary fuel
Used tyres Non-Renewable Secondary fuel
Table 5: Secondary fuels excluded from the product system

In addition to the above, during the LCA several assumptions were made, which have been
documented below for transparency:

e No waste is produced during the clinker production process.

e _ Thereis a difference between the mass of the raw meal consumed and the clinker produced which
is due to the water (remaining humidity of raw materials) that evaporates and mainly CO2that is
released from decarbonation.

4.7 Comparability

EPDs within the same product category but from different programmes may not be comparable.
EPDs of construction products may not be comparable if they do not comply with EN 15804.

© 2025 Holcim (Romania) SA 7
EPD DOROSOL® Binder — Holcim Romania

5. Environmental Performance
The environmental impacts are declared and reported using the parameters and units shown in
the Tables below. Baseline characterisation factors are taken from EF 8.0 methodology (dated November
2019)
The impact categories presented in the following table refer to 1 tonne of DOROSOL®

produced from the locations fully owned and operated by Holcim in Romania.

Parameter Unit Aî A2 A3 A1-A3

Parameters describing environmental impacts

GWP-total: Global Warming
Potential total! kg CO2 eq. 161 7.73 191 360

GWP - GHG kg COZ eq. 159 7.62 190 356.6
GWP — Fossil: Global
Warming Potential fossil fuels

GWP-biogenic: Global
Warming Potential biogenic
GWP-luluc: Global Warming
Potential land use and land kg COZ eq. | 387E-02 | 4.64E-03 | 9.26E-03 5.26E-02
use change?

ODP: Depletion potential of kg CFC 11
the stratospheric ozone layer ed.

kg COZ eq. 161 7.71 191 360

kg COZ2 eq. | 7.62E-02 | 1.67E-02 | -1.43E-02 7.86E-02

9.38E-06 | 1.62E-06 7.86E-06 1.89E-05

AP: Acidification potential mol H+ eq. 2.42E-01 3.87E-02 2.70E-01 5,51E-01

EP-freshwater:

Eutrophication potential,
fraction of nutrients reaching ICRA 4.85E-03 | 1.04E-03 | 5.83E-02 | 6.42E-02
freshwater end compartment
(EP-freshwater)

EP-marine: Eutrophication

potential, fraction of nutrients kg N ea.

RCE HET CRE 5.14E-02 | 1.23E-02 1.48E-01 0.212
compartment
EP-terrestrial: Eutrophication
potential, Accumulated mol N eq. 0.570 0.134 0.593 1.30
Exceedance

.: kg NMVOC
POCP: Formation potential of 0.210 0.041 0.409 0.660

tropospheric ozone eq.

1 The total global warming potential (GWP-total) is the sum of
— GWP-fossil

— GWP-biogenic

— GWP-luluc

2Itis permitted to omit GWP-luluc as separate information if its contribution is < 5 % of GWP-total over the
declared modules excluding module D.

© 2025 Holcim (Romania) SA 8
EPD DOROSOL® Binder — Holcim Romania

ADP
ADIO aepleltio
O O ie
ADP-TO ADIO
Or 10 ie
potentila
DP aie
deprivalion poie
deprivailo eiq
O DIIO
D » DA
enerq ed a
» » Dana
D a SO
onte eg a
PER otal re
D a SO
D D O a
D a ie
enero arrie
D D O
D a SO
onte eg a
P h oÏa
D a SO
econda
DA N
h ab
D O a
econda e
of ne A ate
D azardo
asie dISposec

kg Sb eq. 6.00E-05 | 2.15E-05 | 4.43E-05 1-26E-04

My, net ;

calorific 759 117 1140 2016

value

m3 world

eq. 6.55 0.583 36.7 43.8

deprived

a ele Qe D e 6e O 650 e
MJ 41.0 3.04 96.1 140
MJ 1.33 0.468 3.28 5.08
MJ 42.3 3.51 99.4 145
MJ 761 119 1310 2190
MJ 0 0 0 0
MJ 761 119 1310 2190
Kg 351 0 0 351
MJ 0 0 0.167 0.167
MJ 0 0 0.222 0.222
ms -1.45E-02 | 1.70E-02 0.988 0.991

a ete Qe D e a e DrOû O
kg 5.87E-03 | 1.03E-03 8.57E-03 1.55E-02

3 The abiotic depletion potential is calculated and declared in two different indicators:
— ADP-minerals&metals include all non-renewable, abiotic material resources (i.e. excepting fossil

resources);

— ADP-fossil include all fossil resources and includes uranium.

4 ultimate reserve model of the ADP-minerals&metals model

© 2025 Holcim (Romania) SA 9

EPD DOROSOL® Binder — Holcim Romania

Parameter

NHWD: Non-hazardous

waste disposed 4.74 9.11 2.91 16.8

RWD: Radioactive waste
disposal

4.91E-03 | 7.60E-04 | 8.21E-03 | 39-02

Parameters describing outputs flows

CRU: Components for reuse

MR: Material for recycling

MER: Materials for energy
recovery

ÉËÉE: Exported energy,
electrical

EET: Exported energy,
thermal

© 2025 Holcim (Romania) SA 10
6. References

Boulay et al (2017). The WULCA consensus characterization model for water scarcity footprint: assessing
impacts of water consumption bases on available water remaining (AWARE). Water Use in LCA, 23.

Centrum voor Milieuwetenschappen Leiden (CML) (2012). CML-IA baseline v4.1 / EU25 characterisation
factors. CML, Leiden.

PCR 2019_14 Construction Products (EN 15804+2)
Cement and Building Lime (EN 16908:2017) C-PCR-001 (To PCR 2019:14) Version: 2019-12-20

Ecoinvent (2017). Ecoinvent v3.4, Swiss Centre for Life Cycle Inventories. Available from
www.ecoinvent.ch

Guo (2012). Life Cycle Assessment (LCA) of Light-Weight Eco-composites. Springer, Berlin
Huïjbregts, Steinmann, Elshout, Stam, Verones, Vieira, Zijp, Hollander, van Zelm. ReCiPe 2016: a
harmonized life cycle impact assessment method at midpoint and endpoint level. International Journal
of LCA, DOI 10.1007/s11367-016-1246-y.

ISO (2000), ISO 14020:2000, Environmental labels and declarations — General principles

ISO (2004), ISO 8601:2004 Data elements and interchange formats — Information interchange —
Representation of dates and times

ISO (2006a), ISO 14025:2006, Environmental labels and declarations — Type Il environmental
declarations — Principles and procedures

ISO (2006b), ISO 14040:2006, Environmental management — Life cycle assessment — Principles and
framework ISO (2006c)

ISO 14044: 2006, Environmental management — Life cycle assessment — Requirements and guidelines
ISO (2013)

ISO/TS 14067:2013, Greenhouse gases — Carbon footprint of products — Requirements and guidelines for
quantification and communication

ISO (2014), ISO 14046:2014, Environmental management — Water footprint — Principles, requirements
and guidelines

IPCC (2007). Working Group | Contribution to the IPCC Fourth Assessment Report Climate Change 2007:
The Physical Science Basis, Summary for Policymakers. Intergovernmental Panel on Climate Change,
Geneva

IPCC (2006). 2006 IPCC Guidelines for National Greenhouse Gas Inventories, Volume 4: Agriculture,
Forestry and Other Land Use. IPCC, Geneva

JRC (2011). ILCD Handbook: recommendations for life cycle impact assessment in the European context.
European Commission Joint Research Centre Institute for Environment and Sustainability.

http://eplea.jrc.ec.europa.eu/?page id=86

Pre Consultants (2019). SimaPro v9. Pre Consultant, Amersfoort

Weidema B P, Bauer C, Hischier R, Mutel C, Nemecek T, Reinhard J, Vandenbo C O, Wernet G (2013).
Overview and methodology: data quality guideline for the ecoinvent database version 3 (final). Swiss
Centre for Life Cycle Inventories: St Gallen

© 2025 Holcim (Romania) SA 11
