= EPD
Environmental
Product
Declaration EPD

In accordance with ISO 14025 and UNE-EN 15804:2014+A2:2019 for: ASIA

ECOPact: H30, H25 Agilia, HDOS330, H30 Agilia
and HYDROMEDIA.

FROM

HOLCIM

HOLCIM

Programme: The International EPD® System, www.environdec.com

Programme operator: | EPD International AB

EPD Version 3

EPD registration S-P-08537

number:

Publication date: 2023-04-21

Revision date: 2023-05-29

Valid until: 2028-04-20
An EPD should provide current information and may be updated if conditions change. The stated
validity is therefore subject to the continued registration and publication at www.environdec.com

HOLCIM ee EPD

General information
Programme information

Programme: The International EPDS System
EPD International AB
Box 210 60

Address: SE-100 31 Stockholm
Sweden

Website: www.environdec.com

E-mail: infon@environdec.com

CEN standard EN 15804 serves as the Core Product Category Rules (PCR)

Product category rules (PCR): PCR 2019:14 Construction Products. Version 1.11, c-PCR-003
Concrete and concrete elements (EN 16757). Version 2019-12-20.

PCR review was conducted by: The Technical Committee of the International EPD® System.
See www.environdec.com/TC for a list of members.

Review chair: Claudia A. Peña. The review panel may be contacted via the
Secretariat info@environdec.com

Independent third-party verification of the declaration and data, according to ISO 14025:2006:

[] EPD process certification X EPD verification

Third party verifier:

TECNALIA R&I Certificaciôn S.L. Auditor: Cristina Gazulla Santos
Accredited by: ENAC. Accreditation no.125/C-PR283

Procedure for follow-up of data during EPD validity involves third party verifier:

Yes CO No

The EPD owner has the sole ownership, liability, and responsibility for the EPD.
EPDs within the same product category but from different programmes may not be

comparable. EPDs of construction products may not be comparable if they do not comply with
EN 15804. For further information about comparability, see EN 15804 and ISO 14025.

PAGE 2/21
HOLCIM ee EPD

Company information

Owner of the EPD: HOLCIM SPAIN.
Avenida de Manoteras 20 Edif. Tokyo 1#planta. 28050 Madrid (Spain).
https://www.Holcim.es/

Contact: HOLCIM ESPANA
Telephone: 34 912 13 31 00
Email: marketing.spain@Holcim.com

Description of the organisation: Holcim is one of the world leaders in building materials and
solutions with activity in four business segments: cement, aggregate, concrete solutions and
products in the field of construction. Its ambition is to lead the industry towards reducing carbon
emissions and moving towards low carbon construction. With the strongest R&D area in the
industry, the company seeks to promote the development and marketing of high-quality and
sustainable building materials and solutions for its customers around the world.

Holcim has five cement factories in Spain with an installed capacity of seven million tons per
year, 20 concrete plants, a mortar plant, a plant for the preparation of alternative fuels from
waste, four terminals and two distribution centers, where about 700 employees work. The
company is distinguished by having the first Laboratory with an exclusive area of alternative
fuels and the first Research and Development Center for New Concrete and Mortars. Holcim
contributes to global development by making significant efforts in innovation, which materialize
in the creation of safe, sustainable and high-performance materials and solutions that respond
to customer challenges

Product-related or management system-related certifications:
Holcim has implemented ISO 9001 and ISO 14001 management systems.

Name and location of production site(s):
The results are valid for the product produced in all the manufacturing plants of Holcim in
Spain. The formulation of the products is representative for a complete year.

Product information

Product name: ECOPact: H30, H25 AGILIA, H30 AGILIA, ARTEVIA HDOS 330 and
HYDROMEDIA.

Product description: Holcim is a leading manufacturer and supplier of high quality concrete and
mortar, and has projects and activities on road and network, collective housing.

Concrete and mortar production is a specific process: depending on the nature and quantity of
each of the components (cement, aggregates, water, additives), it will have different
characteristics. Once manufactured, the ready-mixed concrete/mortar is a fresh product, which
must be transported and used quickly on local markets, and under optimal conditions.

Holcim's concretes and mortars offer an outstanding combination of product quality and

performance. All products manufactured are high quality concretes and mortars, characterised
by their extraordinary capacity and high finish.

PAGE 3/21
HOLCIM ee EPD

The products are a ready-mixed concrete/mortar, and the ranges included are structural
concretes, except ECOPact Artevia HDOS H330, which is used in continuous paving and
flooring, and ECOPact Hydromedia which is a draining concrete.

See more product properties in www.Holcim.es/ecopact-hormigon-sostenible

UN CPC code: 375 Articles of concrete, cement and plaster.

LCA information

Functional unit: One m3 of ready-mix of concrete/mortar which fuffills the requirements of
technical performance for construction for a reference service life of 100 years. Ready-mix
concrete for structural applications has a strength of 25 to 30 MPa, while ready-mix concrete
for surface paving must be applied with a dosage of 325 to 330 kg/m°

ECOPact H30 30 rase SENS E oc
ECOPact H25 AGILIA 25 applicable 2311,25 NE on
ECOPact H30 AGILIA 30 rase 2318,00 NERO
CS
RO TER rate ce ZRSLES T an

e For product references that have MPa: the use is structural.

e Forthe product references that do not have MPa: the use is in paving and flooring (they do
not have the "strength" data, in MPa, because they are not structural and are not
characterised by their compression).

Reference service life: 100 years (as functional by the manufacturer) and recommended in c-
PCR for structural concrete.

Time representativeness: the data inventory of the LCA study presented representative of a
regular annual production inventory since Ecopact began to manufacturing on march 2021.
The residual electricity mix is from Spain in 2021 . The amount used of raw materials (cement,
water, gravel stone) has been obtained from the recipe in Papiol and Alcobendas
manufacturing plant in 2021. Energy consumption, waste production, pollutant emissions and
transport distance (in A2 and A4) have been obtained from Alcobendas and Papiol
manufacturing plants in 2021 (from the 1st of January 2021 to the 31st of December 2021)
since the production process is the same for the different concrete products manufactured in
the plants. The composition of the specific cement used for each product has been obtained
also directly from the manufacturing plants and therefore correspondés to reality.

l'UNE-EN 12350-6:2020. Testing fresh concrete - Part 6: Density

PAGE 4/21
U? HOLCIM ee EPD

Residual electricity Mix, Spain 2021

0% = Renowables
# Cogeneration (high efficiency)
Cogeneration
CC natural gas
32%

2%

s Coal

Fuel/Gas

# Nuclear

# Others

Database(s) and LCA software used: generic data on the impact per unit of matter or energy
have been taken to determine emissions per kg of matter, KWh of energy or tkm transported.
These data have been obtained from the Ecoinvent database version 3.8. (updated in <2
years) and Simapro 9.3. The impact models used are those indicated in UNE-EN
15804:2014+A2:2019.

Description of system boundaries:
Cradle to grave and Module D (A+B+C+D)

PAGE 5/21

HOLCIM = EPD

System diagram:

Cement

Recycled cement

Emiss
ions to

air,
. .. soil &
Raw A1-A3 (storage of raw materials, mixing) water
materia
Is

A4 Transport
AS Installation

C End of life

More information: www.Holcim.es

e Technical support for the implementation of the EPD: Marcel Gémez Consultoria
Ambiental.

e The modularity principle, as well as the polluter-payer principle have been followed.
Cut off rules: according to EN 15804 a minimum of 95% of total inflows (mass and
energy) per module are included and more than 99% of the inflows are accounted for.

e Allocation procedure: where necessary (energy and water consumption, waste
production) an allocation based in volume has been used.

e The next processes have not been included since its impact is not significant:

o Environmental impact from infrastructure, construction, production equipment,
and tools that are not directly consumed in the production process.
o  Personnel-related impacts, such as transportation to and from work.
Research and development activities.
o  Long-term emissions.

©

PAGE 6/21
HOLCIM ee EPD

Modules functional, geographical scope, share of specific data (in GWP-GHG indicator) and
data variation:

Construction Resource
Product stage process Use stage End of life stage recovery
stage stage
8 2
c = O
2 D ro] re) S
> œ 3/SIlE ®
Ch = > O œ
es 5 D | 5) D L
a e s|2|8ls=S à S
2 e) = s | T6 | > |2£ a ss
E £ 5 8 Ses) s|S 8 8
© E 2 + 5 S = E SSlEel+e| 2 | (
œ © © © S ce 9 | S|212|0|S|S| x CS
E 2 = Q 5 © | = 025 | | S<S S | © | © d =
= S C S C œ | = o | © | à © © O = u Q 5 ©
© œ œ œ [e) ta] œ © © © Q | Q | © œ GS | © 5
œ - = + © |D|=| | 000 |=E |A Œ à
Module Aî A2 A3 A4 A5 B1 B2 B3 B4 B5 B6 B7 C1 C2 C3 Ca D
Modules X X X X X X X X X X X X X X
functional X
ES ES ES ES ES ES | ES | ES | ES | ES | ES | ES | ES | ES | ES | ES
Geography ES
Specific More than 99% specific data is used in - - - - - - - - - - - -
data used the EPD.
Variation — | Less than 10% inside of every group of - - - - - - - - - - - -
products products
Variation — Less than 10% - - - - - - - - - - - -
sites

e _A1-A3 Product stage

o A1 Raw materials supply: this module takes into account the extraction and
processing of raw materials and the energy that is produced prior to the
manufacturing process under study. The product uses ECOPlanet I/A 42.5N
cement, which contains 41% recycled cement, since a significative amount of
clinker has been replaced by sludge.

o A2 Transport: this module includes the transport of the different raw materials
from the manufacturer to the factory. The distance and type of concrete truck
for each raw material has been introduced.

o A3 Manufacturing: this module includes the consumption of energy and water
used during the manufacturing process, as well as the transport and
management of the factory-produced waste. The manufacture of concreate or
mortar consists mainly of a mixing process of different components.

PAGE 7/21

HOLCIM

—— EPD

e _A4-A5 Construction process stage

o A4 Transport

Fuel type and consumption of vehicle or vehicle
type used for transport e.g. long distance truck,
boat, etc
Distance
Capacity utilisation (including empty returns)
Bulk density of transported products*
Volume capacity utilisation factor

o A5 Construction/installation

Truck of 16- 32 tn. Fuel consumption: 43 L/100
Km

Truck: 10,3 km
% according to Ecoinvent database
See table in LCA information section
1

The product is directly transferred from the truck to the construction site

Auxiliary materials for installation
Use of water
Use of other resources

Quantitative description of the type of energy
(regional mix) and the consumption during the
installation process

Wastage of materials on the building site before
waste processing, generated by the products
installation (specified by type)

No auxiliary material used
Not used
No other resource consumption
Not used

Product losses (2%)

ee __B Use stage: the products fix CO: by carbonatation during the use phase (B1), and
do not require maintenance (B2), repair (B3), replacement (Bd), refurbishment (B5),
operational energy use (B6) or operational water use (B7) during its Reference

Service Life.

CO: fixed by carbonatation of cement during the use phase has been included as
required in c-PCR, following the methodology explained in EN 167572.

CO2 uptake = k * |

Vt
1000

}r vice» c+ pe

Where:

K:K factor, mm of carbonatation/year°
Utcc: maximum theorical uptake in g CO2/Kg of cement

2 UNE-EN 16757:2018. Sustainability of construction works -

Category Rules for concrete and concrete elements

Environmental product declarations - Product

PAGE 8/21
HOLCIM ee EPD

C:cement content in kg/m* of concrete
Dc: degree of carbonation

A hypothesis is made where only one face of one m* of concrete is in contact with air, being
the other 3 faces not in contact with air.

e  C End of life stage

o C1 Deconstruction/demoblition: the use of diesel during the demoblition
process has been included.

o C2 Transport to waste processing: the model use for the transportation
(see A4, transportation to the building site) is applied.

o C3 Waste processing for reuse, recovery and/or recycling: the product is
89% recycled$.

o C4 Disposal: the product is 11% landfilled.

Collection process specified by type The product is collected mixed with construction
waste
Recovery system specified by type 89% recycling
Disposal specified by type 11% landfill

Assumptions for scenario development (e.g. 16-32 tn truck. Fuel consumption: 25 1/100 Km
transportation) Distance: 50 km

e D Reuse-Recovery-Recycling potential
The product is recycled in 89%$. As a consequence, the module D has been calculated, where
the results of recycled content that the product already includes has been taken into account.
The avoided product is considered crushed gravel.

2 https://ec.europa.eu/eurostat/documents/2995521/9629294/8-04032019-BP-EN.pdf/295c2302-4ed1-45b9-af86-
96d1bbb7acb1

PAGE 9/21

U? HOLCIM ee EPD

Content information

EcoPact H30

CEM ECOPlanet INI/A 42,5N 275-325 41 0
Gravel 1800-1900 0
Water 150-170 0
Additves 1-10 0
TOTAL 2305,55 5,4 0
EcoPact H25 Agjilia
CEM ECOPlanet INI/A 42,5N 275-325 41 0
Gravel 1600-1800 0 0
Water 150-200 0 0
Additives 1-8 0 0
Total 2311,25 5,23 0
EcoPact H30 Agilia
CEM ECOPlanet IN/A 42,5N 300-350 41 0
Gravel 1700-1800 0 0
Water 160-190 0 0
Additives 1-8 0
TOTAL 2318,15 5,75 0
EcoPact Artevia HDOS 330
CEM ECOPlanet INI/A 42,5N 300-350 41 0
Gravel 1700-1800 0
Water 150-170 0
Additives 1-5 0
TOTAL 2287,3 5,65 0

PAGE 10/21

U? HOLCIM

—— EPD

EcoPact Prime Hydromedia

CEM ECOPlanet III/A 42,5N 300-350 41
Gravel 1600-1800
Water 60-100
Additives 1-5
Total 2086,25 6,39

© © © © ©

During the life cycle of the product any hazardous substance listed in the “Candidate List of
Substances of Very High Concern (SVHC) for authorization” has not been used in a

percentage higher than 0,1% of the weight of the product.

Environmental Information- results are by m° of product

Estimated impact results are only relative statements which do not indicate the end points of
the impact categories, exceeding threshold values, safety margins or risks.

These results are valid for the next products since their impact differs less than 10%. A
representative virtual product has been chosen, showing the highest results found per stage
and per environmental impact category among the analyzed products.

PAGE 11/21
HOLCIM = EPD

ECOPact H30, H25 AGILIA, H30 AGILIA, ARTEVIA HDOS 330 and HYDROMEDIA
Potential environmental impact - mandatory indicators according to UNE-EN 15804:2014+A2:2019

Manufacture Construction Use End of life Module
A1-A3 A4 A5 B1 B2 | B3 | B4 | B5 | B6  B7 C1 C2 C3 Ca D
Climate change - Fossil kg CO2 eq 2,06E+02 1,70E+00 1,48E+00 -2,17E-01| 0! 0] O0! 0] 0| 0 8,56E+00 1,73E+01 0,00E+00 5,91E-01 -9,73E+00
Climate change - Biogenic kg CO2 eq 2,38E-01 7,25E-04 3,50E-03 0,00E+00 | 0] 0! 0] O0] O0| 0 3,21E-03 1,58E-02 0,00E+00 3,40E-04 -1,76E-01
Climate change - Land use and LU change | kg CO2 eq 3,76E-02 1,78E-05 9,76E-04 0,00E+00 | 0] 0] 0] 0| 0! 0 8,54E-04 6,94E-03 0,00E+00 2,01E-05 -1,87E-02
Climate change kg CO2 eq 2,07E+02 1,70E+00 1,49E+00 -2,17E-01| 0! 0] 0| 0] O0! 0 8,56E+00 1,74E+01 0,00E+00 5,92E-01 -9,92E+00
Ozone depletion kg CFC11 eq 1,93E-05 5,24E-07 3,06E-07 0,00E+00 | 0! 0| 0|[ 0| O0! 0 1,83E-06 4,02E-06 | 0,00E+00 1,23E-07 -2,66E-07
Acidification mol H+ eq 5,67E-01 4,21E-03 6,87E-03 0,00E+00 | 0! 0| 0|[ 0| O0! 0 8,89E-02 4,93E-02 | 0,00E+00 6,09E-03 -4,70E-02
Eutrophication kg PO4--- eq 3,61E-02 3,96E-04 8,16E-04 0,00E+00 | 0! 0| 0|[ 0| O0! 0 1,39E-02 5,14E-03 |  0,00E+00 9,34E-04 -3,81E-03
Eutrophication, freshwater kg P eq 5,67E-03 1,13E-06 1,58E-05 0,00E+00 | 0] 0] 0] 0| 0! 0 2,84E-05 1,24E-04 | 0,00E+00 2,10E-06 -7,78E-04
Eutrophication, marine kg N eq 1,79E-01 6,40E-04 1,94E-03 0,00E+00 | 0] 0! 0] O0] O0| 0 3,94E-02 9,79E-03 0,00E+00 2,65E-03 -8,69E-04
Eutrophication, terrestrial mol N eq 1,97E+00 7,09E-03 2,15E-02 0,00E+00 | 0] 0! 0] O0] O0| 0 4,32E-01 1,09E-01 0,00E+00 2,90E-02 -4,72E-02
Photochemical ozone formation kg NMVOC eq 5,53E-01 2,59E-03 7,01E-03 0,00E+00 | 0] 0] 0] 0| 0! 0 1,19E-01 4,19E-02 0,00E+00 8,09E-03 -9,09E-03
*Resource use, minerals and metals kg Sb eq 2,36E-04 9,59E-08 4,36E-06 0,00E+00 | 0] 0] 0] 0| 0! 0 4,40E-06 6,15E-05 0,00E+00 2,85E-08 -1,26E-04
*Resource use, fossils MJ 1,55E+03 3,13E+01 2,67E+01 0,00E+00 | 0] 0! 0] O0] O0| 0 1,17E+02 2,63E+02 0,00E+00 7,88E+00 -1,47E+02
*Water use m3 depriv. 2,70E+01 -5,23E-03 6,50E-01 0,00E+00 | 0! 0| 0|[ 0| O0! 0 1,84E-01 8,01E-01 | 0,00E+00 3,18E-03 -2,36E+01

* Disclaimer: The results of this Environmental Impact Indicator should be used with caution as the uncertainties of these results are high or as there is limited experience with the Indicator.
* The additional environmental indicators of EN 15804:2012+A2:2019 are not stated in this EPD.

PAGE 12/21

HOLCIM = EPD

Use of resources

Manufacture Construction Use End of life Module
A1-A3 A4 A5 B1 | B2 | B3 | B4 | B5 | B6 | B7 C1 C2 C3 C4 D

Use of renewable primary energy,
excluding the resources of non- M 4,20E+02 4,80E-02 | 7,73E-01 |o|olololololol 66001 | 3,76E+00 | 0,00E+00 | 3,30F-02 | -1,84E+01
renewable primary energy used as a raw
materials
Use of renewable primary energy used M 0,00E+00 0,00E+00 | 0,00E+00 | 0 0 |0/)0|0o|o!o| o00€+00 | 0,00E+00 | 0,00E+00 | 0,00E+00 | 0,00E+00
as raw materials
Total use a renewable primary energy
(primary energy and resources of M 4,20E+02 4,80E-02 | 7,73E-01 |o|olololololol 660601 | 3,76E+00 | 0,00E+00 | 3,30E-02 | -1,84E+01
renewable primary energy used as raw
materials)
Use of non-renewable primary energy,
excluding the resources of non- M 1,57E+03 3,32E+01 | 2,84E+01 | 0 | 0 |o|o!ololo! 125E+02 | 2,79E+02 | 0,00+00 | 8,36E+00 | -1,56E+02
renewable primary energy used as a raw
materials
Use of non-renewable primary energy M 0,00E+00 0,00E+00 | 0,00E+00 | 0 0 |0/)0|0o|o!o| o00€+00 | 0,00E+00 | 0,00E+00 | 0,00E+00 | 0,00E+00
used as raw materials
Total use of non-renewable primary
energy (primary energy and resources of M 1,57E+03 3,32E+01 | 2,92E+01 | 0 |o|o!o!lololol 125E+02 | 2,79E+02 | 0,00E+00 | 8,36E+00 | -1,56E+02
renewable primary energy used as raw
materials)
Use of secondary materials MJ 1,33E+02 0,00E+00 4,66E+00 0100001010 0,00E +00 0,00E+00 0,00E+00 0,00E+00 0,00E+00
Use of renewable secondary fuels MJ 0,00E+00 0,00E+00 0,00E+00 01010|1010|0|0 0,00E+00 0,00E+00 0,00E+00 0,00E+00 0,00E+00
Use of non-renewable secondary fuels MJ 0,00E+00 0,00E+00 0,00E+00 01010|1010|0|0 0,00E+00 0,00E+00 0,00E+00 0,00E+00 0,00E+00
Net use of fresh water m3 1,02E+00 8,58E-05 2,63E-02 01010|0101|0|0 6,70E-03 2,98E-02 0,00E+00 1,68E-04 -6,05E-01

PAGE 13/21

(? HOLCIM = EPD

Waste production and output flows

Waste production

Manufacture Construction Use End of life Module
A1-A3 A4 A5 B1 | B2|B3  B4 | B5 | B6 | B7 C1 C2 C3 Ca D
Hazardous waste disposed Kg 4,85E-03 8,22E-05 4,87E-05 0101010 0|010 3,22E-04 6,87E-04 0,00E+00 1,99E-05 -2,75E-04
Non-hazardous waste disposed Kg 5,64E+01 1,29E-03 5,82E+00 0101010 0|010 1,57E-01 1,38E+01 0,00E+00 2,34E+02 -3,22E+00
Radioactive waste disposed Kg 8,18E-03 2,24E-04 1,39E-04 010010101010 8,11E-04 1,78E-03 0,00E +00 5,44E-05 -6,45E-04
Other output flows
Manufacture Construction Use End of life Module
A1-A3 A4 A5 B1 B2 B3 B4 B5 B6 B7 c1 C2 C3 ca D
Components for re-use Kg (e) (e) (e) 0 0 0 0 0 0 0 0 0 0 0 0
Materials for recycling Kg 0 0 0 0 0 0 0 0 0 0 0 0 1,92E+03 0 0
Materials for energy recovery Kg 0 0 0 0 0 0 0 0 0 0 0 0 0 0 0
Exported energy M] per vector (e) (e) (e) 0 0 0 0 0 0 0 0 0 0 0 0
Potential environmental impact - additional mandatory indicators
Manufacture Construction Use End of life Module
A1-A3 A4 A5 B1 B2 | B3 | B4 | B5 | B6 | B7 c1 C2 C3 Ca D
Global warming (GWP100a)* kg CO2 eq 1,85E+02 1,68E+00 | 1,22E+00 | -1,65E-01 | O | O0 | O0 | O | O | O | 8,56E+00 1,74E+01 | O,00E+00 | 5,87E-01 -9,83E+00

*This indicator includes all greenhouse gases in Total Climate Change but excludes removals and emissions of biogenic carbon dioxide as well as biogenic carbon stored in the product. Therefore,
this indicator is almost the same as the GWP indicator originally defined in EN 15804:2012+A1:2013.

PAGE 14/21

U? HOLCIM = EPD

Information on biogenic carbon content

Biogenic carbon content Unit Quantity
Biogenic carbon content in the product kg C 0,00E +00
Biogenic carbon content in packaging kg C 0,00E +00

Note: 1 kg biogenic carbon is equivalent to 44/12 kg CO:

PAGE 15/21

HOLCIM = EPD

Interpretarion of results

As we can see in Table and Figure, the product stage (A1-A3) is the life cycle stage with the
greatest impact for all the impact categories analyzed, representing between 97,07%
(Eutrophication, freshwater) and 77,02% (Resource use, mienrals and metals) of the total
impact of the product life cycle.

The module (A4-A5) represents a low impact for all the impact categories analyzed. Transport
(Ad) represents between 0,02% (Eutrophication, freshwater) and 2,01% (Ozone depletion) of
the total life cycle impact. On the other hand, AS5-Installation stage represents less than 2% of
the total impact for all impact indicators.

In relation to End of life stages (C1-C4), the impact of C1 is between 16,86% (Eutrophication,
marine) and 0,49% (Eutrophication, terrestrial). C2 Transport represents between 2,12%
(Eutrophication, freshwater) and 20,08% for Resource use, minerals and metals. Finally, C4
Waste treatment represents an impact from 0,01% for Abiotic depletion minerals, and 1,13%
for Eutrophication, marine and Eutrophication, terrestrial.

Table. Potential impact on the environment of the life cycle of one m° of product, in percentage.

Global Warming 88,28% 0,68% 0,59% -0,09% 3,40% 6,91% 0,23%
Ozone depletion 73,98% 2,01% 1,17% 0,00% 7,00% 15,38% 0,47%
Acidification 78,49% 0,58% 0,95% 0,00% 12,31% 6,82% 0,84%
Eutrophication, freshwater 97,07% 0,02% 0,27% 0,00% 0,49% 2,12% 0,04%
Eutrophication, marine 76,71% 0,27% 0,83% 0,00% 16,86% 4,19% 1,13%
Eutrophication, terrestrial 76,70% 0,28% 0,84% 0,00% 16,81% 4,25% 1,13%
Photochemical ozone formation 75,60% 0,35% 0,96% 0,00% 16,24% 5,74% 1,11%
R r minerals an

le Use erals and 77,02% 0,03% 1,42% 0,00% 1,44% 20,08% 0,01%
Resource use, fossils 77,65% 1,57% 1,34% 0,00% 5,88% 13,17% 0,39%

PAGE 16/21

U? HOLCIM = EPD

100%

90% n |

80% EE _ | | | | |. |
70%
60%
50%
40%
30%
20%
10%
0%
NS e SN Cu d” S
x S S # S ° S Où À
S 2 G Q Fa & A so
Ka où S > & S D o e
N d ES «e RS x? LC L &
ES & Ÿ \ & .S Rù PS e
S © À SÈ à ea CA D
RSS & N Q @ Da
CS) S où Q S
Q © S S
F © Ca
LR

HA1-A3 mA4 AS B1 - CO2 absortion C1 C2 mcCa

Figure. Potential impact on the environment of the life cycle of one m of product, in percentage.

Additional information

With the aim of achieving a positive contribution to nature and society, we develop our activity
based on principles of sustainable development, through continuous improvement in our
environmental behaviour and focused on these four fundamental principles: our Management
System, control environmental impact, contribution to the circular economy and transparent
relationship with the environment.

Registry of carbon footprint, compensation and CO: absorption projects of the
Ministerio para la Transiciôn Ecologica y el Reto Demogräfico de España.

2016 2017 2018 Eos k 2020
ds) Vs) Ve, ee,
de me dem dm dem

Holcim Spain has registered its carbon footprint in section a) of the Carbon footprint and
commitment to reduce greenhouse gas emissions for the years 2016, 2017, 2018, 2019 and
2020.

The limits of the organization included in the calculation are: cement, concrete and mortar

manufacturing activity carried out in all its facilities in Spain, central offices in Madrid and 63
production centers

PAGE 17/21
U? HOLCIM = EPD

Our commitment to the circular economy as the main way to take advantage of the
waste life cycle

The transition from a linear economy to a circular economy is one of the environmental
priorities of our business. Within our activity, our objective is to reuse the value of waste as
resources, that is, to maximize its life cycle.

At Holcim, we achieve the transition to circularity by complementing the activity of Geocycle, a
subsidiary of the Group that is dedicated to the pre-treatment of waste to turn it into fuel, and
the cement factories that use it in their clinker production process (component cement base).

Proactive restoration of our quarries

At Holcim we have been working, for more than 30 years, for the restoration of our quarries
with the aim of generating a net positive impact on biodiversity. We are committed to a
participatory model of quarry rehabilitation in which the increase of biodiversity and natural
capital is favoured.

Our restoration model serves as a lever for change on the critical problem of biodiversity loss
and its potential to reverse its current negative trend. This work, key when it comes to creating
shared value with the communities in which we operate, has been recognized in 2018 with the
first second prize in the "Company and Biodiversity" category in the latest edition of the
European Business Awards for the Environment , promoted by the Biodiversity Foundation.

PAGE 18/21
PH

HOLCIM *EPD

Information related to Sector EPD
Individual EPD.

Differences versus previous versions
The EPD was updated considering the following changes:

2"d version:

The registration number of the first version of the EPD is S-P-03786.

There is a new and specific EPD for ECOPlanet CEM I/A 42,5 N (S-P-05185),
therefore the values for the impacts in (A1 — raw materials) were updated.

The residual electricity mix used was from 2021 it means the impacts of electricity in
(A3-manufacture) were updated.

Transport consumptions for A4 have been updated according to specific consumptions
of the trucks used.

The grouping of concrete products is updated. On the first version of the EPD (S-P-
03786), up to 11 products were included, but on this version of the EPD products have
been separated in different EPDs.

The PCR 2019:14 version 1.11 is used.

3'd version:

A new logotype of Holcim is used.

PAGE 19/21
U? HOLCIM = EPD

References

+ General Programme Instruction of the International EPD® System. Version 3.01.

e ISO 14020:2000 Environmental labels and declarations - General principles.

e ISO 14025:2010 Environmental labels and declarations - Type Ill Environmental
Declarations - Principles and procedures.

e ISO 14040:2006 Environmental management - Life Cycle Assessment - Principles and
framework.

e ISO 14044:2006 Environmental management - Life Cycle Assessment - Requirements
and guidelines.

e  UNE-EN 12350-6:2020. Testing fresh concrete - Part 6: Density

e Real Decreto 470/2021, 29th June, Spain

e  UNE-EN 12390-3:2020 Testing hardened concrete - Part 3: Compressive strength of
test specimens.

e PCR 2019:14 Construction products (EN 15804:A2) version 1.11.

e  UNE-EN 15804:2014+A2:2019 Sustainability of construction works - Environmental
Product Declarations - Core rules for the product category of construction products.

e _c-PCR-003 Concrete and concrete elements (EN 16757).

e  Holcim ECOPlanet CEM H/A 42,5N https://www.environdec.com/library/epd5185
https://www.Holcim.es/ecoplanet-cemento-sostenible

e The underlaying LCA report. Version 4, March 2023

PAGE 20/21

tecnal:a D — ©
certification EPD

VERIFICATION STATEMENT CERTIFICATE
CERTIFICADO DE DECLARACIÔN DE VERIFICACION

Certificate No. / Certificado n°2: EPD04609

TECNALIA R&l CERTIFICACION S.L, confirms that independent third-party verification has been conducted of the
Environmental Product Declaration (EPD) on behalf of:

TECNALIA R&I CERTIFICACION S.L., confirma que\se ha realizado verificaciôn de tercera parte independiente de la Declaraciôn
Ambiental de Producto (DAP) en nombre de:

HOLCIM ESPANA, S.A.U.
Avd. Manoteras, 20
28050 MADRID - SPAIN

for the following product(s):
para el siguiente(s) producto(s):

ECOPact: H30, H25 AGILIA, HDOS330, H30 AGILIA and HYDROMEDIA.
ECOPact: H30, H25 AGILIA, HDOS330, H30 AGILIA e HYDROMEDIA.

with registration number S-P-08537 in the International EPD® System {www.environdec.com)
con nümero de registro S-P-08537 en el Sistema International EPD® (www.environdec.com)

it's in conformity with:
es conforme con:

* General Programme Instructions for the International EPD® System v.3.01.
= PCR 2019:14 Construction products v1.11.

“ c-PCR-003 Concrete and concrete elements (EN 16757).

= UN CPC code: 375 Articles of concrete, cement and plaster.

isiôn: 21/04/2023
Issued date / Fecha de emisiôn /04/ Carlos Nazabal Alsua
Update date / Fecha de actualizacién: 21/04/2023 Manager
Valid until / Vélido hasta: 20/04/2028
Serial N° / N£ Serie: EPD0460900-E

This certificate is not valid without its related EPD.
Este certificado no es vélido sin su correspondiente EPD. £
CERTIFICACION
El presente certificado est sujeto a modificaciones, suspensiones temporales y retiradas por TECNALIA R&l CERTIFICACION. ISO 17065

This certificate is subject to modifications, temporary suspensions and withdrawals by TECNALIA R&I CERTIFICACION. N°125 / C-PR283
El estado de vigencia del certificado puede confirmarse mediante consulta en www.tecnaliacertificacion.com.

The validity of this certificate can be checked through consultation in www.tecnaliacertificacion.com.

TECNALIA R&I CERTIFICACION S.L. Area Anardi, n° 5. 20730 AZPEITIA (Gipuzkoa) SPAIN. Tel.:+34 678 860 822 — www.tecnaliacertificacion.com

—— EPD

www.environdec.com
