ENVIROCORE 201 EPD

NORTH & SOUTH ISLAND - AUCKLAND / WELLINGTON / DUNEDIN- ENVIROCORE 201

Managed By: Holcim NZ Ltd Valid From 6 June 2023 | Valid To 6 June 2028
EPD Process Certificate No. 1012 Revision Date: 6 June 2023

Verified Accreditation Body: Epsten Group, Inc. Revision Number: 1.0

EPD Registration No. S-P-08440 Geographical Scope: New Zealand

y

——————

CONTENTS

INTRODUCTION

ABOUT HOLCIM NEW ZEALAND

LOW CARBON CEMENT IN NEW ZEALAND

LCA INFORMATION

EPD PRODUCT DESCRIPTION AND USE
ENVIRONMENTAL PERFORMANCE

PREVIOUS VERSION

REFERENCES

PROGRAM-RELATED INFORMATION AND VERIFICATION

1.0 6 June 2023 N/A

INTRODUCTION

Cement is a key ingredient in the most commonly used building
material in the world. Each year in New Zealand, over 1.5 million tonnes
of traditional cement is used, generating 1.23 million tonnes of CO:.1

This clearly demonstrates both the essential need for construction materials now and in the future, as
well as the necessity for the construction materials industry to be a leading part of the solution
addressing climate change.

With Aotearoa committed to net zero by 2050, Holcim New Zealand is building progress for a lower
carbon footprint in the built environment.

For us, building progress means a complete range of low carbon, high-performance, and specialty
cement and cement binders suitable for Aotearoa's homes, buildings, and infrastructure. It means
advice, tools and resources to help you specify your next project with confidence. It means solutions
that are right for you each and every time.

Together, we can build better
to help decarbonise Aotearoa.

1 International Energy Agency (IEA) report "The Future of Cement in a Carbon-Constrained World"(2018); Cement and
Concrete Association of New Zealand - Key Facts and Figures; The International Energy Agency (IEA) Cement Technology
Roadmap 2009 estimates that the production of 1 tonne of cement results in the emission of approximately 0.82 tonnes
of CO. Using the conversion factor of 0.82 tonnes of CO: per tonne of cement, the production of 1.5 million tonnes of
cement in New Zealand would result in the emission of approximately 1.23 million tonnes of CO. The actual amount of
CO2emissions may vary.

ENVIROCORE 201 EPD | 1

Z
©
F
O
2
[a)
[e)
œ
[es
£Z

ABOUT HOLCIM
NEW ZEALAND

BUILDING PROGRESS

Holcim New Zealand (NZ) is a leading
solutions provider for your design and
construction needs in New Zealand,
dating back to 1888. Today, we supply
essential construction materials from
import terminals, depots, and quarries to
customers. Our cement and aggregates
are used in ready-mix concrete,
engineered precast concrete, and
prestressed concrete solutions for various
projects throughout the country.

AUCKLAND TAURANGA

NEW PLYMOUTH
NAPIER
NELSON

This EPD provides our stakeholders with confidence about
the environmental impact of our products.

Globally, Holcim is 60,000 people around the world who
are passionate about building progress for people and the
planet through four business segments: Cement, Ready-
Mix Concrete, Aggregates and Solutions & Products.

Sustainability is at the core of our global strategy, with our
industry's first 2030 and 2050 net-zero targets validated by D»

DUNEDIN

the Science Based Targets initiative for all scopes. We are
leading the transition towards low-carbon construction
and driving a circular economy by providing materials and
solutions that are re-shaping the way our industry builds.
Holcim NZ has developed a range of low carbon cements
and cement replacements specifically for the New Zealand
market.

ENVIROCORE 201 EPD | 2

[a]
Z
<
_—
<
Li
N
Z
Lu
z
=
O
_—
O
JL
[=
2
[e]
m
<

LOW CARBON CEMENT
IN NEW ZEALAND

EF
2
>
Lu Q
24
Z
Oz
 uj
ŒÆN
HE
05
Zz z
9z

HOLCIM NZ’'S CEMENT AT À GLANCE

Holcim NZ provides project-specific, on-demand
Environmental Product Declarations (EPDs) to customers.
This capability represents a significant step in Holcim NZ's
sustainability journey and embodies our multi-disciplinary
approach to embedding sustainability into our
organisation and operations. With the introduction of our
cement blends, third-party verified data will underpin our
capability to work with our customers from tender through
to design and construction to optimise sustainability
performance.

Holcim NZ's cementitious materials are backed by an EPD
Process Certification. It's not only a first for cement, but a
first for any product in New Zealand. Our EPD Process
Certification is a stamp of approval to produce compliant
EPDs in-house, opening up significant capability and
flexibility in producing and using life cycle impact data to
inform our operations and our customers.

To gain our EPD Process Certification, Holcim invested in
embedding Life Cycle Assessment (LCA) into our systems
and processes. We have satisfied a rigorous, third-party
evaluation in accordance with the relevant ISO standards
and guidelines of the International EPD Program and EPD
Australasia. 2?

This EPD has been developed using our EPD Process
Certification for NORTH & SOUTH ISLAND - AUCKLAND /
WELLINGTON / DUNEDIN - ENVIROCORE 201 with
production occurring at AUCKLAND / WELLINGTON /
DUNEDIN.

25-6 and 8-12 in the References section.

ENVIROCORE 201 EPD | 3
LCA INFORMATION

Declared Unit

1 tonne of cement blend

Reference Service Life (RSL)

The RSL is not specified as the scope is from cradle to gate
with distribution (module A4) option.

Time Representativeness

The plant data for the LCA is based on 2021 calendar year
production data. The mix data for the LCA is based on
2021 calendar year production data.

Databases and LCA Software Used

SimaPro® LCA software (v 9.4) was used for the LCA
modelling which developed the LCA Calculator, used as
per the certified EPD Process. It uses background data
from:

1. The Australian Life Cycle Inventory Database (AusLCI
v1.39) (2022)

2. Ecoinvent 3.8 (2021)

The environmental impacts modelled from the existing
EPDs do not include impacts for the additional Green Star
(v1.2) impact categories included in the environmental
impact tables. The following impact categories were
calculated manually for the foreground data:

ee __ Use of renewable primary energy resources used as raw
materials

e __ Use of non-renewable primary energy, excluding non-
renewable primary energy resources used as raw
materials

e Use of secondary materials
e Use of renewable secondary fuels

e Use of non-renewable secondary fuels

$ Australian Life Cycle Inventory Database Initiative
(AuSLCI). (2022). Guidelines for Data Development for an
Australian Life Cycle Inventory Database, Data Standard.

LCA INFORMATION

Allocation

Allocation was necessary to proportion inputs and outputs
to intermediate flows and processes at the plant level. As
much as possible, intermediate flows were allocated
physically based on the weight of cement.

Ground granulated blast furnace slag from steel blast
furnace production was allocated economically. Please
refer to the “Recycled Material” section for further detail.

Cut-Off Criteria

No flows were excluded on the basis of cut-off criteria.

Address and Contact Information

Holcim (New Zealand) Ltd
23 Plumer Street, Central Auckland 1010
New Zealand

www.holcim.co.nz

ENVIROCORE 201 EPD | 4
Data Quality

Data quality for the foreground data was assessed in terms
of geographic and temporal representativeness. Al data
sources were scored medium or higher.

Background data sources were also assessed with respect
to their timeliness, with all data sources being updated
within the 10 years required under PCR 2019:14.

ENVIROCORE 201 EPD | 5

LCA INFORMATION

SYSTEM DIAGRAM

The processes included in the LCA are presented in a process diagram in the figure below.

Ship Cement Unloading Ship Cement Loading Distribution

DESCRIPTION OF SYSTEM BOUNDARIES
AND EXCLUDED LIFECYCLE STAGES

The scope of the LCA and EPD is from cradle to gate (A1-A4). Life cycle stages beyond Holcim's gate
are excluded from the LCA (see figure below).

Environmental impacts relating to personnel, infrastructure and production equipment not directly
consumed in the process are excluded from the system boundary as per the Product Category Rules
(2019:14 Construction Production and Construction Services).

Construction Benefits & loads for
Product Stage Use Stage End of Life Stage the next product

Stage system

Raw Material Supply
Transport
Manufacturing
Transport
Construction/Installation process
Use
Maintenance incl. transport
Repair incl. transport
Replacement incl. transport
Refurbishment incl. transport
Operational Energy Use
Operational Water Use

AI A2 A3 A4 A5 B1 B2 B3 B4 B5 B6 B7

ND: Module not declared

ENVIROCORE 201 EPD | 6

Z
©
FE
<
Z
œ
[e)
LL
Es
<
O
en]

EPD PRODUCT DESCRIPTION
AND USE

Z
©
EF
a
[ra
re]
n
LU
[a)
=
e]
2
[a)
O
[ra
©
[a]
©
LU

Lu
[2]
2
Q
Z
<

HOLCIM NZ’'S CEMENTITIOUS PRODUCTS NORTH & SOUTH ISLAND - AUCKLAND /
WELLINGTON / DUNEDIN- ENVIROCORE 201

A detailed breakdown of the functional properties of the cement included in this EPD are provided
below. Product environmental information should only be compared with consideration of the
product's requisite function.

NORTH & SOUTH ISLAND - AUCKLAND / WELLINGTON / DUNEDIN - ENVIROCORE 201

Manufacturing process and flow diagram

Fly Ash ]

Devanning and

Debagging

MIX DESCRIPTIONS
Do | pant | Produetbrand | ns u atonhtnihe nr. =
use use
Supplementary Supplementary
North Island Auckland ENVRRT Core Cementitious South Island Dunedin ENVRO Gore Cementitious
Material Material
Supplementary
North Island Wellington ENVRRT Core Cementitious
Material

ENVIROCORE 201 EPD | 7
Content Declaration

The following table provides a summary of the materials included in Holcim's cement and their
relative composition by weight. The gross weight of this declared material makes up a minimum of
99% of the products covered by this EPD.

Zz
©
=
Eu
œ
re]
n
LL
[a]
=
e]
2
Q
O
œ
ru
[a]
0.
Lu

Lu
M]
=)
Q
Z
<

Packaging Default background data from LCA databases was
used to model the above co-products:
Holcim cement is delivered in either bulk or
packaging. e Fly ash: AusLCI process for fly ash treats it as a
waste material and only includes transport
impacts.

Recycled Material
e Ground granulated blast furnace slag: the

BS EN 16757:2017 specifically lists the following AusLCI process for slag is allocated based on

materials relevant to the study as co-products: economic value, as the product has a
significant economic value at the point of

+ Flyash; collection.

°__ Ground granulated blast furnace slag; and The allocation approach of the AusLCI LCA

database was adopted as a default for secondary
data and processes (eg. secondary fuel in cement
production). The AusLCI dataset conforms to EN
15804 when applying allocation to its various
processes and sub-processes.

As such, the above materials are considered as co-
products of their production process and the
impacts for their production process are allocated
according to PCR 2019:14 Construction Products
and Construction Services (co-produced goods,
multi-output allocation).

Item Hazardous Content MES) Post-consumer material (%) Renewable Material (%)

Fly Ash Ÿ 100% 0 0

ENVIROCORE 201 EPD | 8
ENVIRONMENTAL
PERFORMANCE

The environmental impacts considered in this EPD are listed in the table below.

Al further tables from this point will contain abbreviation only.

Impact Category

Potential Environmental Impacts

Abbreviation

Measurement

Total global warming potential GWPT g CO: equivalents (GWP100)
Global warming potential (fossil) GWPF g CO: equivalents (GWP100)
Global warming potential (biogenic) GWPB g CO: equivalents (GWP100)
Global warming potential (land use/ land transformation) GWPL g CO: equivalents (GWP100)
Ozone depletion potential ODP g CFC 11 equivalents
Acidification potential AP mol H+ eq.

Eutrophication - aquatic freshwater

EP - freshwater

g PO43- equivalents

Eutrophication - aquatic freshwater

EP - freshwater

g P equivalent

Eutrophication - aquatic marine

EP - marine

g N equivalent

Eutrophication -— terrestrial

EP -— terrestrial

mol N equivalent

»
uw
Zz ©
Lu Z
E <
Z 2
CL:
ED
> ©
Z LU
Lu ©

Photochemical ozone creation potential POCP g NMVOC equivalents
Abiotic depletion potential (elements) ADPE g Sb equivalents
Abiotic depletion potential (fossil fuels) ADPF MJ net calorific value
Water Depletion Potential WDP m3 equivalent deprived
Resource use
Use of renewable primary energy excluding renewable primary energy resources PERE M3, net calorific value
used as raw materials
Use of renewable primary energy resources used as raw materials PERM M9, net calorific value
Total use of renewable primary energy resources (primary energy and primary PERT M3, net calorific value
energy resources used as raw materials)
Use of non-renewable primary energy excluding non-renewable primary energy PENRE M3, net calorific value
resources used as raw materials
Use of non-renewable primary energy resources used as raw materials PENRM M9, net calorific value
Total use of non-renewable primary energy resources (primary energy and PENRT M3, net calorific value
primary energy resources used as raw materials)
Use of secondary material SM kg
Use of renewable secondary fuels RSF M), net calorific value
Use of non-renewable secondary fuels NRSF M), net calorific value
Use of net fresh water FW m3
Waste categories and Output flows
Hazardous waste disposed HWD kg
Non-hazardous waste disposed NHWD kg
Radioactive waste disposed/stored RWD kg

CFR kg

Components for reuse

ENVIROCORE 201 EPD | 9
Impact Category Abbreviation Measurement

z
: : EE
Materials for recycling MER kg Z 2
tr]
E <
Materials for energy recovery MFEE kg 5 =
& O
Exported energy EE -e MJ per energy carrier = Œ
Z
Lu ©
Exported energy, thermal EE -t MJ per energy carrier

Additional environmental impacts

Global warming potential, excluding biogenic uptake, emissions and storage GWP-GHG kg CO: equivalents (GWP100)
Particulate matter PM disease incidence

lonising radiation - human health IRP kBq U-235 eq

Eco-toxicity (freshwater) ETP-fw CTUe

Human toxicity potential - cancer effects HTP-c CTUh

Human toxicity potential - non cancer effects HTP-nc CTUh

Soil quality SQP dimensionless

ENVIROCORE 201 EPD | 10
TT | Qd3 TOC AHODOHIANZT

NORTH & SOUTH ISLAND - AUCKLAND / WELLINGTON / DUNEDIN- ENVIROCORE 201 - MODULE A1-A3

Primary indicators - 1 tonne of cement

Lu]
LL
_—
)
<
re
>
œ
<
Z
Z
=]
u

ENVIRONMENTAL IMPACTS

GWP-F GWP-B re GWP-T opP AP EP-F EP - F2 EP-M EP-T POCP ADP ADPF WDP
Plant product kg CO-eq kgCO-eq kgCO:eq kgCO-eq kg rs mol H+ eq kg Fa 3- kg P eq kg N eq mol N eq kg press kg Sb eq MJ deprive d
Auckland En IROCOre 8669  -5.22E-02 5.45E-02 86.69 1.66E-05 2.43 0.02 5.79E-03 0.55 6.11 1.62 -3.12E-04 1116.02 2.89
Wellington En IROCOIS 1042 -7.33E-02  6.94E-02 110.42  2.12E-05 3.10 0.02 7.26E-03 0.70 7.80 2.07 -3.99E-04 1417.14 3.63
Dunedin S0n IROCOe 10265  -6.64E-02  6.45E-02 102.65  1.97E-05 2.88 0.02 6.78E-03 0.65 7.25 192  -3.70E-04 1318.48 3.39

2T | Qd3 TOC AHODOHIANZ

NORTH & SOUTH ISLAND - AUCKLAND / WELLINGTON / DUNEDIN- ENVIROCORE 201 - MODULE A1-A3

Resource use parameters - 1 tonne of cement

PERE PERM PERT PENRE PENRM PENRT sM RSE NRSF FW

Plant Product MJ MJ MJ MJ MJ MI kg MJ MI m3
brand

Auckland Nes 3.9E+01 0.0E+00 3.9E+01 1.2E+03 0.0E+00 1.2E+03 0.0E+00 0.0E+00 0.0E+00 4.1E-02

Wellington En IROCOre 4 2E+01 0.0E+00 4.2E+01 1.5E+03 0.0E+00 1.5E+03 0.0E+00 0.0E+00 0.0E+00 5.2E-02

Dunedin Nés 4.1E+01 0.0E+00 4.1E+01 1.4E+03 0.0E+00 1.4E+03 0.0E+00 0.0E+00 0.0E+00 4.8E-02

Lu]
LL
_—
)
<
re
>
œ
<
Z
Z
=]
u

€T | Gd3 TOC 2HODOHIANZ

NORTH & SOUTH ISLAND - AUCKLAND / WELLINGTON / DUNEDIN- ENVIROCORE 201 - MODULE A1-A3

Waste categories and output flows - 1 tonne of cement

Lu]
Lu
_—
c]
<
re
>
œ
<
Z
Z
=]
u

WASTE CATEGORIES AND OUTPUT FLOWS

HWD NHWD RWD CRU MER MERE EE-e EE-t
Plant product kg kg kg kg kg kg MI MI
Auckland S0n IROCO'e 1 08E-03 4.52E+00 7.29E-03 O0.00E+00  0.00E+00  O.00E+00  O.00E+00  0.00E+00
Wellington S0n IROCOe 1 37E-03 5.73E+00  ©.31E-03 O0.00E+00  0.00E+00  O.00E+00  O.00E+00  0.00E+00
Dunedin En IROCOe  127E-03 5.33E+00 8.65E-03 0.00E+00  0.00E+00  O.00E+00  O.00E+00  0.00E+00

ŸT | Qd3 TOC AHODOHIANZ

NORTH & SOUTH ISLAND - AUCKLAND / WELLINGTON / DUNEDIN- ENVIROCORE 201 - MODULE A1-A3

Additional indicators 1 tonne of cement

ADDITIONAL ENVIRONMENTAL IMPACTS

GWP-GHG PM IRP ETP-fw HTP-c  HTP-nc sQP
Plant product kg CO: eq Ress kBqU-235eq  CTUe CTUh CTUh Pt

Auckland Don IROCore 85.90 2.62E-06  4.55E+00 7.25E+02 6.32E-08  4.38E-07  1.63E+02
Wellington Don IROCOre 59 43 3.34E-06  5.81E+00 9.17E+02  B8.06E-08  5.57E-07  2.08E+02
Dunedin On IROCOS 10172  310E-06 5.40E+00 8.54E+02  7.49E-08  5.18E-07  1.93E+02

Lu]
Lu
_—
c]
<
re
>
œ
<
Z
Z
=]
u

ST | Gd3 TOC 2HODOHIANZ

NORTH & SOUTH ISLAND - AUCKLAND / WELLINGTON / DUNEDIN- ENVIROCORE 201 - MODULE A4

Primary indicators - 1 tonne of cement

ENVIRONMENTAL IMPACTS

GWP-F GWP-B re GWP -T ODP AP EP-F EP - F2 EP -M EP-T POCP ADP ADPF WDP
Product kg CFC-11 kg POA4. 3- kg NMVOC m3 eq
Plant brand kg CO:eq kgCO:eq kgCO:eq kgCO:eq eq mol H+ eq eq kg P eq kg N eq mol N eq eq kg Sb eq MI deprived
ENVIROCore
Auckland 201 0.00 0.00E+00  O.00E+00 0.00 0.00E+00  0.00E+00  O.00E+00  0.00E+00  O.00E+00  O.00E+00  O.00E+00  0.00E+00 0.00 0.00
: ENVIROCore
Wellington 201 0.00 0.00E+00  O.00E+00 0.00 0.00E+00  0.00E+00  O.00E+00  0.00E+00  O.00E+00  O.00E+00  O.00E+00  0.00E+00 0.00 0.00
. ENVIROCore
Dunedin 201 0.00 0.00E+00  O.00E+00 0.00 0.00E+00  0.00E+00  O.00E+00  0.00E+00  O.00E+00  O.00E+00  O.00E+00  0.00E+00 0.00 0.00

Lu]
LL
_—
)
<
re
>
œ
<
Z
Z
=]
u

9T | Ad TOC AHODOHIANZ

NORTH & SOUTH ISLAND - AUCKLAND / WELLINGTON / DUNEDIN- ENVIROCORE 201 - MODULE A4

Resource use parameters - 1 tonne of cement

Lu]
Lu
_—
c]
<
re
>
œ
<
Z
Z
=]
u

PERE PERM PERT PENRE  PENRM  PENRT sM RSF NRSF FW

Plant Product MI MI MI MI MI MI kg MI MI m3
brand

Auckland Nes 0.00E+00  0.00E+00 0.00 0.00 0.00E+00 0.00 0.00E+00  O.00E+00  O.00E+00  0.00E+00

Wellington S0n IROCOre 5 00E+00  0.00E+00 0.00 0.00 0.00E+00 0.00 0.00E+00 0.00E+00  0.00E+00  0.00E+00

Dunedin Nes 0.00E+00  0.00E+00 0.00 0.00 0.00E+00 0.00 0.00E+00 0.00E+00  0.00E+00  0.00E+00

ZT | Ad3 TOC AHODOHIANZ

NORTH & SOUTH ISLAND - AUCKLAND / WELLINGTON / DUNEDIN- ENVIROCORE 201 - MODULE A4

Waste categories and output flows - 1 tonne of cement

WASTE CATEGORIES AND OUTPUT FLOWS

HWD NHWD RWD CRU MER MFRE EE-e EE-t
Plant product kg kg kg kg kg kg MI MI

Auckland En IROCOIS GO O0E+00  0.00E+00  O0.00E+00 O0.00E+00  0.00E+00 0.00E+00  0.00E+00  0.00E+00
Wellington En IROCOIS GO O0E+00  0.00E+00  O0.00E+00 O0.00E+00  0.00E+00 0.00E+00  0.00E+00  0.00E+00
Dunedin S0n IROCO'e D 00E+00  0.00E+00  O.00E+00 0.00E+00  0.00E+00  O.00E+00  O.00E+00  0.00E+00

Lu]
Lu
_—
c]
<
re
>
œ
<
Z
Z
=]
u

8T | Gd1 TOC 2HODOHIANZ

NORTH & SOUTH ISLAND - AUCKLAND / WELLINGTON / DUNEDIN- ENVIROCORE 201 - MODULE A4

Additional indicators 1 tonne of cement

Lu]
Lu
_—
c]
<
re
>
œ
<
Z
Z
=]
u

ADDITIONAL ENVIRONMENTAL IMPACTS

GWP-GHG PM IRP ETP-fw  HTP-c  HTP-nc
Plant product kg CO: eq see kKBqU-235eq  CTUe CTUh CTUh

Auckland Don IROGore 0.00 0.00E+00  O.00E+00  O.00E+00  O0.00E+00  0.00E+00
Wellington On IROCore 0.00 0.00E+00  0.00E+00  0.00E+00  O.00E+00  0.00E+00
Dunedin On IROCore 0.00 0.00E+00  O.00E+00  O.00E+00  0.00E+00  O.00E+00

PREVIOUS VERSION

REFERENCES

5 © D hR

10.

11.

12.

13.
14.

REFERENCES

Australasian EPD Program. (2017). Guidance on the use of INA in EPDs.
Australasian EPD Program. (2018). Guidance on the use of background LCI data.
Australasian EPD Program (2019) Instructions of the Australasian EPD Program V3.01.

Australian Life Cycle Inventory Database Initiative (AuSLCI). (2022). Guidelines for Data
Development for an Australian Life Cycle Inventory Database, Data Standard.

British Standards Institution. (2019). Sustainability of construction works. Environmental product
declarations. Core rules for the product category of construction products, BS EN
15804:2012+A2:2019. British Standards Institution.

British Standards Institution. (2017). Sustainability of construction works - Environmental
product declarations - Product Category Rules for concrete and concrete elements, BS EN
16757:2017. British Standards Institution.

Ecoinvent Centre. (2019). Ecoinvent version 3 database. Zurich: ETH, Agroscope, EMPA, EPFL, PSI.
Retrieved from www.ecoinvent.org.

EPD International. (2019). General Program Instructions (GPI) for the International EPD System
V4.0. Retrieved from www.envirodec.com.

EPD International. (2021). Product Category Rules for Construction Products and Construction
Services, PCR2019:14 v1.11. Stockholm: EPD International.

ISO. (2006). Environmental labels and declarations - Type Ill environmental declarations -
Principles and procedures, ISO 14025:2006. Geneva: International Organization for
Standardization.

ISO. (2006). Environmental management -— Life cycle assessment - Principles and framework, ISO
14040:2006. Geneva: International Organization for Standardization.

ISO. (2018). Environmental management. Life cycle assessment. Requirements and guidelines,
ISO 14044:2006+A1:2018. Geneva: International Organization for Standardization.

AUSLCI. (2018) AusLCI Database. Retrieved from AusLCI: www.auslci.com.au/

Man Yu, Thomes Wiedmann, Robert Crawford, Catriona Tait, ‘The Carbon Footprint of New
Zealand's Construction Sector’, Procedia Engineering, Volume 180, 2017, Pages 211-220, ISSN
1877-7058, (http://www.sciencedirect.com/science/article/pii/S1877705817316879)

ENVIROCORE 201 EPD | 20
PROGRAM-RELATED
INFORMATION AND VERIFICATION

n Holcim (New Zealand) Ltd
Declaration Owner 23 Plumer Street, Central Auckland 1010, New Zealand
v www.holcim.co.nz

® EPD Australasia Limited
EPD Program Operator AUSTRALASIA F PD 8315a Hardy Street Nelson 7010, New Zealand

WWW. = ralasia.com | info@epd-australasia.com
ENVIRONMENTAL PRODUCT DECLARATION +64 9 889 2909

n Holcim (New Zealand) Ltd
EPD Produced by VU H O LC I1M 23 Plumer Street, Central Auckland 1010, New Zealand

www.holcim.co.nz

Epsten Group

EPD Process Certified by epstengroupæ Suite 2600, 101 Marietta St NW, Atlanta, Georgia 30303, USA

wWww.epstengroup.com

PCR 2019:14 Construction Products and Construction Services, Version 1.2.5, 2022-06-22
2021 Plant Data, 2023 Production Year

CEN standard EN 15804:2012+a1:2013 served as the core PCR

Product category rules PCR 2019:14 Construction Products and Construction Services, Version 1.2.5, 2022-06-22

The Technical Committee of the International EPD® System. Chair: Claudia A. Peña. Contact via

PCR review was conducted by info@environdec.com

Independent third-party verification
of the declaration and data,
according to ISO 14025:2006:

X EPD process certification
EPD verification

Epsten Group, Inc.
Accredited by: A2LA, Certificate #3142.03

EPD Process Certified by

Procedure for follow-up of data o
during EPD validity involves third
party verifier:

Yes
No

Programme-related information and verification

The EPD owner has the sole ownership, liability, and responsibility for the EPD. EPDs within the same product category
but from different programmes may not be comparable. EPDs of construction products may not be comparable if they do
not comply with EN 15804.

ENVIROCORE 201 EPD | 21
Contact your Holcim representative
today for more information.

Holcim (New Zealand) Ltd
23 Plumer Street

Central Auckland 1010
New Zealand

T 0800 465 246
www.holcim.co.nz

This publication supersedes all previous literature on this subject. As the specifications and details contained in this publication may change, please check
with Holcim Customer Service for confirmation of current issue. This publication provides general information only and is no substitute for professional
technical engineering advice. Users must make their own determination as to the suitability of this information or any Holcim product for their specific
circumstances. Holcim accepts no liability for any loss or damage resulting from their specific circumstances. Holcim accepts no liability for any loss or
damage resulting from any reliance on the information provided in this publication. Holcim is a registered trademark of Holcim Ltd.

© June 2023 Holcim (New Zealand) Ltd
Al rights reserved. This guide or any part of it may not be reproduced

U’HOLCIM

